lava/out/Benchmark/SoftwareFoundations.v
@@ -214,28 +214,28 @@ Proof.
   [refine (exist (λ (b2 : SFBool_u), SFBool_wf b2 ∧ True) b2 ltac:(solver)) | refine SFFalse].
 Defined.
 
-Definition andb3_spec (ds_d5Tg ds_d5Th ds_d5Ti : SFBool): Type :=
+Definition andb3_spec (ds_d5U1 ds_d5U2 ds_d5U3 : SFBool): Type :=
   SFBool.
 
 #[global] Hint Unfold andb3_spec: lia_unfold.
 
-Definition andb3 (ds_d5Tg ds_d5Th ds_d5Ti : SFBool): andb3_spec ds_d5Tg ds_d5Th ds_d5Ti.
+Definition andb3 (ds_d5U1 ds_d5U2 ds_d5U3 : SFBool): andb3_spec ds_d5U1 ds_d5U2 ds_d5U3.
 Proof.
-  destruct ds_d5Tg as [ds_d5Tg ds_d5Tg_p].
-  destruct ds_d5Th as [ds_d5Th ds_d5Th_p].
-  destruct ds_d5Ti as [ds_d5Ti ds_d5Ti_p].
-  destruct ds_d5Tg as [|].
+  destruct ds_d5U1 as [ds_d5U1 ds_d5U1_p].
+  destruct ds_d5U2 as [ds_d5U2 ds_d5U2_p].
+  destruct ds_d5U3 as [ds_d5U3 ds_d5U3_p].
+  destruct ds_d5U1 as [|].
   - refine SFFalse.
-  - destruct ds_d5Th as [|].
+  - destruct ds_d5U2 as [|].
     + refine SFFalse.
-    + destruct ds_d5Ti as [|].
+    + destruct ds_d5U3 as [|].
       * refine SFFalse.
       * refine SFTrue.
 Defined.
 
 Inductive andb3_rel: SFBool_u → SFBool_u → SFBool_u → SFBool_u → Prop :=
-  | andb3_SFFalse_x_x: ∀ ds_d5Th ds_d5Ti, andb3_rel SFFalse_u ds_d5Th ds_d5Ti SFFalse_u
-  | andb3_SFTrue_SFFalse_x: ∀ ds_d5Ti, andb3_rel SFTrue_u SFFalse_u ds_d5Ti SFFalse_u
+  | andb3_SFFalse_x_x: ∀ ds_d5U2 ds_d5U3, andb3_rel SFFalse_u ds_d5U2 ds_d5U3 SFFalse_u
+  | andb3_SFTrue_SFFalse_x: ∀ ds_d5U3, andb3_rel SFTrue_u SFFalse_u ds_d5U3 SFFalse_u
   | andb3_SFTrue_SFTrue_SFFalse: andb3_rel SFTrue_u SFTrue_u SFFalse_u SFFalse_u
   | andb3_SFTrue_SFTrue_SFTrue: andb3_rel SFTrue_u SFTrue_u SFTrue_u SFTrue_u.
 
@@ -245,14 +245,14 @@ Inductive andb3_rel: SFBool_u → SFBool_u → SFBool_u → SFBool_u → Prop :=
 
 #[global] Instance andb3_getF: getFunc andb3_rel := { getF' := andb3 }.
 
-Theorem andb3_rel_funct [ds_d5Tg ds_d5Th ds_d5Ti : SFBool_u]:
+Theorem andb3_rel_funct [ds_d5U1 ds_d5U2 ds_d5U3 : SFBool_u]:
   ∀ (VV VV' : SFBool_u),
-  andb3_rel ds_d5Tg ds_d5Th ds_d5Ti VV → (andb3_rel ds_d5Tg ds_d5Th ds_d5Ti VV' → VV = VV').
+  andb3_rel ds_d5U1 ds_d5U2 ds_d5U3 VV → (andb3_rel ds_d5U1 ds_d5U2 ds_d5U3 VV' → VV = VV').
 Proof.
-  destruct ds_d5Tg as [|];
+  destruct ds_d5U1 as [|];
   [ |
-   destruct ds_d5Th as [|];
-   [ | destruct ds_d5Ti as [|]]];
+   destruct ds_d5U2 as [|];
+   [ | destruct ds_d5U3 as [|]]];
   rel_functionhood_body.
 Qed.
 
@@ -261,8 +261,8 @@ Qed.
 #[global] Instance andb3_lookup_funct: dictionary functionhood andb3 := {
     lookup' := andb3_rel_funct }.
 
-Theorem andb3_SFFalse_x_x_lem ds_d5Th ds_d5Ti andb3_SFFalse_x_x_lem_res:
-  andb3_rel SFFalse_u ds_d5Th ds_d5Ti andb3_SFFalse_x_x_lem_res
+Theorem andb3_SFFalse_x_x_lem ds_d5U2 ds_d5U3 andb3_SFFalse_x_x_lem_res:
+  andb3_rel SFFalse_u ds_d5U2 ds_d5U3 andb3_SFFalse_x_x_lem_res
   ↔ andb3_SFFalse_x_x_lem_res == SFFalse_u.
 Proof.
   rel_back' _nil.
@@ -270,8 +270,8 @@ Qed.
 
 #[global] Hint Rewrite andb3_SFFalse_x_x_lem: f_rel_back.
 
-Theorem andb3_SFTrue_SFFalse_x_lem ds_d5Ti andb3_SFTrue_SFFalse_x_lem_res:
-  andb3_rel SFTrue_u SFFalse_u ds_d5Ti andb3_SFTrue_SFFalse_x_lem_res
+Theorem andb3_SFTrue_SFFalse_x_lem ds_d5U3 andb3_SFTrue_SFFalse_x_lem_res:
+  andb3_rel SFTrue_u SFFalse_u ds_d5U3 andb3_SFTrue_SFFalse_x_lem_res
   ↔ andb3_SFTrue_SFFalse_x_lem_res == SFFalse_u.
 Proof.
   rel_back' _nil.
@@ -298,25 +298,25 @@ Qed.
 #[global] Hint Rewrite andb3_SFTrue_SFTrue_SFTrue_lem: f_rel_back.
 
 Theorem andb3_rel_ex
-  (ds_d5Tg : SFBool_u)
-  (ds_d5Tg_p : SFBool_wf ds_d5Tg ∧ True)
-  (ds_d5Th : SFBool_u)
-  (ds_d5Th_p : SFBool_wf ds_d5Th ∧ True)
-  (ds_d5Ti : SFBool_u)
-  (ds_d5Ti_p : SFBool_wf ds_d5Ti ∧ True):
+  (ds_d5U1 : SFBool_u)
+  (ds_d5U1_p : SFBool_wf ds_d5U1 ∧ True)
+  (ds_d5U2 : SFBool_u)
+  (ds_d5U2_p : SFBool_wf ds_d5U2 ∧ True)
+  (ds_d5U3 : SFBool_u)
+  (ds_d5U3_p : SFBool_wf ds_d5U3 ∧ True):
   andb3_rel
-  ds_d5Tg
-  ds_d5Th
-  ds_d5Ti
-  ⌊ andb3 (exist _ ds_d5Tg ds_d5Tg_p) (exist _ ds_d5Th ds_d5Th_p) (exist _ ds_d5Ti ds_d5Ti_p) -⌋.
+  ds_d5U1
+  ds_d5U2
+  ds_d5U3
+  ⌊ andb3 (exist _ ds_d5U1 ds_d5U1_p) (exist _ ds_d5U2 ds_d5U2_p) (exist _ ds_d5U3 ds_d5U3_p) -⌋.
 Proof.
   Opaque andb3.
   existence_lemma_pre andb3;
-  destruct ds_d5Tg as [|];
+  destruct ds_d5U1 as [|];
   [fix_notations |
-   destruct ds_d5Th as [|];
+   destruct ds_d5U2 as [|];
    [fix_notations |
-    destruct ds_d5Ti as [|];
+    destruct ds_d5U3 as [|];
     [fix_notations | fix_notations]]];
   simpl in *.
   Transparent andb3.
@@ -328,15 +328,15 @@ Qed.
 #[global] Opaque andb3.
 
 Theorem andb3__andb3_rel_rw
-  (ds_d5Tg : SFBool_u)
-  (ds_d5Tg_p : SFBool_wf ds_d5Tg ∧ True)
-  (ds_d5Th : SFBool_u)
-  (ds_d5Th_p : SFBool_wf ds_d5Th ∧ True)
-  (ds_d5Ti : SFBool_u)
-  (ds_d5Ti_p : SFBool_wf ds_d5Ti ∧ True)
+  (ds_d5U1 : SFBool_u)
+  (ds_d5U1_p : SFBool_wf ds_d5U1 ∧ True)
+  (ds_d5U2 : SFBool_u)
+  (ds_d5U2_p : SFBool_wf ds_d5U2 ∧ True)
+  (ds_d5U3 : SFBool_u)
+  (ds_d5U3_p : SFBool_wf ds_d5U3 ∧ True)
   (VV : SFBool_u):
-  ⌊ andb3 (exist _ ds_d5Tg ds_d5Tg_p) (exist _ ds_d5Th ds_d5Th_p) (exist _ ds_d5Ti ds_d5Ti_p) -⌋ = VV
-  ↔ andb3_rel ds_d5Tg ds_d5Th ds_d5Ti VV.
+  ⌊ andb3 (exist _ ds_d5U1 ds_d5U1_p) (exist _ ds_d5U2 ds_d5U2_p) (exist _ ds_d5U3 ds_d5U3_p) -⌋ = VV
+  ↔ andb3_rel ds_d5U1 ds_d5U2 ds_d5U3 VV.
 Proof.
   f__f_rel_rw.
 Qed.
@@ -347,8 +347,8 @@ Qed.
 
 #[global] Instance andb3_lookup_rw: dictionary rwLem andb3 := { lookup' := andb3__andb3_rel_rw }.
 
-Theorem andb3__andb3_rel (ds_d5Tg ds_d5Th ds_d5Ti : SFBool) (VV : SFBool_u):
-  ⌊ andb3 ds_d5Tg ds_d5Th ds_d5Ti -⌋ = VV ↔ andb3_rel ⌊ ds_d5Tg ⌋ ⌊ ds_d5Th ⌋ ⌊ ds_d5Ti ⌋ VV.
+Theorem andb3__andb3_rel (ds_d5U1 ds_d5U2 ds_d5U3 : SFBool) (VV : SFBool_u):
+  ⌊ andb3 ds_d5U1 ds_d5U2 ds_d5U3 -⌋ = VV ↔ andb3_rel ⌊ ds_d5U1 ⌋ ⌊ ds_d5U2 ⌋ ⌊ ds_d5U3 ⌋ VV.
 Proof.
   f__f_rel.
 Qed.
@@ -356,31 +356,31 @@ Qed.
 #[global] Hint Rewrite andb3__andb3_rel: f_rel_funct_db.
 
 Theorem andb3__andb3_rel'
-  (ds_d5Tg_u ds_d5Th_u ds_d5Ti_u : SFBool_u) (ds_d5Tg ds_d5Th ds_d5Ti : SFBool) (VV : SFBool_u):
-  ds_d5Tg_u = ⌊ ds_d5Tg ⌋
-  → (ds_d5Th_u = ⌊ ds_d5Th ⌋
-     → (ds_d5Ti_u = ⌊ ds_d5Ti ⌋
-        → ⌊ andb3 ds_d5Tg ds_d5Th ds_d5Ti -⌋ = VV ↔ andb3_rel ds_d5Tg_u ds_d5Th_u ds_d5Ti_u VV)).
+  (ds_d5U1_u ds_d5U2_u ds_d5U3_u : SFBool_u) (ds_d5U1 ds_d5U2 ds_d5U3 : SFBool) (VV : SFBool_u):
+  ds_d5U1_u = ⌊ ds_d5U1 ⌋
+  → (ds_d5U2_u = ⌊ ds_d5U2 ⌋
+     → (ds_d5U3_u = ⌊ ds_d5U3 ⌋
+        → ⌊ andb3 ds_d5U1 ds_d5U2 ds_d5U3 -⌋ = VV ↔ andb3_rel ds_d5U1_u ds_d5U2_u ds_d5U3_u VV)).
 Proof.
-  intros -> -> ->. refine (andb3__andb3_rel ds_d5Tg ds_d5Th ds_d5Ti VV).
+  intros -> -> ->. refine (andb3__andb3_rel ds_d5U1 ds_d5U2 ds_d5U3 VV).
 Qed.
 
 #[global] Hint Resolve andb3__andb3_rel': f_rel_funct_db.
 
 Theorem andb3_rel_mk
-  (ds_d5Tg : SFBool_u)
-  (ds_d5Tg_p : SFBool_wf ds_d5Tg ∧ True)
-  (ds_d5Th : SFBool_u)
-  (ds_d5Th_p : SFBool_wf ds_d5Th ∧ True)
-  (ds_d5Ti : SFBool_u)
-  (ds_d5Ti_p : SFBool_wf ds_d5Ti ∧ True):
-  {VV: _ | andb3_rel ds_d5Tg ds_d5Th ds_d5Ti VV}.
+  (ds_d5U1 : SFBool_u)
+  (ds_d5U1_p : SFBool_wf ds_d5U1 ∧ True)
+  (ds_d5U2 : SFBool_u)
+  (ds_d5U2_p : SFBool_wf ds_d5U2 ∧ True)
+  (ds_d5U3 : SFBool_u)
+  (ds_d5U3_p : SFBool_wf ds_d5U3 ∧ True):
+  {VV: _ | andb3_rel ds_d5U1 ds_d5U2 ds_d5U3 VV}.
 Proof.
   intros;
   refine (subsumptionCast
           _
-          (λ VV, andb3_rel ds_d5Tg ds_d5Th ds_d5Ti VV)
-          (andb3 (exist _ ds_d5Tg ds_d5Tg_p) (exist _ ds_d5Th ds_d5Th_p) (exist _ ds_d5Ti ds_d5Ti_p))
+          (λ VV, andb3_rel ds_d5U1 ds_d5U2 ds_d5U3 VV)
+          (andb3 (exist _ ds_d5U1 ds_d5U1_p) (exist _ ds_d5U2 ds_d5U2_p) (exist _ ds_d5U3 ds_d5U3_p))
           _);
   rewrite <- andb3__andb3_rel';
   quicksolve.
@@ -391,20 +391,20 @@ Qed.
 #[global] Instance andb3_pack:
   @Pack
   (SFBool
-   ::RT λ (ds_d5Tg : SFBool),
-        SFBool ::RT λ (ds_d5Th : SFBool), SFBool ::RT λ (ds_d5Ti : SFBool), nilRT)
+   ::RT λ (ds_d5U1 : SFBool),
+        SFBool ::RT λ (ds_d5U2 : SFBool), SFBool ::RT λ (ds_d5U3 : SFBool), nilRT)
   (SFBool_u ::UT (SFBool_u ::UT (SFBool_u ::UT nilUT)))
   ltac:(mkProjectsArgListTG (SFBool
- ::RT λ (ds_d5Tg : SFBool),
+ ::RT λ (ds_d5U1 : SFBool),
       SFBool
-      ::RT λ (ds_d5Th : SFBool), SFBool ::RT λ (ds_d5Ti : SFBool), nilRT) ((SFBool_u ::UT (SFBool_u ::UT (SFBool_u ::UT nilUT)))))
+      ::RT λ (ds_d5U2 : SFBool), SFBool ::RT λ (ds_d5U3 : SFBool), nilRT) ((SFBool_u ::UT (SFBool_u ::UT (SFBool_u ::UT nilUT)))))
   SFBool_u
-  (λ (x_79501799 : ArgList (SFBool
-                            ::RT λ (ds_d5Tg : SFBool),
-                                 SFBool ::RT λ (ds_d5Th : SFBool), SFBool ::RT λ (ds_d5Ti : SFBool), nilRT))
-     (v_x_79501799 : SFBool_u),
-   ltac:(flattenP (λ (ds_d5Tg ds_d5Th ds_d5Ti : SFBool) (VV : SFBool_u),
- SFBool_wf VV ∧ True) x_79501799 v_x_79501799)).
+  (λ (x_22068354 : ArgList (SFBool
+                            ::RT λ (ds_d5U1 : SFBool),
+                                 SFBool ::RT λ (ds_d5U2 : SFBool), SFBool ::RT λ (ds_d5U3 : SFBool), nilRT))
+     (v_x_22068354 : SFBool_u),
+   ltac:(flattenP (λ (ds_d5U1 ds_d5U2 ds_d5U3 : SFBool) (VV : SFBool_u),
+ SFBool_wf VV ∧ True) x_22068354 v_x_22068354)).
 Proof.
   buildPackG andb3 andb3_rel andb3__andb3_rel andb3_rel_funct.
 Defined.
@@ -479,20 +479,20 @@ Proof.
           ltac:(solver)).
 Qed.
 
-Definition andb_commutative_spec (ds_d5Sf ds_d5Sg : SFBool): Type :=
+Definition andb_commutative_spec (ds_d5T0 ds_d5T1 : SFBool): Type :=
   {{∃ (andb_res : SFBool_u),
-    andb_rel ⌊ ds_d5Sf -⌋ ⌊ ds_d5Sg -⌋ andb_res
+    andb_rel ⌊ ds_d5T0 -⌋ ⌊ ds_d5T1 -⌋ andb_res
     ∧ ∃ (andb_res_2 : SFBool_u),
-      andb_rel ⌊ ds_d5Sg -⌋ ⌊ ds_d5Sf -⌋ andb_res_2 ∧ andb_res == andb_res_2}}.
+      andb_rel ⌊ ds_d5T1 -⌋ ⌊ ds_d5T0 -⌋ andb_res_2 ∧ andb_res == andb_res_2}}.
 
 #[global] Hint Unfold andb_commutative_spec: lia_unfold.
 
-Theorem andb_commutative (ds_d5Sf ds_d5Sg : SFBool): andb_commutative_spec ds_d5Sf ds_d5Sg.
+Theorem andb_commutative (ds_d5T0 ds_d5T1 : SFBool): andb_commutative_spec ds_d5T0 ds_d5T1.
 Proof.
-  destruct ds_d5Sf as [ds_d5Sf ds_d5Sf_p].
-  destruct ds_d5Sg as [ds_d5Sg ds_d5Sg_p].
-  destruct ds_d5Sf as [|].
-  - destruct ds_d5Sg as [|].
+  destruct ds_d5T0 as [ds_d5T0 ds_d5T0_p].
+  destruct ds_d5T1 as [ds_d5T1 ds_d5T1_p].
+  destruct ds_d5T0 as [|].
+  - destruct ds_d5T1 as [|].
     + refine (subsumptionCast
               Unit
               (λ (VV : Unit),
@@ -509,7 +509,7 @@ Proof.
                ∧ ∃ (andb_res_2 : SFBool_u), andb_rel SFTrue_u SFFalse_u andb_res_2 ∧ andb_res == andb_res_2)
               (# unit)
               ltac:(solver)).
-  - destruct ds_d5Sg as [|].
+  - destruct ds_d5T1 as [|].
     + refine (subsumptionCast
               Unit
               (λ (VV : Unit),
@@ -529,50 +529,99 @@ Proof.
 Qed.
 
 Definition andb_true_elim2_spec
-  (ds_d5Sc ds_d5Sd : SFBool)
-  (ds_d5Se : {{∃ (andb_res : SFBool_u),
-               andb_rel ⌊ ds_d5Sc -⌋ ⌊ ds_d5Sd -⌋ andb_res ∧ andb_res == SFTrue_u}}):
+  (ds_d5SX ds_d5SY : SFBool)
+  (ds_d5SZ : {{∃ (andb_res : SFBool_u),
+               andb_rel ⌊ ds_d5SX -⌋ ⌊ ds_d5SY -⌋ andb_res ∧ andb_res == SFTrue_u}}):
   Type :=
-  {{⌊ ds_d5Sd -⌋ == SFTrue_u}}.
+  {{⌊ ds_d5SY -⌋ == SFTrue_u}}.
 
 #[global] Hint Unfold andb_true_elim2_spec: lia_unfold.
 
 Theorem andb_true_elim2
-  (ds_d5Sc ds_d5Sd : SFBool)
-  (ds_d5Se : {{∃ (andb_res : SFBool_u),
-               andb_rel ⌊ ds_d5Sc -⌋ ⌊ ds_d5Sd -⌋ andb_res ∧ andb_res == SFTrue_u}}):
-  andb_true_elim2_spec ds_d5Sc ds_d5Sd ds_d5Se.
+  (ds_d5SX ds_d5SY : SFBool)
+  (ds_d5SZ : {{∃ (andb_res : SFBool_u),
+               andb_rel ⌊ ds_d5SX -⌋ ⌊ ds_d5SY -⌋ andb_res ∧ andb_res == SFTrue_u}}):
+  andb_true_elim2_spec ds_d5SX ds_d5SY ds_d5SZ.
 Proof.
-  destruct ds_d5Sc as [ds_d5Sc ds_d5Sc_p].
-  destruct ds_d5Sd as [ds_d5Sd ds_d5Sd_p].
-  destruct ds_d5Se as [ds_d5Se ds_d5Se_p].
-  destruct ds_d5Sc as [|].
-  - destruct ds_d5Sd as [|].
+  destruct ds_d5SX as [ds_d5SX ds_d5SX_p].
+  destruct ds_d5SY as [ds_d5SY ds_d5SY_p].
+  destruct ds_d5SZ as [ds_d5SZ ds_d5SZ_p].
+  destruct ds_d5SX as [|].
+  - destruct ds_d5SY as [|].
     + refine (subsumptionCast Unit (λ (VV : Unit), SFFalse_u == SFTrue_u) (# unit) ltac:(solver)).
     + refine (subsumptionCast Unit (λ (VV : Unit), SFTrue_u == SFTrue_u) (# unit) ltac:(solver)).
-  - destruct ds_d5Sd as [|].
+  - destruct ds_d5SY as [|].
     + refine (subsumptionCast Unit (λ (VV : Unit), SFFalse_u == SFTrue_u) (# unit) ltac:(solver)).
     + refine (subsumptionCast Unit (λ (VV : Unit), SFTrue_u == SFTrue_u) (# unit) ltac:(solver)).
 Qed.
 
-Definition nandb_spec (ds_d5Tn ds_d5To : SFBool): Type :=
+Definition identity_fn_applied_twice_spec
+  (f : @Pack
+       (SFBool ::RT λ (lq_tmp0 : SFBool), nilRT)
+       (SFBool_u ::UT nilUT)
+       ltac:(mkProjectsArgListTG (SFBool ::RT λ (lq_tmp0 : SFBool), nilRT) ((SFBool_u ::UT nilUT)))
+       SFBool_u
+       (λ (x_80611037 : ArgList (SFBool ::RT λ (lq_tmp0 : SFBool), nilRT)) (v_x_80611037 : SFBool_u),
+        ltac:(flattenP (λ (lq_tmp0 : SFBool) (VV : SFBool_u), SFBool_wf VV ∧ True) x_80611037 v_x_80611037)))
+  (h : ∀ (x : SFBool), {{∃ (f_res : SFBool_u), getPackRel f ⌊ x -⌋ f_res ∧ f_res == ⌊ x -⌋}})
+  (b : SFBool):
+  Type :=
+  {{∃ (f_res : SFBool_u),
+    getPackRel f ⌊ b -⌋ f_res
+    ∧ ∃ (f_res_2 : SFBool_u), getPackRel f f_res f_res_2 ∧ f_res_2 == ⌊ b -⌋}}.
+
+#[global] Hint Unfold identity_fn_applied_twice_spec: lia_unfold.
+
+Theorem identity_fn_applied_twice
+  (f : @Pack
+       (SFBool ::RT λ (lq_tmp0 : SFBool), nilRT)
+       (SFBool_u ::UT nilUT)
+       ltac:(mkProjectsArgListTG (SFBool ::RT λ (lq_tmp0 : SFBool), nilRT) ((SFBool_u ::UT nilUT)))
+       SFBool_u
+       (λ (x_80611037 : ArgList (SFBool ::RT λ (lq_tmp0 : SFBool), nilRT)) (v_x_80611037 : SFBool_u),
+        ltac:(flattenP (λ (lq_tmp0 : SFBool) (VV : SFBool_u), SFBool_wf VV ∧ True) x_80611037 v_x_80611037)))
+  (h : ∀ (x : SFBool), {{∃ (f_res : SFBool_u), getPackRel f ⌊ x -⌋ f_res ∧ f_res == ⌊ x -⌋}})
+  (b : SFBool):
+  identity_fn_applied_twice_spec f h b.
+Proof.
+  destruct b as [b b_p].
+  try assert (b_inj_wit_58609636 : (λ (b : SFBool_u), SFBool_wf b ∧ True) b) by (solver).
+  pose (exist (λ (b : SFBool_u), SFBool_wf b ∧ True) b b_inj_wit_58609636) as h_64017348_1.
+  pose (h h_64017348_1) as h_64017348.
+  try assert (b_inj_wit_58609636 : (λ (b : SFBool_u), SFBool_wf b ∧ True) b) by (solver).
+  pose (exist (λ (b : SFBool_u), SFBool_wf b ∧ True) b b_inj_wit_58609636) as h_21480545_1_1.
+  pose (getPackF f h_21480545_1_1) as h_21480545_1.
+  pose (h h_21480545_1) as h_21480545.
+  try assert (b_inj_wit_58609636 : (λ (b : SFBool_u), SFBool_wf b ∧ True) b) by (solver).
+  pose (exist (λ (b : SFBool_u), SFBool_wf b ∧ True) b b_inj_wit_58609636) as x_19873709_1_1.
+  pose (getPackF f x_19873709_1_1) as x_19873709_1.
+  pose (getPackF f x_19873709_1) as x_19873709.
+  pose (getPackF f (exist (λ (b : SFBool_u), SFBool_wf b ∧ True) b ltac:(solver))) as h_74969166.
+  pose (exist (λ (b : SFBool_u), SFBool_wf b ∧ True) b ltac:(solver)) as h_35781707.
+  refine (exist (λ (VV : Unit),
+                 ∃ (f_res : SFBool_u),
+                 getPackRel f b f_res
+                 ∧ ∃ (f_res_2 : SFBool_u), getPackRel f f_res f_res_2 ∧ f_res_2 == b) unit ltac:(solver)).
+Qed.
+
+Definition nandb_spec (ds_d5U8 ds_d5U9 : SFBool): Type :=
   SFBool.
 
 #[global] Hint Unfold nandb_spec: lia_unfold.
 
-Definition nandb (ds_d5Tn ds_d5To : SFBool): nandb_spec ds_d5Tn ds_d5To.
+Definition nandb (ds_d5U8 ds_d5U9 : SFBool): nandb_spec ds_d5U8 ds_d5U9.
 Proof.
-  destruct ds_d5Tn as [ds_d5Tn ds_d5Tn_p].
-  destruct ds_d5To as [ds_d5To ds_d5To_p].
-  destruct ds_d5Tn as [|].
+  destruct ds_d5U8 as [ds_d5U8 ds_d5U8_p].
+  destruct ds_d5U9 as [ds_d5U9 ds_d5U9_p].
+  destruct ds_d5U8 as [|].
   - refine SFTrue.
-  - destruct ds_d5To as [|].
+  - destruct ds_d5U9 as [|].
     + refine SFTrue.
     + refine SFFalse.
 Defined.
 
 Inductive nandb_rel: SFBool_u → SFBool_u → SFBool_u → Prop :=
-  | nandb_SFFalse_x: ∀ ds_d5To, nandb_rel SFFalse_u ds_d5To SFTrue_u
+  | nandb_SFFalse_x: ∀ ds_d5U9, nandb_rel SFFalse_u ds_d5U9 SFTrue_u
   | nandb_SFTrue_SFFalse: nandb_rel SFTrue_u SFFalse_u SFTrue_u
   | nandb_SFTrue_SFTrue: nandb_rel SFTrue_u SFTrue_u SFFalse_u.
 
@@ -582,11 +631,11 @@ Inductive nandb_rel: SFBool_u → SFBool_u → SFBool_u → Prop :=
 
 #[global] Instance nandb_getF: getFunc nandb_rel := { getF' := nandb }.
 
-Theorem nandb_rel_funct [ds_d5Tn ds_d5To : SFBool_u]:
-  ∀ (VV VV' : SFBool_u), nandb_rel ds_d5Tn ds_d5To VV → (nandb_rel ds_d5Tn ds_d5To VV' → VV = VV').
+Theorem nandb_rel_funct [ds_d5U8 ds_d5U9 : SFBool_u]:
+  ∀ (VV VV' : SFBool_u), nandb_rel ds_d5U8 ds_d5U9 VV → (nandb_rel ds_d5U8 ds_d5U9 VV' → VV = VV').
 Proof.
-  destruct ds_d5Tn as [|];
-  [ | destruct ds_d5To as [|]];
+  destruct ds_d5U8 as [|];
+  [ | destruct ds_d5U9 as [|]];
   rel_functionhood_body.
 Qed.
 
@@ -595,8 +644,8 @@ Qed.
 #[global] Instance nandb_lookup_funct: dictionary functionhood nandb := {
     lookup' := nandb_rel_funct }.
 
-Theorem nandb_SFFalse_x_lem ds_d5To nandb_SFFalse_x_lem_res:
-  nandb_rel SFFalse_u ds_d5To nandb_SFFalse_x_lem_res ↔ nandb_SFFalse_x_lem_res == SFTrue_u.
+Theorem nandb_SFFalse_x_lem ds_d5U9 nandb_SFFalse_x_lem_res:
+  nandb_rel SFFalse_u ds_d5U9 nandb_SFFalse_x_lem_res ↔ nandb_SFFalse_x_lem_res == SFTrue_u.
 Proof.
   rel_back' _nil.
 Qed.
@@ -621,17 +670,17 @@ Qed.
 #[global] Hint Rewrite nandb_SFTrue_SFTrue_lem: f_rel_back.
 
 Theorem nandb_rel_ex
-  (ds_d5Tn : SFBool_u)
-  (ds_d5Tn_p : SFBool_wf ds_d5Tn ∧ True)
-  (ds_d5To : SFBool_u)
-  (ds_d5To_p : SFBool_wf ds_d5To ∧ True):
-  nandb_rel ds_d5Tn ds_d5To ⌊ nandb (exist _ ds_d5Tn ds_d5Tn_p) (exist _ ds_d5To ds_d5To_p) -⌋.
+  (ds_d5U8 : SFBool_u)
+  (ds_d5U8_p : SFBool_wf ds_d5U8 ∧ True)
+  (ds_d5U9 : SFBool_u)
+  (ds_d5U9_p : SFBool_wf ds_d5U9 ∧ True):
+  nandb_rel ds_d5U8 ds_d5U9 ⌊ nandb (exist _ ds_d5U8 ds_d5U8_p) (exist _ ds_d5U9 ds_d5U9_p) -⌋.
 Proof.
   Opaque nandb.
   existence_lemma_pre nandb;
-  destruct ds_d5Tn as [|];
+  destruct ds_d5U8 as [|];
   [fix_notations |
-   destruct ds_d5To as [|];
+   destruct ds_d5U9 as [|];
    [fix_notations | fix_notations]];
   simpl in *.
   Transparent nandb.
@@ -643,13 +692,13 @@ Qed.
 #[global] Opaque nandb.
 
 Theorem nandb__nandb_rel_rw
-  (ds_d5Tn : SFBool_u)
-  (ds_d5Tn_p : SFBool_wf ds_d5Tn ∧ True)
-  (ds_d5To : SFBool_u)
-  (ds_d5To_p : SFBool_wf ds_d5To ∧ True)
+  (ds_d5U8 : SFBool_u)
+  (ds_d5U8_p : SFBool_wf ds_d5U8 ∧ True)
+  (ds_d5U9 : SFBool_u)
+  (ds_d5U9_p : SFBool_wf ds_d5U9 ∧ True)
   (VV : SFBool_u):
-  ⌊ nandb (exist _ ds_d5Tn ds_d5Tn_p) (exist _ ds_d5To ds_d5To_p) -⌋ = VV
-  ↔ nandb_rel ds_d5Tn ds_d5To VV.
+  ⌊ nandb (exist _ ds_d5U8 ds_d5U8_p) (exist _ ds_d5U9 ds_d5U9_p) -⌋ = VV
+  ↔ nandb_rel ds_d5U8 ds_d5U9 VV.
 Proof.
   f__f_rel_rw.
 Qed.
@@ -660,8 +709,8 @@ Qed.
 
 #[global] Instance nandb_lookup_rw: dictionary rwLem nandb := { lookup' := nandb__nandb_rel_rw }.
 
-Theorem nandb__nandb_rel (ds_d5Tn ds_d5To : SFBool) (VV : SFBool_u):
-  ⌊ nandb ds_d5Tn ds_d5To -⌋ = VV ↔ nandb_rel ⌊ ds_d5Tn ⌋ ⌊ ds_d5To ⌋ VV.
+Theorem nandb__nandb_rel (ds_d5U8 ds_d5U9 : SFBool) (VV : SFBool_u):
+  ⌊ nandb ds_d5U8 ds_d5U9 -⌋ = VV ↔ nandb_rel ⌊ ds_d5U8 ⌋ ⌊ ds_d5U9 ⌋ VV.
 Proof.
   f__f_rel.
 Qed.
@@ -669,27 +718,27 @@ Qed.
 #[global] Hint Rewrite nandb__nandb_rel: f_rel_funct_db.
 
 Theorem nandb__nandb_rel'
-  (ds_d5Tn_u ds_d5To_u : SFBool_u) (ds_d5Tn ds_d5To : SFBool) (VV : SFBool_u):
-  ds_d5Tn_u = ⌊ ds_d5Tn ⌋
-  → (ds_d5To_u = ⌊ ds_d5To ⌋ → ⌊ nandb ds_d5Tn ds_d5To -⌋ = VV ↔ nandb_rel ds_d5Tn_u ds_d5To_u VV).
+  (ds_d5U8_u ds_d5U9_u : SFBool_u) (ds_d5U8 ds_d5U9 : SFBool) (VV : SFBool_u):
+  ds_d5U8_u = ⌊ ds_d5U8 ⌋
+  → (ds_d5U9_u = ⌊ ds_d5U9 ⌋ → ⌊ nandb ds_d5U8 ds_d5U9 -⌋ = VV ↔ nandb_rel ds_d5U8_u ds_d5U9_u VV).
 Proof.
-  intros -> ->. refine (nandb__nandb_rel ds_d5Tn ds_d5To VV).
+  intros -> ->. refine (nandb__nandb_rel ds_d5U8 ds_d5U9 VV).
 Qed.
 
 #[global] Hint Resolve nandb__nandb_rel': f_rel_funct_db.
 
 Theorem nandb_rel_mk
-  (ds_d5Tn : SFBool_u)
-  (ds_d5Tn_p : SFBool_wf ds_d5Tn ∧ True)
-  (ds_d5To : SFBool_u)
-  (ds_d5To_p : SFBool_wf ds_d5To ∧ True):
-  {VV: _ | nandb_rel ds_d5Tn ds_d5To VV}.
+  (ds_d5U8 : SFBool_u)
+  (ds_d5U8_p : SFBool_wf ds_d5U8 ∧ True)
+  (ds_d5U9 : SFBool_u)
+  (ds_d5U9_p : SFBool_wf ds_d5U9 ∧ True):
+  {VV: _ | nandb_rel ds_d5U8 ds_d5U9 VV}.
 Proof.
   intros;
   refine (subsumptionCast
           _
-          (λ VV, nandb_rel ds_d5Tn ds_d5To VV)
-          (nandb (exist _ ds_d5Tn ds_d5Tn_p) (exist _ ds_d5To ds_d5To_p))
+          (λ VV, nandb_rel ds_d5U8 ds_d5U9 VV)
+          (nandb (exist _ ds_d5U8 ds_d5U8_p) (exist _ ds_d5U9 ds_d5U9_p))
           _);
   rewrite <- nandb__nandb_rel';
   quicksolve.
@@ -699,15 +748,15 @@ Qed.
 
 #[global] Instance nandb_pack:
   @Pack
-  (SFBool ::RT λ (ds_d5Tn : SFBool), SFBool ::RT λ (ds_d5To : SFBool), nilRT)
+  (SFBool ::RT λ (ds_d5U8 : SFBool), SFBool ::RT λ (ds_d5U9 : SFBool), nilRT)
   (SFBool_u ::UT (SFBool_u ::UT nilUT))
   ltac:(mkProjectsArgListTG (SFBool
- ::RT λ (ds_d5Tn : SFBool), SFBool ::RT λ (ds_d5To : SFBool), nilRT) ((SFBool_u ::UT (SFBool_u ::UT nilUT))))
+ ::RT λ (ds_d5U8 : SFBool), SFBool ::RT λ (ds_d5U9 : SFBool), nilRT) ((SFBool_u ::UT (SFBool_u ::UT nilUT))))
   SFBool_u
-  (λ (x_91705089 : ArgList (SFBool
-                            ::RT λ (ds_d5Tn : SFBool), SFBool ::RT λ (ds_d5To : SFBool), nilRT))
-     (v_x_91705089 : SFBool_u),
-   ltac:(flattenP (λ (ds_d5Tn ds_d5To : SFBool) (VV : SFBool_u), SFBool_wf VV ∧ True) x_91705089 v_x_91705089)).
+  (λ (x_53018143 : ArgList (SFBool
+                            ::RT λ (ds_d5U8 : SFBool), SFBool ::RT λ (ds_d5U9 : SFBool), nilRT))
+     (v_x_53018143 : SFBool_u),
+   ltac:(flattenP (λ (ds_d5U8 ds_d5U9 : SFBool) (VV : SFBool_u), SFBool_wf VV ∧ True) x_53018143 v_x_53018143)).
 Proof.
   buildPackG nandb nandb_rel nandb__nandb_rel nandb_rel_funct.
 Defined.
@@ -777,15 +826,15 @@ Proof.
           ltac:(solver)).
 Qed.
 
-Definition negb_spec (ds_d5Tv : SFBool): Type :=
+Definition negb_spec (ds_d5Ug : SFBool): Type :=
   SFBool.
 
 #[global] Hint Unfold negb_spec: lia_unfold.
 
-Definition negb (ds_d5Tv : SFBool): negb_spec ds_d5Tv.
+Definition negb (ds_d5Ug : SFBool): negb_spec ds_d5Ug.
 Proof.
-  destruct ds_d5Tv as [ds_d5Tv ds_d5Tv_p].
-  destruct ds_d5Tv as [|].
+  destruct ds_d5Ug as [ds_d5Ug ds_d5Ug_p].
+  destruct ds_d5Ug as [|].
   - refine SFTrue.
   - refine SFFalse.
 Defined.
@@ -799,10 +848,10 @@ Inductive negb_rel: SFBool_u → SFBool_u → Prop :=
 
 #[global] Instance negb_getF: getFunc negb_rel := { getF' := negb }.
 
-Theorem negb_rel_funct [ds_d5Tv : SFBool_u]:
-  ∀ (VV VV' : SFBool_u), negb_rel ds_d5Tv VV → (negb_rel ds_d5Tv VV' → VV = VV').
+Theorem negb_rel_funct [ds_d5Ug : SFBool_u]:
+  ∀ (VV VV' : SFBool_u), negb_rel ds_d5Ug VV → (negb_rel ds_d5Ug VV' → VV = VV').
 Proof.
-  destruct ds_d5Tv as [|]; rel_functionhood_body.
+  destruct ds_d5Ug as [|]; rel_functionhood_body.
 Qed.
 
 #[global] Hint Resolve negb_rel_funct: f_rel_funct_db.
@@ -826,12 +875,12 @@ Qed.
 
 #[global] Hint Rewrite negb_SFTrue_lem: f_rel_back.
 
-Theorem negb_rel_ex (ds_d5Tv : SFBool_u) (ds_d5Tv_p : SFBool_wf ds_d5Tv ∧ True):
-  negb_rel ds_d5Tv ⌊ negb (exist _ ds_d5Tv ds_d5Tv_p) -⌋.
+Theorem negb_rel_ex (ds_d5Ug : SFBool_u) (ds_d5Ug_p : SFBool_wf ds_d5Ug ∧ True):
+  negb_rel ds_d5Ug ⌊ negb (exist _ ds_d5Ug ds_d5Ug_p) -⌋.
 Proof.
   Opaque negb.
   existence_lemma_pre negb;
-  destruct ds_d5Tv as [|];
+  destruct ds_d5Ug as [|];
   [fix_notations | fix_notations];
   simpl in *.
   Transparent negb.
@@ -843,8 +892,8 @@ Qed.
 #[global] Opaque negb.
 
 Theorem negb__negb_rel_rw
-  (ds_d5Tv : SFBool_u) (ds_d5Tv_p : SFBool_wf ds_d5Tv ∧ True) (VV : SFBool_u):
-  ⌊ negb (exist _ ds_d5Tv ds_d5Tv_p) -⌋ = VV ↔ negb_rel ds_d5Tv VV.
+  (ds_d5Ug : SFBool_u) (ds_d5Ug_p : SFBool_wf ds_d5Ug ∧ True) (VV : SFBool_u):
+  ⌊ negb (exist _ ds_d5Ug ds_d5Ug_p) -⌋ = VV ↔ negb_rel ds_d5Ug VV.
 Proof.
   f__f_rel_rw.
 Qed.
@@ -855,27 +904,27 @@ Qed.
 
 #[global] Instance negb_lookup_rw: dictionary rwLem negb := { lookup' := negb__negb_rel_rw }.
 
-Theorem negb__negb_rel (ds_d5Tv : SFBool) (VV : SFBool_u):
-  ⌊ negb ds_d5Tv -⌋ = VV ↔ negb_rel ⌊ ds_d5Tv ⌋ VV.
+Theorem negb__negb_rel (ds_d5Ug : SFBool) (VV : SFBool_u):
+  ⌊ negb ds_d5Ug -⌋ = VV ↔ negb_rel ⌊ ds_d5Ug ⌋ VV.
 Proof.
   f__f_rel.
 Qed.
 
 #[global] Hint Rewrite negb__negb_rel: f_rel_funct_db.
 
-Theorem negb__negb_rel' (ds_d5Tv_u : SFBool_u) (ds_d5Tv : SFBool) (VV : SFBool_u):
-  ds_d5Tv_u = ⌊ ds_d5Tv ⌋ → ⌊ negb ds_d5Tv -⌋ = VV ↔ negb_rel ds_d5Tv_u VV.
+Theorem negb__negb_rel' (ds_d5Ug_u : SFBool_u) (ds_d5Ug : SFBool) (VV : SFBool_u):
+  ds_d5Ug_u = ⌊ ds_d5Ug ⌋ → ⌊ negb ds_d5Ug -⌋ = VV ↔ negb_rel ds_d5Ug_u VV.
 Proof.
-  intros ->. refine (negb__negb_rel ds_d5Tv VV).
+  intros ->. refine (negb__negb_rel ds_d5Ug VV).
 Qed.
 
 #[global] Hint Resolve negb__negb_rel': f_rel_funct_db.
 
-Theorem negb_rel_mk (ds_d5Tv : SFBool_u) (ds_d5Tv_p : SFBool_wf ds_d5Tv ∧ True):
-  {VV: _ | negb_rel ds_d5Tv VV}.
+Theorem negb_rel_mk (ds_d5Ug : SFBool_u) (ds_d5Ug_p : SFBool_wf ds_d5Ug ∧ True):
+  {VV: _ | negb_rel ds_d5Ug VV}.
 Proof.
   intros;
-  refine (subsumptionCast _ (λ VV, negb_rel ds_d5Tv VV) (negb (exist _ ds_d5Tv ds_d5Tv_p)) _);
+  refine (subsumptionCast _ (λ VV, negb_rel ds_d5Ug VV) (negb (exist _ ds_d5Ug ds_d5Ug_p)) _);
   rewrite <- negb__negb_rel';
   quicksolve.
 Qed.
@@ -884,12 +933,12 @@ Qed.
 
 #[global] Instance negb_pack:
   @Pack
-  (SFBool ::RT λ (ds_d5Tv : SFBool), nilRT)
+  (SFBool ::RT λ (ds_d5Ug : SFBool), nilRT)
   (SFBool_u ::UT nilUT)
-  ltac:(mkProjectsArgListTG (SFBool ::RT λ (ds_d5Tv : SFBool), nilRT) ((SFBool_u ::UT nilUT)))
+  ltac:(mkProjectsArgListTG (SFBool ::RT λ (ds_d5Ug : SFBool), nilRT) ((SFBool_u ::UT nilUT)))
   SFBool_u
-  (λ (x_94703936 : ArgList (SFBool ::RT λ (ds_d5Tv : SFBool), nilRT)) (v_x_94703936 : SFBool_u),
-   ltac:(flattenP (λ (ds_d5Tv : SFBool) (VV : SFBool_u), SFBool_wf VV ∧ True) x_94703936 v_x_94703936)).
+  (λ (x_77100824 : ArgList (SFBool ::RT λ (ds_d5Ug : SFBool), nilRT)) (v_x_77100824 : SFBool_u),
+   ltac:(flattenP (λ (ds_d5Ug : SFBool) (VV : SFBool_u), SFBool_wf VV ∧ True) x_77100824 v_x_77100824)).
 Proof.
   buildPackG negb negb_rel negb__negb_rel negb_rel_funct.
 Defined.
@@ -911,17 +960,17 @@ Proof.
   [refine SFFalse | refine SFTrue].
 Defined.
 
-Definition negb_involutive_spec (ds_d5Sh : SFBool): Type :=
+Definition negb_involutive_spec (ds_d5T2 : SFBool): Type :=
   {{∃ (negb_res : SFBool_u),
-    negb_rel ⌊ ds_d5Sh -⌋ negb_res
-    ∧ ∃ (negb_res_2 : SFBool_u), negb_rel negb_res negb_res_2 ∧ negb_res_2 == ⌊ ds_d5Sh -⌋}}.
+    negb_rel ⌊ ds_d5T2 -⌋ negb_res
+    ∧ ∃ (negb_res_2 : SFBool_u), negb_rel negb_res negb_res_2 ∧ negb_res_2 == ⌊ ds_d5T2 -⌋}}.
 
 #[global] Hint Unfold negb_involutive_spec: lia_unfold.
 
-Theorem negb_involutive (ds_d5Sh : SFBool): negb_involutive_spec ds_d5Sh.
+Theorem negb_involutive (ds_d5T2 : SFBool): negb_involutive_spec ds_d5T2.
 Proof.
-  destruct ds_d5Sh as [ds_d5Sh ds_d5Sh_p].
-  destruct ds_d5Sh as [|].
+  destruct ds_d5T2 as [ds_d5T2 ds_d5T2_p].
+  destruct ds_d5T2 as [|].
   - refine (subsumptionCast
             Unit
             (λ (VV : Unit),
@@ -1070,30 +1119,30 @@ Proof.
 Defined.
 
 Definition andb_eq_orb_spec
-  (ds_d5S8 ds_d5S9 : SFBool)
-  (ds_d5Sa : {{∃ (andb_res : SFBool_u),
-               andb_rel ⌊ ds_d5S8 -⌋ ⌊ ds_d5S9 -⌋ andb_res
-               ∧ ∃ (orb_res : SFBool_u), orb_rel ⌊ ds_d5S8 -⌋ ⌊ ds_d5S9 -⌋ orb_res ∧ andb_res == orb_res}}):
+  (ds_d5ST ds_d5SU : SFBool)
+  (ds_d5SV : {{∃ (andb_res : SFBool_u),
+               andb_rel ⌊ ds_d5ST -⌋ ⌊ ds_d5SU -⌋ andb_res
+               ∧ ∃ (orb_res : SFBool_u), orb_rel ⌊ ds_d5ST -⌋ ⌊ ds_d5SU -⌋ orb_res ∧ andb_res == orb_res}}):
   Type :=
-  {{⌊ ds_d5S8 -⌋ == ⌊ ds_d5S9 -⌋}}.
+  {{⌊ ds_d5ST -⌋ == ⌊ ds_d5SU -⌋}}.
 
 #[global] Hint Unfold andb_eq_orb_spec: lia_unfold.
 
 Theorem andb_eq_orb
-  (ds_d5S8 ds_d5S9 : SFBool)
-  (ds_d5Sa : {{∃ (andb_res : SFBool_u),
-               andb_rel ⌊ ds_d5S8 -⌋ ⌊ ds_d5S9 -⌋ andb_res
-               ∧ ∃ (orb_res : SFBool_u), orb_rel ⌊ ds_d5S8 -⌋ ⌊ ds_d5S9 -⌋ orb_res ∧ andb_res == orb_res}}):
-  andb_eq_orb_spec ds_d5S8 ds_d5S9 ds_d5Sa.
+  (ds_d5ST ds_d5SU : SFBool)
+  (ds_d5SV : {{∃ (andb_res : SFBool_u),
+               andb_rel ⌊ ds_d5ST -⌋ ⌊ ds_d5SU -⌋ andb_res
+               ∧ ∃ (orb_res : SFBool_u), orb_rel ⌊ ds_d5ST -⌋ ⌊ ds_d5SU -⌋ orb_res ∧ andb_res == orb_res}}):
+  andb_eq_orb_spec ds_d5ST ds_d5SU ds_d5SV.
 Proof.
-  destruct ds_d5S8 as [ds_d5S8 ds_d5S8_p].
-  destruct ds_d5S9 as [ds_d5S9 ds_d5S9_p].
-  destruct ds_d5Sa as [ds_d5Sa ds_d5Sa_p].
-  destruct ds_d5S8 as [|].
-  - destruct ds_d5S9 as [|].
+  destruct ds_d5ST as [ds_d5ST ds_d5ST_p].
+  destruct ds_d5SU as [ds_d5SU ds_d5SU_p].
+  destruct ds_d5SV as [ds_d5SV ds_d5SV_p].
+  destruct ds_d5ST as [|].
+  - destruct ds_d5SU as [|].
     + refine (subsumptionCast Unit (λ (VV : Unit), SFFalse_u == SFFalse_u) (# unit) ltac:(solver)).
     + refine (subsumptionCast Unit (λ (VV : Unit), SFFalse_u == SFTrue_u) (# unit) ltac:(solver)).
-  - destruct ds_d5S9 as [|].
+  - destruct ds_d5SU as [|].
     + refine (subsumptionCast Unit (λ (VV : Unit), SFTrue_u == SFFalse_u) (# unit) ltac:(solver)).
     + refine (subsumptionCast Unit (λ (VV : Unit), SFTrue_u == SFTrue_u) (# unit) ltac:(solver)).
 Qed.
@@ -1341,15 +1390,15 @@ Defined.
 
 #[global] Hint Unfold SoftwareFoundations__Z: ref_constr_db.
 
-Definition bin_to_nat_spec (ds_d5Rl : SFBin): Type :=
+Definition bin_to_nat_spec (ds_d5S6 : SFBin): Type :=
   {VV: Z | True}.
 
 #[global] Hint Unfold bin_to_nat_spec: lia_unfold.
 
-Definition bin_to_nat (ds_d5Rl : SFBin): bin_to_nat_spec ds_d5Rl.
+Definition bin_to_nat (ds_d5S6 : SFBin): bin_to_nat_spec ds_d5S6.
 Proof.
-  destruct ds_d5Rl as [ds_d5Rl ds_d5Rl_p].
-  induction ds_d5Rl as [m' IH_m'| m' IH_m'|].
+  destruct ds_d5S6 as [ds_d5S6 ds_d5S6_p].
+  induction ds_d5S6 as [m' IH_m'| m' IH_m'|].
   - refine (subsumptionCast
             Z
             (λ (VV : Z), True)
@@ -1392,10 +1441,10 @@ Inductive bin_to_nat_rel: SFBin_u → Z → Prop :=
 
 #[global] Instance bin_to_nat_getF: getFunc bin_to_nat_rel := { getF' := bin_to_nat }.
 
-Theorem bin_to_nat_rel_funct [ds_d5Rl : SFBin_u]:
-  ∀ (VV VV' : Z), bin_to_nat_rel ds_d5Rl VV → (bin_to_nat_rel ds_d5Rl VV' → VV = VV').
+Theorem bin_to_nat_rel_funct [ds_d5S6 : SFBin_u]:
+  ∀ (VV VV' : Z), bin_to_nat_rel ds_d5S6 VV → (bin_to_nat_rel ds_d5S6 VV' → VV = VV').
 Proof.
-  induction ds_d5Rl as [m' IH_m'| m' IH_m'|]; rel_functionhood_body.
+  induction ds_d5S6 as [m' IH_m'| m' IH_m'|]; rel_functionhood_body.
 Qed.
 
 #[global] Hint Resolve bin_to_nat_rel_funct: f_rel_funct_db.
@@ -1436,12 +1485,12 @@ Qed.
 
 #[global] Hint Rewrite bin_to_nat_SoftwareFoundations__Z_lem: f_rel_back.
 
-Theorem bin_to_nat_rel_ex (ds_d5Rl : SFBin_u) (ds_d5Rl_p : SFBin_wf ds_d5Rl ∧ True):
-  bin_to_nat_rel ds_d5Rl ⌊ bin_to_nat (exist _ ds_d5Rl ds_d5Rl_p) -⌋.
+Theorem bin_to_nat_rel_ex (ds_d5S6 : SFBin_u) (ds_d5S6_p : SFBin_wf ds_d5S6 ∧ True):
+  bin_to_nat_rel ds_d5S6 ⌊ bin_to_nat (exist _ ds_d5S6 ds_d5S6_p) -⌋.
 Proof.
   Opaque bin_to_nat.
   existence_lemma_pre bin_to_nat;
-  induction ds_d5Rl as [m' IH_m'| m' IH_m'|];
+  induction ds_d5S6 as [m' IH_m'| m' IH_m'|];
   [fix_notations; pose proof (IH_m' ltac:(try clear IH_m'; solver)) as IH_34714780; try clear IH_m' |
    fix_notations; pose proof (IH_m' ltac:(try clear IH_m'; solver)) as IH_34714780; try clear IH_m' |
    fix_notations];
@@ -1455,8 +1504,8 @@ Qed.
 #[global] Opaque bin_to_nat.
 
 Theorem bin_to_nat__bin_to_nat_rel_rw
-  (ds_d5Rl : SFBin_u) (ds_d5Rl_p : SFBin_wf ds_d5Rl ∧ True) (VV : Z):
-  ⌊ bin_to_nat (exist _ ds_d5Rl ds_d5Rl_p) -⌋ = VV ↔ bin_to_nat_rel ds_d5Rl VV.
+  (ds_d5S6 : SFBin_u) (ds_d5S6_p : SFBin_wf ds_d5S6 ∧ True) (VV : Z):
+  ⌊ bin_to_nat (exist _ ds_d5S6 ds_d5S6_p) -⌋ = VV ↔ bin_to_nat_rel ds_d5S6 VV.
 Proof.
   f__f_rel_rw.
 Qed.
@@ -1468,30 +1517,30 @@ Qed.
 #[global] Instance bin_to_nat_lookup_rw: dictionary rwLem bin_to_nat := {
     lookup' := bin_to_nat__bin_to_nat_rel_rw }.
 
-Theorem bin_to_nat__bin_to_nat_rel (ds_d5Rl : SFBin) (VV : Z):
-  ⌊ bin_to_nat ds_d5Rl -⌋ = VV ↔ bin_to_nat_rel ⌊ ds_d5Rl ⌋ VV.
+Theorem bin_to_nat__bin_to_nat_rel (ds_d5S6 : SFBin) (VV : Z):
+  ⌊ bin_to_nat ds_d5S6 -⌋ = VV ↔ bin_to_nat_rel ⌊ ds_d5S6 ⌋ VV.
 Proof.
   f__f_rel.
 Qed.
 
 #[global] Hint Rewrite bin_to_nat__bin_to_nat_rel: f_rel_funct_db.
 
-Theorem bin_to_nat__bin_to_nat_rel' (ds_d5Rl_u : SFBin_u) (ds_d5Rl : SFBin) (VV : Z):
-  ds_d5Rl_u = ⌊ ds_d5Rl ⌋ → ⌊ bin_to_nat ds_d5Rl -⌋ = VV ↔ bin_to_nat_rel ds_d5Rl_u VV.
+Theorem bin_to_nat__bin_to_nat_rel' (ds_d5S6_u : SFBin_u) (ds_d5S6 : SFBin) (VV : Z):
+  ds_d5S6_u = ⌊ ds_d5S6 ⌋ → ⌊ bin_to_nat ds_d5S6 -⌋ = VV ↔ bin_to_nat_rel ds_d5S6_u VV.
 Proof.
-  intros ->. refine (bin_to_nat__bin_to_nat_rel ds_d5Rl VV).
+  intros ->. refine (bin_to_nat__bin_to_nat_rel ds_d5S6 VV).
 Qed.
 
 #[global] Hint Resolve bin_to_nat__bin_to_nat_rel': f_rel_funct_db.
 
-Theorem bin_to_nat_rel_mk (ds_d5Rl : SFBin_u) (ds_d5Rl_p : SFBin_wf ds_d5Rl ∧ True):
-  {VV: _ | bin_to_nat_rel ds_d5Rl VV}.
+Theorem bin_to_nat_rel_mk (ds_d5S6 : SFBin_u) (ds_d5S6_p : SFBin_wf ds_d5S6 ∧ True):
+  {VV: _ | bin_to_nat_rel ds_d5S6 VV}.
 Proof.
   intros;
   refine (subsumptionCast
           _
-          (λ VV, bin_to_nat_rel ds_d5Rl VV)
-          (bin_to_nat (exist _ ds_d5Rl ds_d5Rl_p))
+          (λ VV, bin_to_nat_rel ds_d5S6 VV)
+          (bin_to_nat (exist _ ds_d5S6 ds_d5S6_p))
           _);
   rewrite <- bin_to_nat__bin_to_nat_rel';
   quicksolve.
@@ -1501,12 +1550,12 @@ Qed.
 
 #[global] Instance bin_to_nat_pack:
   @Pack
-  (SFBin ::RT λ (ds_d5Rl : SFBin), nilRT)
+  (SFBin ::RT λ (ds_d5S6 : SFBin), nilRT)
   (SFBin_u ::UT nilUT)
-  ltac:(mkProjectsArgListTG (SFBin ::RT λ (ds_d5Rl : SFBin), nilRT) ((SFBin_u ::UT nilUT)))
+  ltac:(mkProjectsArgListTG (SFBin ::RT λ (ds_d5S6 : SFBin), nilRT) ((SFBin_u ::UT nilUT)))
   Z
-  (λ (x_88016881 : ArgList (SFBin ::RT λ (ds_d5Rl : SFBin), nilRT)) (v_x_88016881 : Z),
-   ltac:(flattenP (λ (ds_d5Rl : SFBin) (VV : Z), True) x_88016881 v_x_88016881)).
+  (λ (x_32298126 : ArgList (SFBin ::RT λ (ds_d5S6 : SFBin), nilRT)) (v_x_32298126 : Z),
+   ltac:(flattenP (λ (ds_d5S6 : SFBin) (VV : Z), True) x_32298126 v_x_32298126)).
 Proof.
   buildPackG bin_to_nat bin_to_nat_rel bin_to_nat__bin_to_nat_rel bin_to_nat_rel_funct.
 Defined.
@@ -1533,15 +1582,15 @@ Proof.
           ltac:(solver)).
 Qed.
 
-Definition incr_spec (ds_d5Rm : SFBin): Type :=
+Definition incr_spec (ds_d5S7 : SFBin): Type :=
   SFBin.
 
 #[global] Hint Unfold incr_spec: lia_unfold.
 
-Definition incr (ds_d5Rm : SFBin): incr_spec ds_d5Rm.
+Definition incr (ds_d5S7 : SFBin): incr_spec ds_d5S7.
 Proof.
-  destruct ds_d5Rm as [ds_d5Rm ds_d5Rm_p].
-  induction ds_d5Rm as [m' _| m' IH_m'|].
+  destruct ds_d5S7 as [ds_d5S7 ds_d5S7_p].
+  induction ds_d5S7 as [m' _| m' IH_m'|].
   - refine (Bin1 (exist (λ (n : SFBin_u), SFBin_wf n ∧ True) m' ltac:(solver))).
   - refine (Bin0 (IH_m' ltac:(try clear IH_m'; solver))).
   - refine (Bin1 SoftwareFoundations__Z).
@@ -1559,10 +1608,10 @@ Inductive incr_rel: SFBin_u → SFBin_u → Prop :=
 
 #[global] Instance incr_getF: getFunc incr_rel := { getF' := incr }.
 
-Theorem incr_rel_funct [ds_d5Rm : SFBin_u]:
-  ∀ (VV VV' : SFBin_u), incr_rel ds_d5Rm VV → (incr_rel ds_d5Rm VV' → VV = VV').
+Theorem incr_rel_funct [ds_d5S7 : SFBin_u]:
+  ∀ (VV VV' : SFBin_u), incr_rel ds_d5S7 VV → (incr_rel ds_d5S7 VV' → VV = VV').
 Proof.
-  induction ds_d5Rm as [m' _| m' IH_m'|]; rel_functionhood_body.
+  induction ds_d5S7 as [m' _| m' IH_m'|]; rel_functionhood_body.
 Qed.
 
 #[global] Hint Resolve incr_rel_funct: f_rel_funct_db.
@@ -1596,12 +1645,12 @@ Qed.
 
 #[global] Hint Rewrite incr_SoftwareFoundations__Z_lem: f_rel_back.
 
-Theorem incr_rel_ex (ds_d5Rm : SFBin_u) (ds_d5Rm_p : SFBin_wf ds_d5Rm ∧ True):
-  incr_rel ds_d5Rm ⌊ incr (exist _ ds_d5Rm ds_d5Rm_p) -⌋.
+Theorem incr_rel_ex (ds_d5S7 : SFBin_u) (ds_d5S7_p : SFBin_wf ds_d5S7 ∧ True):
+  incr_rel ds_d5S7 ⌊ incr (exist _ ds_d5S7 ds_d5S7_p) -⌋.
 Proof.
   Opaque incr.
   existence_lemma_pre incr;
-  induction ds_d5Rm as [m' _| m' IH_m'|];
+  induction ds_d5S7 as [m' _| m' IH_m'|];
   [fix_notations |
    fix_notations; pose proof (IH_m' ltac:(try clear IH_m'; solver)) as IH_34714780; try clear IH_m' |
    fix_notations];
@@ -1614,8 +1663,8 @@ Qed.
 
 #[global] Opaque incr.
 
-Theorem incr__incr_rel_rw (ds_d5Rm : SFBin_u) (ds_d5Rm_p : SFBin_wf ds_d5Rm ∧ True) (VV : SFBin_u):
-  ⌊ incr (exist _ ds_d5Rm ds_d5Rm_p) -⌋ = VV ↔ incr_rel ds_d5Rm VV.
+Theorem incr__incr_rel_rw (ds_d5S7 : SFBin_u) (ds_d5S7_p : SFBin_wf ds_d5S7 ∧ True) (VV : SFBin_u):
+  ⌊ incr (exist _ ds_d5S7 ds_d5S7_p) -⌋ = VV ↔ incr_rel ds_d5S7 VV.
 Proof.
   f__f_rel_rw.
 Qed.
@@ -1626,27 +1675,27 @@ Qed.
 
 #[global] Instance incr_lookup_rw: dictionary rwLem incr := { lookup' := incr__incr_rel_rw }.
 
-Theorem incr__incr_rel (ds_d5Rm : SFBin) (VV : SFBin_u):
-  ⌊ incr ds_d5Rm -⌋ = VV ↔ incr_rel ⌊ ds_d5Rm ⌋ VV.
+Theorem incr__incr_rel (ds_d5S7 : SFBin) (VV : SFBin_u):
+  ⌊ incr ds_d5S7 -⌋ = VV ↔ incr_rel ⌊ ds_d5S7 ⌋ VV.
 Proof.
   f__f_rel.
 Qed.
 
 #[global] Hint Rewrite incr__incr_rel: f_rel_funct_db.
 
-Theorem incr__incr_rel' (ds_d5Rm_u : SFBin_u) (ds_d5Rm : SFBin) (VV : SFBin_u):
-  ds_d5Rm_u = ⌊ ds_d5Rm ⌋ → ⌊ incr ds_d5Rm -⌋ = VV ↔ incr_rel ds_d5Rm_u VV.
+Theorem incr__incr_rel' (ds_d5S7_u : SFBin_u) (ds_d5S7 : SFBin) (VV : SFBin_u):
+  ds_d5S7_u = ⌊ ds_d5S7 ⌋ → ⌊ incr ds_d5S7 -⌋ = VV ↔ incr_rel ds_d5S7_u VV.
 Proof.
-  intros ->. refine (incr__incr_rel ds_d5Rm VV).
+  intros ->. refine (incr__incr_rel ds_d5S7 VV).
 Qed.
 
 #[global] Hint Resolve incr__incr_rel': f_rel_funct_db.
 
-Theorem incr_rel_mk (ds_d5Rm : SFBin_u) (ds_d5Rm_p : SFBin_wf ds_d5Rm ∧ True):
-  {VV: _ | incr_rel ds_d5Rm VV}.
+Theorem incr_rel_mk (ds_d5S7 : SFBin_u) (ds_d5S7_p : SFBin_wf ds_d5S7 ∧ True):
+  {VV: _ | incr_rel ds_d5S7 VV}.
 Proof.
   intros;
-  refine (subsumptionCast _ (λ VV, incr_rel ds_d5Rm VV) (incr (exist _ ds_d5Rm ds_d5Rm_p)) _);
+  refine (subsumptionCast _ (λ VV, incr_rel ds_d5S7 VV) (incr (exist _ ds_d5S7 ds_d5S7_p)) _);
   rewrite <- incr__incr_rel';
   quicksolve.
 Qed.
@@ -1655,12 +1704,12 @@ Qed.
 
 #[global] Instance incr_pack:
   @Pack
-  (SFBin ::RT λ (ds_d5Rm : SFBin), nilRT)
+  (SFBin ::RT λ (ds_d5S7 : SFBin), nilRT)
   (SFBin_u ::UT nilUT)
-  ltac:(mkProjectsArgListTG (SFBin ::RT λ (ds_d5Rm : SFBin), nilRT) ((SFBin_u ::UT nilUT)))
+  ltac:(mkProjectsArgListTG (SFBin ::RT λ (ds_d5S7 : SFBin), nilRT) ((SFBin_u ::UT nilUT)))
   SFBin_u
-  (λ (x_54307901 : ArgList (SFBin ::RT λ (ds_d5Rm : SFBin), nilRT)) (v_x_54307901 : SFBin_u),
-   ltac:(flattenP (λ (ds_d5Rm : SFBin) (VV : SFBin_u), SFBin_wf VV ∧ True) x_54307901 v_x_54307901)).
+  (λ (x_87102322 : ArgList (SFBin ::RT λ (ds_d5S7 : SFBin), nilRT)) (v_x_87102322 : SFBin_u),
+   ltac:(flattenP (λ (ds_d5S7 : SFBin) (VV : SFBin_u), SFBin_wf VV ∧ True) x_87102322 v_x_87102322)).
 Proof.
   buildPackG incr incr_rel incr__incr_rel incr_rel_funct.
 Defined.
@@ -2028,19 +2077,19 @@ Defined.
 
 #[global] Hint Unfold Bits: ref_constr_db.
 
-Definition allzero_spec (ds_d5T0 : Nibble): Type :=
+Definition allzero_spec (ds_d5TL : Nibble): Type :=
   SFBool.
 
 #[global] Hint Unfold allzero_spec: lia_unfold.
 
-Definition allzero (ds_d5T0 : Nibble): allzero_spec ds_d5T0.
+Definition allzero (ds_d5TL : Nibble): allzero_spec ds_d5TL.
 Proof.
-  destruct ds_d5T0 as [ds_d5T0 ds_d5T0_p].
-  destruct ds_d5T0 as [ds_d5T1 ds_d5T2 ds_d5T3 ds_d5T4].
-  - destruct ds_d5T1 as [|].
-    + destruct ds_d5T2 as [|].
-      * destruct ds_d5T3 as [|].
-        -- destruct ds_d5T4 as [|].
+  destruct ds_d5TL as [ds_d5TL ds_d5TL_p].
+  destruct ds_d5TL as [ds_d5TM ds_d5TN ds_d5TO ds_d5TP].
+  - destruct ds_d5TM as [|].
+    + destruct ds_d5TN as [|].
+      * destruct ds_d5TO as [|].
+        -- destruct ds_d5TP as [|].
            ++ refine SFTrue.
            ++ refine SFFalse.
         -- refine SFFalse.
@@ -2186,15 +2235,15 @@ Defined.
 
 #[global] Hint Unfold Pair: ref_constr_db.
 
-Definition swap_pair_spec (ds_d5Rb : Natprod): Type :=
+Definition swap_pair_spec (ds_d5RW : Natprod): Type :=
   Natprod.
 
 #[global] Hint Unfold swap_pair_spec: lia_unfold.
 
-Definition swap_pair (ds_d5Rb : Natprod): swap_pair_spec ds_d5Rb.
+Definition swap_pair (ds_d5RW : Natprod): swap_pair_spec ds_d5RW.
 Proof.
-  destruct ds_d5Rb as [ds_d5Rb ds_d5Rb_p].
-  destruct ds_d5Rb as [x y].
+  destruct ds_d5RW as [ds_d5RW ds_d5RW_p].
+  destruct ds_d5RW as [x y].
   - refine (Pair
             (exist (λ (n2 : MyNat_u), MyNat_wf n2 ∧ True) y ltac:(solver))
             (exist (λ (n1 : MyNat_u), MyNat_wf n1 ∧ True) x ltac:(solver))).
@@ -2209,10 +2258,10 @@ Inductive swap_pair_rel: Natprod_u → Natprod_u → Prop :=
 
 #[global] Instance swap_pair_getF: getFunc swap_pair_rel := { getF' := swap_pair }.
 
-Theorem swap_pair_rel_funct [ds_d5Rb : Natprod_u]:
-  ∀ (VV VV' : Natprod_u), swap_pair_rel ds_d5Rb VV → (swap_pair_rel ds_d5Rb VV' → VV = VV').
+Theorem swap_pair_rel_funct [ds_d5RW : Natprod_u]:
+  ∀ (VV VV' : Natprod_u), swap_pair_rel ds_d5RW VV → (swap_pair_rel ds_d5RW VV' → VV = VV').
 Proof.
-  destruct ds_d5Rb as [x y]; rel_functionhood_body.
+  destruct ds_d5RW as [x y]; rel_functionhood_body.
 Qed.
 
 #[global] Hint Resolve swap_pair_rel_funct: f_rel_funct_db.
@@ -2228,12 +2277,12 @@ Qed.
 
 #[global] Hint Rewrite swap_pair_Pair_lem: f_rel_back.
 
-Theorem swap_pair_rel_ex (ds_d5Rb : Natprod_u) (ds_d5Rb_p : Natprod_wf ds_d5Rb ∧ True):
-  swap_pair_rel ds_d5Rb ⌊ swap_pair (exist _ ds_d5Rb ds_d5Rb_p) -⌋.
+Theorem swap_pair_rel_ex (ds_d5RW : Natprod_u) (ds_d5RW_p : Natprod_wf ds_d5RW ∧ True):
+  swap_pair_rel ds_d5RW ⌊ swap_pair (exist _ ds_d5RW ds_d5RW_p) -⌋.
 Proof.
   Opaque swap_pair.
   existence_lemma_pre swap_pair;
-  destruct ds_d5Rb as [x y];
+  destruct ds_d5RW as [x y];
   [fix_notations];
   simpl in *.
   Transparent swap_pair.
@@ -2245,8 +2294,8 @@ Qed.
 #[global] Opaque swap_pair.
 
 Theorem swap_pair__swap_pair_rel_rw
-  (ds_d5Rb : Natprod_u) (ds_d5Rb_p : Natprod_wf ds_d5Rb ∧ True) (VV : Natprod_u):
-  ⌊ swap_pair (exist _ ds_d5Rb ds_d5Rb_p) -⌋ = VV ↔ swap_pair_rel ds_d5Rb VV.
+  (ds_d5RW : Natprod_u) (ds_d5RW_p : Natprod_wf ds_d5RW ∧ True) (VV : Natprod_u):
+  ⌊ swap_pair (exist _ ds_d5RW ds_d5RW_p) -⌋ = VV ↔ swap_pair_rel ds_d5RW VV.
 Proof.
   f__f_rel_rw.
 Qed.
@@ -2258,30 +2307,30 @@ Qed.
 #[global] Instance swap_pair_lookup_rw: dictionary rwLem swap_pair := {
     lookup' := swap_pair__swap_pair_rel_rw }.
 
-Theorem swap_pair__swap_pair_rel (ds_d5Rb : Natprod) (VV : Natprod_u):
-  ⌊ swap_pair ds_d5Rb -⌋ = VV ↔ swap_pair_rel ⌊ ds_d5Rb ⌋ VV.
+Theorem swap_pair__swap_pair_rel (ds_d5RW : Natprod) (VV : Natprod_u):
+  ⌊ swap_pair ds_d5RW -⌋ = VV ↔ swap_pair_rel ⌊ ds_d5RW ⌋ VV.
 Proof.
   f__f_rel.
 Qed.
 
 #[global] Hint Rewrite swap_pair__swap_pair_rel: f_rel_funct_db.
 
-Theorem swap_pair__swap_pair_rel' (ds_d5Rb_u : Natprod_u) (ds_d5Rb : Natprod) (VV : Natprod_u):
-  ds_d5Rb_u = ⌊ ds_d5Rb ⌋ → ⌊ swap_pair ds_d5Rb -⌋ = VV ↔ swap_pair_rel ds_d5Rb_u VV.
+Theorem swap_pair__swap_pair_rel' (ds_d5RW_u : Natprod_u) (ds_d5RW : Natprod) (VV : Natprod_u):
+  ds_d5RW_u = ⌊ ds_d5RW ⌋ → ⌊ swap_pair ds_d5RW -⌋ = VV ↔ swap_pair_rel ds_d5RW_u VV.
 Proof.
-  intros ->. refine (swap_pair__swap_pair_rel ds_d5Rb VV).
+  intros ->. refine (swap_pair__swap_pair_rel ds_d5RW VV).
 Qed.
 
 #[global] Hint Resolve swap_pair__swap_pair_rel': f_rel_funct_db.
 
-Theorem swap_pair_rel_mk (ds_d5Rb : Natprod_u) (ds_d5Rb_p : Natprod_wf ds_d5Rb ∧ True):
-  {VV: _ | swap_pair_rel ds_d5Rb VV}.
+Theorem swap_pair_rel_mk (ds_d5RW : Natprod_u) (ds_d5RW_p : Natprod_wf ds_d5RW ∧ True):
+  {VV: _ | swap_pair_rel ds_d5RW VV}.
 Proof.
   intros;
   refine (subsumptionCast
           _
-          (λ VV, swap_pair_rel ds_d5Rb VV)
-          (swap_pair (exist _ ds_d5Rb ds_d5Rb_p))
+          (λ VV, swap_pair_rel ds_d5RW VV)
+          (swap_pair (exist _ ds_d5RW ds_d5RW_p))
           _);
   rewrite <- swap_pair__swap_pair_rel';
   quicksolve.
@@ -2291,12 +2340,12 @@ Qed.
 
 #[global] Instance swap_pair_pack:
   @Pack
-  (Natprod ::RT λ (ds_d5Rb : Natprod), nilRT)
+  (Natprod ::RT λ (ds_d5RW : Natprod), nilRT)
   (Natprod_u ::UT nilUT)
-  ltac:(mkProjectsArgListTG (Natprod ::RT λ (ds_d5Rb : Natprod), nilRT) ((Natprod_u ::UT nilUT)))
+  ltac:(mkProjectsArgListTG (Natprod ::RT λ (ds_d5RW : Natprod), nilRT) ((Natprod_u ::UT nilUT)))
   Natprod_u
-  (λ (x_65858049 : ArgList (Natprod ::RT λ (ds_d5Rb : Natprod), nilRT)) (v_x_65858049 : Natprod_u),
-   ltac:(flattenP (λ (ds_d5Rb : Natprod) (VV : Natprod_u), Natprod_wf VV ∧ True) x_65858049 v_x_65858049)).
+  (λ (x_80277571 : ArgList (Natprod ::RT λ (ds_d5RW : Natprod), nilRT)) (v_x_80277571 : Natprod_u),
+   ltac:(flattenP (λ (ds_d5RW : Natprod) (VV : Natprod_u), Natprod_wf VV ∧ True) x_80277571 v_x_80277571)).
 Proof.
   buildPackG swap_pair swap_pair_rel swap_pair__swap_pair_rel swap_pair_rel_funct.
 Defined.
@@ -2306,20 +2355,20 @@ Proof.
   buildUPackG swap_pair_rel swap_pair_rel_funct.
 Defined.
 
-Definition eqb_spec (ds_d5Su ds_d5Sv : MyNat): Type :=
+Definition eqb_spec (ds_d5Tf ds_d5Tg : MyNat): Type :=
   SFBool.
 
 #[global] Hint Unfold eqb_spec: lia_unfold.
 
-Definition eqb (ds_d5Su ds_d5Sv : MyNat): eqb_spec ds_d5Su ds_d5Sv.
+Definition eqb (ds_d5Tf ds_d5Tg : MyNat): eqb_spec ds_d5Tf ds_d5Tg.
 Proof.
-  destruct ds_d5Su as [ds_d5Su ds_d5Su_p].
-  destruct ds_d5Sv as [ds_d5Sv ds_d5Sv_p].
-  try revert ds_d5Sv_p; generalize dependent ds_d5Sv; induction ds_d5Su as [| n' IH_n']; intros.
-  - destruct ds_d5Sv as [| m'].
+  destruct ds_d5Tf as [ds_d5Tf ds_d5Tf_p].
+  destruct ds_d5Tg as [ds_d5Tg ds_d5Tg_p].
+  try revert ds_d5Tg_p; generalize dependent ds_d5Tg; induction ds_d5Tf as [| n' IH_n']; intros.
+  - destruct ds_d5Tg as [| m'].
     + refine SFTrue.
     + refine SFFalse.
-  - destruct ds_d5Sv as [| m'].
+  - destruct ds_d5Tg as [| m'].
     + refine SFFalse.
     + refine (IH_n' ltac:(try clear IH_n'; solver) m' ltac:(try clear IH_n'; solver)).
 Defined.
@@ -2336,11 +2385,11 @@ Inductive eqb_rel: MyNat_u → MyNat_u → SFBool_u → Prop :=
 
 #[global] Instance eqb_getF: getFunc eqb_rel := { getF' := eqb }.
 
-Theorem eqb_rel_funct [ds_d5Su ds_d5Sv : MyNat_u]:
-  ∀ (VV VV' : SFBool_u), eqb_rel ds_d5Su ds_d5Sv VV → (eqb_rel ds_d5Su ds_d5Sv VV' → VV = VV').
+Theorem eqb_rel_funct [ds_d5Tf ds_d5Tg : MyNat_u]:
+  ∀ (VV VV' : SFBool_u), eqb_rel ds_d5Tf ds_d5Tg VV → (eqb_rel ds_d5Tf ds_d5Tg VV' → VV = VV').
 Proof.
-  try revert ds_d5Sv_p; generalize dependent ds_d5Sv; induction ds_d5Su as [| n' IH_n']; intros;
-  [destruct ds_d5Sv as [| m'] | destruct ds_d5Sv as [| m']];
+  try revert ds_d5Tg_p; generalize dependent ds_d5Tg; induction ds_d5Tf as [| n' IH_n']; intros;
+  [destruct ds_d5Tg as [| m'] | destruct ds_d5Tg as [| m']];
   rel_functionhood_body.
 Qed.
 
@@ -2381,18 +2430,18 @@ Qed.
 #[global] Hint Rewrite eqb_S_S_lem: f_rel_back.
 
 Theorem eqb_rel_ex
-  (ds_d5Su : MyNat_u)
-  (ds_d5Su_p : MyNat_wf ds_d5Su ∧ True)
-  (ds_d5Sv : MyNat_u)
-  (ds_d5Sv_p : MyNat_wf ds_d5Sv ∧ True):
-  eqb_rel ds_d5Su ds_d5Sv ⌊ eqb (exist _ ds_d5Su ds_d5Su_p) (exist _ ds_d5Sv ds_d5Sv_p) -⌋.
+  (ds_d5Tf : MyNat_u)
+  (ds_d5Tf_p : MyNat_wf ds_d5Tf ∧ True)
+  (ds_d5Tg : MyNat_u)
+  (ds_d5Tg_p : MyNat_wf ds_d5Tg ∧ True):
+  eqb_rel ds_d5Tf ds_d5Tg ⌊ eqb (exist _ ds_d5Tf ds_d5Tf_p) (exist _ ds_d5Tg ds_d5Tg_p) -⌋.
 Proof.
   Opaque eqb.
   existence_lemma_pre eqb;
-  try revert ds_d5Sv_p; generalize dependent ds_d5Sv; induction ds_d5Su as [| n' IH_n']; intros;
-  [destruct ds_d5Sv as [| m'];
+  try revert ds_d5Tg_p; generalize dependent ds_d5Tg; induction ds_d5Tf as [| n' IH_n']; intros;
+  [destruct ds_d5Tg as [| m'];
    [fix_notations | fix_notations] |
-   destruct ds_d5Sv as [| m'];
+   destruct ds_d5Tg as [| m'];
    [fix_notations |
     fix_notations;
     pose proof (IH_n' ltac:(try clear IH_n'; solver) m' ltac:(try clear IH_n'; solver)) as IH_11391185;
@@ -2407,12 +2456,12 @@ Qed.
 #[global] Opaque eqb.
 
 Theorem eqb__eqb_rel_rw
-  (ds_d5Su : MyNat_u)
-  (ds_d5Su_p : MyNat_wf ds_d5Su ∧ True)
-  (ds_d5Sv : MyNat_u)
-  (ds_d5Sv_p : MyNat_wf ds_d5Sv ∧ True)
+  (ds_d5Tf : MyNat_u)
+  (ds_d5Tf_p : MyNat_wf ds_d5Tf ∧ True)
+  (ds_d5Tg : MyNat_u)
+  (ds_d5Tg_p : MyNat_wf ds_d5Tg ∧ True)
   (VV : SFBool_u):
-  ⌊ eqb (exist _ ds_d5Su ds_d5Su_p) (exist _ ds_d5Sv ds_d5Sv_p) -⌋ = VV ↔ eqb_rel ds_d5Su ds_d5Sv VV.
+  ⌊ eqb (exist _ ds_d5Tf ds_d5Tf_p) (exist _ ds_d5Tg ds_d5Tg_p) -⌋ = VV ↔ eqb_rel ds_d5Tf ds_d5Tg VV.
 Proof.
   f__f_rel_rw.
 Qed.
@@ -2423,35 +2472,35 @@ Qed.
 
 #[global] Instance eqb_lookup_rw: dictionary rwLem eqb := { lookup' := eqb__eqb_rel_rw }.
 
-Theorem eqb__eqb_rel (ds_d5Su ds_d5Sv : MyNat) (VV : SFBool_u):
-  ⌊ eqb ds_d5Su ds_d5Sv -⌋ = VV ↔ eqb_rel ⌊ ds_d5Su ⌋ ⌊ ds_d5Sv ⌋ VV.
+Theorem eqb__eqb_rel (ds_d5Tf ds_d5Tg : MyNat) (VV : SFBool_u):
+  ⌊ eqb ds_d5Tf ds_d5Tg -⌋ = VV ↔ eqb_rel ⌊ ds_d5Tf ⌋ ⌊ ds_d5Tg ⌋ VV.
 Proof.
   f__f_rel.
 Qed.
 
 #[global] Hint Rewrite eqb__eqb_rel: f_rel_funct_db.
 
-Theorem eqb__eqb_rel' (ds_d5Su_u ds_d5Sv_u : MyNat_u) (ds_d5Su ds_d5Sv : MyNat) (VV : SFBool_u):
-  ds_d5Su_u = ⌊ ds_d5Su ⌋
-  → (ds_d5Sv_u = ⌊ ds_d5Sv ⌋ → ⌊ eqb ds_d5Su ds_d5Sv -⌋ = VV ↔ eqb_rel ds_d5Su_u ds_d5Sv_u VV).
+Theorem eqb__eqb_rel' (ds_d5Tf_u ds_d5Tg_u : MyNat_u) (ds_d5Tf ds_d5Tg : MyNat) (VV : SFBool_u):
+  ds_d5Tf_u = ⌊ ds_d5Tf ⌋
+  → (ds_d5Tg_u = ⌊ ds_d5Tg ⌋ → ⌊ eqb ds_d5Tf ds_d5Tg -⌋ = VV ↔ eqb_rel ds_d5Tf_u ds_d5Tg_u VV).
 Proof.
-  intros -> ->. refine (eqb__eqb_rel ds_d5Su ds_d5Sv VV).
+  intros -> ->. refine (eqb__eqb_rel ds_d5Tf ds_d5Tg VV).
 Qed.
 
 #[global] Hint Resolve eqb__eqb_rel': f_rel_funct_db.
 
 Theorem eqb_rel_mk
-  (ds_d5Su : MyNat_u)
-  (ds_d5Su_p : MyNat_wf ds_d5Su ∧ True)
-  (ds_d5Sv : MyNat_u)
-  (ds_d5Sv_p : MyNat_wf ds_d5Sv ∧ True):
-  {VV: _ | eqb_rel ds_d5Su ds_d5Sv VV}.
+  (ds_d5Tf : MyNat_u)
+  (ds_d5Tf_p : MyNat_wf ds_d5Tf ∧ True)
+  (ds_d5Tg : MyNat_u)
+  (ds_d5Tg_p : MyNat_wf ds_d5Tg ∧ True):
+  {VV: _ | eqb_rel ds_d5Tf ds_d5Tg VV}.
 Proof.
   intros;
   refine (subsumptionCast
           _
-          (λ VV, eqb_rel ds_d5Su ds_d5Sv VV)
-          (eqb (exist _ ds_d5Su ds_d5Su_p) (exist _ ds_d5Sv ds_d5Sv_p))
+          (λ VV, eqb_rel ds_d5Tf ds_d5Tg VV)
+          (eqb (exist _ ds_d5Tf ds_d5Tf_p) (exist _ ds_d5Tg ds_d5Tg_p))
           _);
   rewrite <- eqb__eqb_rel';
   quicksolve.
@@ -2461,14 +2510,14 @@ Qed.
 
 #[global] Instance eqb_pack:
   @Pack
-  (MyNat ::RT λ (ds_d5Su : MyNat), MyNat ::RT λ (ds_d5Sv : MyNat), nilRT)
+  (MyNat ::RT λ (ds_d5Tf : MyNat), MyNat ::RT λ (ds_d5Tg : MyNat), nilRT)
   (MyNat_u ::UT (MyNat_u ::UT nilUT))
   ltac:(mkProjectsArgListTG (MyNat
- ::RT λ (ds_d5Su : MyNat), MyNat ::RT λ (ds_d5Sv : MyNat), nilRT) ((MyNat_u ::UT (MyNat_u ::UT nilUT))))
+ ::RT λ (ds_d5Tf : MyNat), MyNat ::RT λ (ds_d5Tg : MyNat), nilRT) ((MyNat_u ::UT (MyNat_u ::UT nilUT))))
   SFBool_u
-  (λ (x_12059133 : ArgList (MyNat ::RT λ (ds_d5Su : MyNat), MyNat ::RT λ (ds_d5Sv : MyNat), nilRT))
-     (v_x_12059133 : SFBool_u),
-   ltac:(flattenP (λ (ds_d5Su ds_d5Sv : MyNat) (VV : SFBool_u), SFBool_wf VV ∧ True) x_12059133 v_x_12059133)).
+  (λ (x_58187509 : ArgList (MyNat ::RT λ (ds_d5Tf : MyNat), MyNat ::RT λ (ds_d5Tg : MyNat), nilRT))
+     (v_x_58187509 : SFBool_u),
+   ltac:(flattenP (λ (ds_d5Tf ds_d5Tg : MyNat) (VV : SFBool_u), SFBool_wf VV ∧ True) x_58187509 v_x_58187509)).
 Proof.
   buildPackG eqb eqb_rel eqb__eqb_rel eqb_rel_funct.
 Defined.
@@ -2478,15 +2527,15 @@ Proof.
   buildUPackG eqb_rel eqb_rel_funct.
 Defined.
 
-Definition fstSF_spec (ds_d5Rf : Natprod): Type :=
+Definition fstSF_spec (ds_d5S0 : Natprod): Type :=
   MyNat.
 
 #[global] Hint Unfold fstSF_spec: lia_unfold.
 
-Definition fstSF (ds_d5Rf : Natprod): fstSF_spec ds_d5Rf.
+Definition fstSF (ds_d5S0 : Natprod): fstSF_spec ds_d5S0.
 Proof.
-  destruct ds_d5Rf as [ds_d5Rf ds_d5Rf_p].
-  destruct ds_d5Rf as [n1 n2].
+  destruct ds_d5S0 as [ds_d5S0 ds_d5S0_p].
+  destruct ds_d5S0 as [n1 n2].
   - refine (exist (λ (n1 : MyNat_u), MyNat_wf n1 ∧ True) n1 ltac:(solver)).
 Defined.
 
@@ -2499,10 +2548,10 @@ Inductive fstSF_rel: Natprod_u → MyNat_u → Prop :=
 
 #[global] Instance fstSF_getF: getFunc fstSF_rel := { getF' := fstSF }.
 
-Theorem fstSF_rel_funct [ds_d5Rf : Natprod_u]:
-  ∀ (VV VV' : MyNat_u), fstSF_rel ds_d5Rf VV → (fstSF_rel ds_d5Rf VV' → VV = VV').
+Theorem fstSF_rel_funct [ds_d5S0 : Natprod_u]:
+  ∀ (VV VV' : MyNat_u), fstSF_rel ds_d5S0 VV → (fstSF_rel ds_d5S0 VV' → VV = VV').
 Proof.
-  destruct ds_d5Rf as [n1 n2]; rel_functionhood_body.
+  destruct ds_d5S0 as [n1 n2]; rel_functionhood_body.
 Qed.
 
 #[global] Hint Resolve fstSF_rel_funct: f_rel_funct_db.
@@ -2518,12 +2567,12 @@ Qed.
 
 #[global] Hint Rewrite fstSF_Pair_lem: f_rel_back.
 
-Theorem fstSF_rel_ex (ds_d5Rf : Natprod_u) (ds_d5Rf_p : Natprod_wf ds_d5Rf ∧ True):
-  fstSF_rel ds_d5Rf ⌊ fstSF (exist _ ds_d5Rf ds_d5Rf_p) -⌋.
+Theorem fstSF_rel_ex (ds_d5S0 : Natprod_u) (ds_d5S0_p : Natprod_wf ds_d5S0 ∧ True):
+  fstSF_rel ds_d5S0 ⌊ fstSF (exist _ ds_d5S0 ds_d5S0_p) -⌋.
 Proof.
   Opaque fstSF.
   existence_lemma_pre fstSF;
-  destruct ds_d5Rf as [n1 n2];
+  destruct ds_d5S0 as [n1 n2];
   [fix_notations];
   simpl in *.
   Transparent fstSF.
@@ -2535,8 +2584,8 @@ Qed.
 #[global] Opaque fstSF.
 
 Theorem fstSF__fstSF_rel_rw
-  (ds_d5Rf : Natprod_u) (ds_d5Rf_p : Natprod_wf ds_d5Rf ∧ True) (VV : MyNat_u):
-  ⌊ fstSF (exist _ ds_d5Rf ds_d5Rf_p) -⌋ = VV ↔ fstSF_rel ds_d5Rf VV.
+  (ds_d5S0 : Natprod_u) (ds_d5S0_p : Natprod_wf ds_d5S0 ∧ True) (VV : MyNat_u):
+  ⌊ fstSF (exist _ ds_d5S0 ds_d5S0_p) -⌋ = VV ↔ fstSF_rel ds_d5S0 VV.
 Proof.
   f__f_rel_rw.
 Qed.
@@ -2547,27 +2596,27 @@ Qed.
 
 #[global] Instance fstSF_lookup_rw: dictionary rwLem fstSF := { lookup' := fstSF__fstSF_rel_rw }.
 
-Theorem fstSF__fstSF_rel (ds_d5Rf : Natprod) (VV : MyNat_u):
-  ⌊ fstSF ds_d5Rf -⌋ = VV ↔ fstSF_rel ⌊ ds_d5Rf ⌋ VV.
+Theorem fstSF__fstSF_rel (ds_d5S0 : Natprod) (VV : MyNat_u):
+  ⌊ fstSF ds_d5S0 -⌋ = VV ↔ fstSF_rel ⌊ ds_d5S0 ⌋ VV.
 Proof.
   f__f_rel.
 Qed.
 
 #[global] Hint Rewrite fstSF__fstSF_rel: f_rel_funct_db.
 
-Theorem fstSF__fstSF_rel' (ds_d5Rf_u : Natprod_u) (ds_d5Rf : Natprod) (VV : MyNat_u):
-  ds_d5Rf_u = ⌊ ds_d5Rf ⌋ → ⌊ fstSF ds_d5Rf -⌋ = VV ↔ fstSF_rel ds_d5Rf_u VV.
+Theorem fstSF__fstSF_rel' (ds_d5S0_u : Natprod_u) (ds_d5S0 : Natprod) (VV : MyNat_u):
+  ds_d5S0_u = ⌊ ds_d5S0 ⌋ → ⌊ fstSF ds_d5S0 -⌋ = VV ↔ fstSF_rel ds_d5S0_u VV.
 Proof.
-  intros ->. refine (fstSF__fstSF_rel ds_d5Rf VV).
+  intros ->. refine (fstSF__fstSF_rel ds_d5S0 VV).
 Qed.
 
 #[global] Hint Resolve fstSF__fstSF_rel': f_rel_funct_db.
 
-Theorem fstSF_rel_mk (ds_d5Rf : Natprod_u) (ds_d5Rf_p : Natprod_wf ds_d5Rf ∧ True):
-  {VV: _ | fstSF_rel ds_d5Rf VV}.
+Theorem fstSF_rel_mk (ds_d5S0 : Natprod_u) (ds_d5S0_p : Natprod_wf ds_d5S0 ∧ True):
+  {VV: _ | fstSF_rel ds_d5S0 VV}.
 Proof.
   intros;
-  refine (subsumptionCast _ (λ VV, fstSF_rel ds_d5Rf VV) (fstSF (exist _ ds_d5Rf ds_d5Rf_p)) _);
+  refine (subsumptionCast _ (λ VV, fstSF_rel ds_d5S0 VV) (fstSF (exist _ ds_d5S0 ds_d5S0_p)) _);
   rewrite <- fstSF__fstSF_rel';
   quicksolve.
 Qed.
@@ -2576,12 +2625,12 @@ Qed.
 
 #[global] Instance fstSF_pack:
   @Pack
-  (Natprod ::RT λ (ds_d5Rf : Natprod), nilRT)
+  (Natprod ::RT λ (ds_d5S0 : Natprod), nilRT)
   (Natprod_u ::UT nilUT)
-  ltac:(mkProjectsArgListTG (Natprod ::RT λ (ds_d5Rf : Natprod), nilRT) ((Natprod_u ::UT nilUT)))
+  ltac:(mkProjectsArgListTG (Natprod ::RT λ (ds_d5S0 : Natprod), nilRT) ((Natprod_u ::UT nilUT)))
   MyNat_u
-  (λ (x_27286868 : ArgList (Natprod ::RT λ (ds_d5Rf : Natprod), nilRT)) (v_x_27286868 : MyNat_u),
-   ltac:(flattenP (λ (ds_d5Rf : Natprod) (VV : MyNat_u), MyNat_wf VV ∧ True) x_27286868 v_x_27286868)).
+  (λ (x_76449427 : ArgList (Natprod ::RT λ (ds_d5S0 : Natprod), nilRT)) (v_x_76449427 : MyNat_u),
+   ltac:(flattenP (λ (ds_d5S0 : Natprod) (VV : MyNat_u), MyNat_wf VV ∧ True) x_76449427 v_x_76449427)).
 Proof.
   buildPackG fstSF fstSF_rel fstSF__fstSF_rel fstSF_rel_funct.
 Defined.
@@ -2591,24 +2640,24 @@ Proof.
   buildUPackG fstSF_rel fstSF_rel_funct.
 Defined.
 
-Definition leb_spec (ds_d5Ss ds_d5St : MyNat): Type :=
+Definition leb_spec (ds_d5Td ds_d5Te : MyNat): Type :=
   SFBool.
 
 #[global] Hint Unfold leb_spec: lia_unfold.
 
-Definition leb (ds_d5Ss ds_d5St : MyNat): leb_spec ds_d5Ss ds_d5St.
+Definition leb (ds_d5Td ds_d5Te : MyNat): leb_spec ds_d5Td ds_d5Te.
 Proof.
-  destruct ds_d5Ss as [ds_d5Ss ds_d5Ss_p].
-  destruct ds_d5St as [ds_d5St ds_d5St_p].
-  try revert ds_d5St_p; generalize dependent ds_d5St; induction ds_d5Ss as [| n' IH_n']; intros.
+  destruct ds_d5Td as [ds_d5Td ds_d5Td_p].
+  destruct ds_d5Te as [ds_d5Te ds_d5Te_p].
+  try revert ds_d5Te_p; generalize dependent ds_d5Te; induction ds_d5Td as [| n' IH_n']; intros.
   - refine SFTrue.
-  - destruct ds_d5St as [| m'].
+  - destruct ds_d5Te as [| m'].
     + refine SFFalse.
     + refine (IH_n' ltac:(try clear IH_n'; solver) m' ltac:(try clear IH_n'; solver)).
 Defined.
 
 Inductive leb_rel: MyNat_u → MyNat_u → SFBool_u → Prop :=
-  | leb_O_x: ∀ ds_d5St, leb_rel O_u ds_d5St SFTrue_u
+  | leb_O_x: ∀ ds_d5Te, leb_rel O_u ds_d5Te SFTrue_u
   | leb_S_O: ∀ n', leb_rel (S_u n') O_u SFFalse_u
   | leb_S_S: ∀ n' m' (leb_res : SFBool_u), leb_rel n' m' leb_res → leb_rel (S_u n') (S_u m') leb_res.
 
@@ -2618,11 +2667,11 @@ Inductive leb_rel: MyNat_u → MyNat_u → SFBool_u → Prop :=
 
 #[global] Instance leb_getF: getFunc leb_rel := { getF' := leb }.
 
-Theorem leb_rel_funct [ds_d5Ss ds_d5St : MyNat_u]:
-  ∀ (VV VV' : SFBool_u), leb_rel ds_d5Ss ds_d5St VV → (leb_rel ds_d5Ss ds_d5St VV' → VV = VV').
+Theorem leb_rel_funct [ds_d5Td ds_d5Te : MyNat_u]:
+  ∀ (VV VV' : SFBool_u), leb_rel ds_d5Td ds_d5Te VV → (leb_rel ds_d5Td ds_d5Te VV' → VV = VV').
 Proof.
-  try revert ds_d5St_p; generalize dependent ds_d5St; induction ds_d5Ss as [| n' IH_n']; intros;
-  [ | destruct ds_d5St as [| m']];
+  try revert ds_d5Te_p; generalize dependent ds_d5Te; induction ds_d5Td as [| n' IH_n']; intros;
+  [ | destruct ds_d5Te as [| m']];
   rel_functionhood_body.
 Qed.
 
@@ -2630,8 +2679,8 @@ Qed.
 
 #[global] Instance leb_lookup_funct: dictionary functionhood leb := { lookup' := leb_rel_funct }.
 
-Theorem leb_O_x_lem ds_d5St leb_O_x_lem_res:
-  leb_rel O_u ds_d5St leb_O_x_lem_res ↔ leb_O_x_lem_res == SFTrue_u.
+Theorem leb_O_x_lem ds_d5Te leb_O_x_lem_res:
+  leb_rel O_u ds_d5Te leb_O_x_lem_res ↔ leb_O_x_lem_res == SFTrue_u.
 Proof.
   rel_back' _nil.
 Qed.
@@ -2656,17 +2705,17 @@ Qed.
 #[global] Hint Rewrite leb_S_S_lem: f_rel_back.
 
 Theorem leb_rel_ex
-  (ds_d5Ss : MyNat_u)
-  (ds_d5Ss_p : MyNat_wf ds_d5Ss ∧ True)
-  (ds_d5St : MyNat_u)
-  (ds_d5St_p : MyNat_wf ds_d5St ∧ True):
-  leb_rel ds_d5Ss ds_d5St ⌊ leb (exist _ ds_d5Ss ds_d5Ss_p) (exist _ ds_d5St ds_d5St_p) -⌋.
+  (ds_d5Td : MyNat_u)
+  (ds_d5Td_p : MyNat_wf ds_d5Td ∧ True)
+  (ds_d5Te : MyNat_u)
+  (ds_d5Te_p : MyNat_wf ds_d5Te ∧ True):
+  leb_rel ds_d5Td ds_d5Te ⌊ leb (exist _ ds_d5Td ds_d5Td_p) (exist _ ds_d5Te ds_d5Te_p) -⌋.
 Proof.
   Opaque leb.
   existence_lemma_pre leb;
-  try revert ds_d5St_p; generalize dependent ds_d5St; induction ds_d5Ss as [| n' IH_n']; intros;
+  try revert ds_d5Te_p; generalize dependent ds_d5Te; induction ds_d5Td as [| n' IH_n']; intros;
   [fix_notations |
-   destruct ds_d5St as [| m'];
+   destruct ds_d5Te as [| m'];
    [fix_notations |
     fix_notations;
     pose proof (IH_n' ltac:(try clear IH_n'; solver) m' ltac:(try clear IH_n'; solver)) as IH_11391185;
@@ -2681,12 +2730,12 @@ Qed.
 #[global] Opaque leb.
 
 Theorem leb__leb_rel_rw
-  (ds_d5Ss : MyNat_u)
-  (ds_d5Ss_p : MyNat_wf ds_d5Ss ∧ True)
-  (ds_d5St : MyNat_u)
-  (ds_d5St_p : MyNat_wf ds_d5St ∧ True)
+  (ds_d5Td : MyNat_u)
+  (ds_d5Td_p : MyNat_wf ds_d5Td ∧ True)
+  (ds_d5Te : MyNat_u)
+  (ds_d5Te_p : MyNat_wf ds_d5Te ∧ True)
   (VV : SFBool_u):
-  ⌊ leb (exist _ ds_d5Ss ds_d5Ss_p) (exist _ ds_d5St ds_d5St_p) -⌋ = VV ↔ leb_rel ds_d5Ss ds_d5St VV.
+  ⌊ leb (exist _ ds_d5Td ds_d5Td_p) (exist _ ds_d5Te ds_d5Te_p) -⌋ = VV ↔ leb_rel ds_d5Td ds_d5Te VV.
 Proof.
   f__f_rel_rw.
 Qed.
@@ -2697,35 +2746,35 @@ Qed.
 
 #[global] Instance leb_lookup_rw: dictionary rwLem leb := { lookup' := leb__leb_rel_rw }.
 
-Theorem leb__leb_rel (ds_d5Ss ds_d5St : MyNat) (VV : SFBool_u):
-  ⌊ leb ds_d5Ss ds_d5St -⌋ = VV ↔ leb_rel ⌊ ds_d5Ss ⌋ ⌊ ds_d5St ⌋ VV.
+Theorem leb__leb_rel (ds_d5Td ds_d5Te : MyNat) (VV : SFBool_u):
+  ⌊ leb ds_d5Td ds_d5Te -⌋ = VV ↔ leb_rel ⌊ ds_d5Td ⌋ ⌊ ds_d5Te ⌋ VV.
 Proof.
   f__f_rel.
 Qed.
 
 #[global] Hint Rewrite leb__leb_rel: f_rel_funct_db.
 
-Theorem leb__leb_rel' (ds_d5Ss_u ds_d5St_u : MyNat_u) (ds_d5Ss ds_d5St : MyNat) (VV : SFBool_u):
-  ds_d5Ss_u = ⌊ ds_d5Ss ⌋
-  → (ds_d5St_u = ⌊ ds_d5St ⌋ → ⌊ leb ds_d5Ss ds_d5St -⌋ = VV ↔ leb_rel ds_d5Ss_u ds_d5St_u VV).
+Theorem leb__leb_rel' (ds_d5Td_u ds_d5Te_u : MyNat_u) (ds_d5Td ds_d5Te : MyNat) (VV : SFBool_u):
+  ds_d5Td_u = ⌊ ds_d5Td ⌋
+  → (ds_d5Te_u = ⌊ ds_d5Te ⌋ → ⌊ leb ds_d5Td ds_d5Te -⌋ = VV ↔ leb_rel ds_d5Td_u ds_d5Te_u VV).
 Proof.
-  intros -> ->. refine (leb__leb_rel ds_d5Ss ds_d5St VV).
+  intros -> ->. refine (leb__leb_rel ds_d5Td ds_d5Te VV).
 Qed.
 
 #[global] Hint Resolve leb__leb_rel': f_rel_funct_db.
 
 Theorem leb_rel_mk
-  (ds_d5Ss : MyNat_u)
-  (ds_d5Ss_p : MyNat_wf ds_d5Ss ∧ True)
-  (ds_d5St : MyNat_u)
-  (ds_d5St_p : MyNat_wf ds_d5St ∧ True):
-  {VV: _ | leb_rel ds_d5Ss ds_d5St VV}.
+  (ds_d5Td : MyNat_u)
+  (ds_d5Td_p : MyNat_wf ds_d5Td ∧ True)
+  (ds_d5Te : MyNat_u)
+  (ds_d5Te_p : MyNat_wf ds_d5Te ∧ True):
+  {VV: _ | leb_rel ds_d5Td ds_d5Te VV}.
 Proof.
   intros;
   refine (subsumptionCast
           _
-          (λ VV, leb_rel ds_d5Ss ds_d5St VV)
-          (leb (exist _ ds_d5Ss ds_d5Ss_p) (exist _ ds_d5St ds_d5St_p))
+          (λ VV, leb_rel ds_d5Td ds_d5Te VV)
+          (leb (exist _ ds_d5Td ds_d5Td_p) (exist _ ds_d5Te ds_d5Te_p))
           _);
   rewrite <- leb__leb_rel';
   quicksolve.
@@ -2735,14 +2784,14 @@ Qed.
 
 #[global] Instance leb_pack:
   @Pack
-  (MyNat ::RT λ (ds_d5Ss : MyNat), MyNat ::RT λ (ds_d5St : MyNat), nilRT)
+  (MyNat ::RT λ (ds_d5Td : MyNat), MyNat ::RT λ (ds_d5Te : MyNat), nilRT)
   (MyNat_u ::UT (MyNat_u ::UT nilUT))
   ltac:(mkProjectsArgListTG (MyNat
- ::RT λ (ds_d5Ss : MyNat), MyNat ::RT λ (ds_d5St : MyNat), nilRT) ((MyNat_u ::UT (MyNat_u ::UT nilUT))))
+ ::RT λ (ds_d5Td : MyNat), MyNat ::RT λ (ds_d5Te : MyNat), nilRT) ((MyNat_u ::UT (MyNat_u ::UT nilUT))))
   SFBool_u
-  (λ (x_23682632 : ArgList (MyNat ::RT λ (ds_d5Ss : MyNat), MyNat ::RT λ (ds_d5St : MyNat), nilRT))
-     (v_x_23682632 : SFBool_u),
-   ltac:(flattenP (λ (ds_d5Ss ds_d5St : MyNat) (VV : SFBool_u), SFBool_wf VV ∧ True) x_23682632 v_x_23682632)).
+  (λ (x_53324001 : ArgList (MyNat ::RT λ (ds_d5Td : MyNat), MyNat ::RT λ (ds_d5Te : MyNat), nilRT))
+     (v_x_53324001 : SFBool_u),
+   ltac:(flattenP (λ (ds_d5Td ds_d5Te : MyNat) (VV : SFBool_u), SFBool_wf VV ∧ True) x_53324001 v_x_53324001)).
 Proof.
   buildPackG leb leb_rel leb__leb_rel leb_rel_funct.
 Defined.
@@ -2752,20 +2801,20 @@ Proof.
   buildUPackG leb_rel leb_rel_funct.
 Defined.
 
-Definition ltb_spec (ds_d5Sq ds_d5Sr : MyNat): Type :=
+Definition ltb_spec (ds_d5Tb ds_d5Tc : MyNat): Type :=
   SFBool.
 
 #[global] Hint Unfold ltb_spec: lia_unfold.
 
-Definition ltb (ds_d5Sq ds_d5Sr : MyNat): ltb_spec ds_d5Sq ds_d5Sr.
+Definition ltb (ds_d5Tb ds_d5Tc : MyNat): ltb_spec ds_d5Tb ds_d5Tc.
 Proof.
-  destruct ds_d5Sq as [ds_d5Sq ds_d5Sq_p].
-  destruct ds_d5Sr as [ds_d5Sr ds_d5Sr_p].
-  try revert ds_d5Sr_p; generalize dependent ds_d5Sr; induction ds_d5Sq as [| n' IH_n']; intros.
-  - destruct ds_d5Sr as [| m'].
+  destruct ds_d5Tb as [ds_d5Tb ds_d5Tb_p].
+  destruct ds_d5Tc as [ds_d5Tc ds_d5Tc_p].
+  try revert ds_d5Tc_p; generalize dependent ds_d5Tc; induction ds_d5Tb as [| n' IH_n']; intros.
+  - destruct ds_d5Tc as [| m'].
     + refine SFFalse.
     + refine SFTrue.
-  - destruct ds_d5Sr as [| m'].
+  - destruct ds_d5Tc as [| m'].
     + refine SFFalse.
     + refine (IH_n' ltac:(try clear IH_n'; solver) m' ltac:(try clear IH_n'; solver)).
 Defined.
@@ -2782,11 +2831,11 @@ Inductive ltb_rel: MyNat_u → MyNat_u → SFBool_u → Prop :=
 
 #[global] Instance ltb_getF: getFunc ltb_rel := { getF' := ltb }.
 
-Theorem ltb_rel_funct [ds_d5Sq ds_d5Sr : MyNat_u]:
-  ∀ (VV VV' : SFBool_u), ltb_rel ds_d5Sq ds_d5Sr VV → (ltb_rel ds_d5Sq ds_d5Sr VV' → VV = VV').
+Theorem ltb_rel_funct [ds_d5Tb ds_d5Tc : MyNat_u]:
+  ∀ (VV VV' : SFBool_u), ltb_rel ds_d5Tb ds_d5Tc VV → (ltb_rel ds_d5Tb ds_d5Tc VV' → VV = VV').
 Proof.
-  try revert ds_d5Sr_p; generalize dependent ds_d5Sr; induction ds_d5Sq as [| n' IH_n']; intros;
-  [destruct ds_d5Sr as [| m'] | destruct ds_d5Sr as [| m']];
+  try revert ds_d5Tc_p; generalize dependent ds_d5Tc; induction ds_d5Tb as [| n' IH_n']; intros;
+  [destruct ds_d5Tc as [| m'] | destruct ds_d5Tc as [| m']];
   rel_functionhood_body.
 Qed.
 
@@ -2827,18 +2876,18 @@ Qed.
 #[global] Hint Rewrite ltb_S_S_lem: f_rel_back.
 
 Theorem ltb_rel_ex
-  (ds_d5Sq : MyNat_u)
-  (ds_d5Sq_p : MyNat_wf ds_d5Sq ∧ True)
-  (ds_d5Sr : MyNat_u)
-  (ds_d5Sr_p : MyNat_wf ds_d5Sr ∧ True):
-  ltb_rel ds_d5Sq ds_d5Sr ⌊ ltb (exist _ ds_d5Sq ds_d5Sq_p) (exist _ ds_d5Sr ds_d5Sr_p) -⌋.
+  (ds_d5Tb : MyNat_u)
+  (ds_d5Tb_p : MyNat_wf ds_d5Tb ∧ True)
+  (ds_d5Tc : MyNat_u)
+  (ds_d5Tc_p : MyNat_wf ds_d5Tc ∧ True):
+  ltb_rel ds_d5Tb ds_d5Tc ⌊ ltb (exist _ ds_d5Tb ds_d5Tb_p) (exist _ ds_d5Tc ds_d5Tc_p) -⌋.
 Proof.
   Opaque ltb.
   existence_lemma_pre ltb;
-  try revert ds_d5Sr_p; generalize dependent ds_d5Sr; induction ds_d5Sq as [| n' IH_n']; intros;
-  [destruct ds_d5Sr as [| m'];
+  try revert ds_d5Tc_p; generalize dependent ds_d5Tc; induction ds_d5Tb as [| n' IH_n']; intros;
+  [destruct ds_d5Tc as [| m'];
    [fix_notations | fix_notations] |
-   destruct ds_d5Sr as [| m'];
+   destruct ds_d5Tc as [| m'];
    [fix_notations |
     fix_notations;
     pose proof (IH_n' ltac:(try clear IH_n'; solver) m' ltac:(try clear IH_n'; solver)) as IH_11391185;
@@ -2853,12 +2902,12 @@ Qed.
 #[global] Opaque ltb.
 
 Theorem ltb__ltb_rel_rw
-  (ds_d5Sq : MyNat_u)
-  (ds_d5Sq_p : MyNat_wf ds_d5Sq ∧ True)
-  (ds_d5Sr : MyNat_u)
-  (ds_d5Sr_p : MyNat_wf ds_d5Sr ∧ True)
+  (ds_d5Tb : MyNat_u)
+  (ds_d5Tb_p : MyNat_wf ds_d5Tb ∧ True)
+  (ds_d5Tc : MyNat_u)
+  (ds_d5Tc_p : MyNat_wf ds_d5Tc ∧ True)
   (VV : SFBool_u):
-  ⌊ ltb (exist _ ds_d5Sq ds_d5Sq_p) (exist _ ds_d5Sr ds_d5Sr_p) -⌋ = VV ↔ ltb_rel ds_d5Sq ds_d5Sr VV.
+  ⌊ ltb (exist _ ds_d5Tb ds_d5Tb_p) (exist _ ds_d5Tc ds_d5Tc_p) -⌋ = VV ↔ ltb_rel ds_d5Tb ds_d5Tc VV.
 Proof.
   f__f_rel_rw.
 Qed.
@@ -2869,35 +2918,35 @@ Qed.
 
 #[global] Instance ltb_lookup_rw: dictionary rwLem ltb := { lookup' := ltb__ltb_rel_rw }.
 
-Theorem ltb__ltb_rel (ds_d5Sq ds_d5Sr : MyNat) (VV : SFBool_u):
-  ⌊ ltb ds_d5Sq ds_d5Sr -⌋ = VV ↔ ltb_rel ⌊ ds_d5Sq ⌋ ⌊ ds_d5Sr ⌋ VV.
+Theorem ltb__ltb_rel (ds_d5Tb ds_d5Tc : MyNat) (VV : SFBool_u):
+  ⌊ ltb ds_d5Tb ds_d5Tc -⌋ = VV ↔ ltb_rel ⌊ ds_d5Tb ⌋ ⌊ ds_d5Tc ⌋ VV.
 Proof.
   f__f_rel.
 Qed.
 
 #[global] Hint Rewrite ltb__ltb_rel: f_rel_funct_db.
 
-Theorem ltb__ltb_rel' (ds_d5Sq_u ds_d5Sr_u : MyNat_u) (ds_d5Sq ds_d5Sr : MyNat) (VV : SFBool_u):
-  ds_d5Sq_u = ⌊ ds_d5Sq ⌋
-  → (ds_d5Sr_u = ⌊ ds_d5Sr ⌋ → ⌊ ltb ds_d5Sq ds_d5Sr -⌋ = VV ↔ ltb_rel ds_d5Sq_u ds_d5Sr_u VV).
+Theorem ltb__ltb_rel' (ds_d5Tb_u ds_d5Tc_u : MyNat_u) (ds_d5Tb ds_d5Tc : MyNat) (VV : SFBool_u):
+  ds_d5Tb_u = ⌊ ds_d5Tb ⌋
+  → (ds_d5Tc_u = ⌊ ds_d5Tc ⌋ → ⌊ ltb ds_d5Tb ds_d5Tc -⌋ = VV ↔ ltb_rel ds_d5Tb_u ds_d5Tc_u VV).
 Proof.
-  intros -> ->. refine (ltb__ltb_rel ds_d5Sq ds_d5Sr VV).
+  intros -> ->. refine (ltb__ltb_rel ds_d5Tb ds_d5Tc VV).
 Qed.
 
 #[global] Hint Resolve ltb__ltb_rel': f_rel_funct_db.
 
 Theorem ltb_rel_mk
-  (ds_d5Sq : MyNat_u)
-  (ds_d5Sq_p : MyNat_wf ds_d5Sq ∧ True)
-  (ds_d5Sr : MyNat_u)
-  (ds_d5Sr_p : MyNat_wf ds_d5Sr ∧ True):
-  {VV: _ | ltb_rel ds_d5Sq ds_d5Sr VV}.
+  (ds_d5Tb : MyNat_u)
+  (ds_d5Tb_p : MyNat_wf ds_d5Tb ∧ True)
+  (ds_d5Tc : MyNat_u)
+  (ds_d5Tc_p : MyNat_wf ds_d5Tc ∧ True):
+  {VV: _ | ltb_rel ds_d5Tb ds_d5Tc VV}.
 Proof.
   intros;
   refine (subsumptionCast
           _
-          (λ VV, ltb_rel ds_d5Sq ds_d5Sr VV)
-          (ltb (exist _ ds_d5Sq ds_d5Sq_p) (exist _ ds_d5Sr ds_d5Sr_p))
+          (λ VV, ltb_rel ds_d5Tb ds_d5Tc VV)
+          (ltb (exist _ ds_d5Tb ds_d5Tb_p) (exist _ ds_d5Tc ds_d5Tc_p))
           _);
   rewrite <- ltb__ltb_rel';
   quicksolve.
@@ -2907,14 +2956,14 @@ Qed.
 
 #[global] Instance ltb_pack:
   @Pack
-  (MyNat ::RT λ (ds_d5Sq : MyNat), MyNat ::RT λ (ds_d5Sr : MyNat), nilRT)
+  (MyNat ::RT λ (ds_d5Tb : MyNat), MyNat ::RT λ (ds_d5Tc : MyNat), nilRT)
   (MyNat_u ::UT (MyNat_u ::UT nilUT))
   ltac:(mkProjectsArgListTG (MyNat
- ::RT λ (ds_d5Sq : MyNat), MyNat ::RT λ (ds_d5Sr : MyNat), nilRT) ((MyNat_u ::UT (MyNat_u ::UT nilUT))))
+ ::RT λ (ds_d5Tb : MyNat), MyNat ::RT λ (ds_d5Tc : MyNat), nilRT) ((MyNat_u ::UT (MyNat_u ::UT nilUT))))
   SFBool_u
-  (λ (x_35558007 : ArgList (MyNat ::RT λ (ds_d5Sq : MyNat), MyNat ::RT λ (ds_d5Sr : MyNat), nilRT))
-     (v_x_35558007 : SFBool_u),
-   ltac:(flattenP (λ (ds_d5Sq ds_d5Sr : MyNat) (VV : SFBool_u), SFBool_wf VV ∧ True) x_35558007 v_x_35558007)).
+  (λ (x_44364634 : ArgList (MyNat ::RT λ (ds_d5Tb : MyNat), MyNat ::RT λ (ds_d5Tc : MyNat), nilRT))
+     (v_x_44364634 : SFBool_u),
+   ltac:(flattenP (λ (ds_d5Tb ds_d5Tc : MyNat) (VV : SFBool_u), SFBool_wf VV ∧ True) x_44364634 v_x_44364634)).
 Proof.
   buildPackG ltb ltb_rel ltb__ltb_rel ltb_rel_funct.
 Defined.
@@ -2924,29 +2973,29 @@ Proof.
   buildUPackG ltb_rel ltb_rel_funct.
 Defined.
 
-Definition minus_spec (ds_d5Sw ds_d5Sx : MyNat): Type :=
+Definition minus_spec (ds_d5Th ds_d5Ti : MyNat): Type :=
   MyNat.
 
 #[global] Hint Unfold minus_spec: lia_unfold.
 
-Definition minus (ds_d5Sw ds_d5Sx : MyNat): minus_spec ds_d5Sw ds_d5Sx.
+Definition minus (ds_d5Th ds_d5Ti : MyNat): minus_spec ds_d5Th ds_d5Ti.
 Proof.
-  destruct ds_d5Sw as [ds_d5Sw ds_d5Sw_p].
-  destruct ds_d5Sx as [ds_d5Sx ds_d5Sx_p].
-  try revert ds_d5Sx_p; generalize dependent ds_d5Sx;
-  induction ds_d5Sw as [| ds_d5Sy IH_ds_d5Sy];
+  destruct ds_d5Th as [ds_d5Th ds_d5Th_p].
+  destruct ds_d5Ti as [ds_d5Ti ds_d5Ti_p].
+  try revert ds_d5Ti_p; generalize dependent ds_d5Ti;
+  induction ds_d5Th as [| ds_d5Tj IH_ds_d5Tj];
   intros.
   - refine O.
-  - destruct ds_d5Sx as [| m'].
-    + refine (S (exist (λ (VV : MyNat_u), MyNat_wf VV ∧ True) ds_d5Sy ltac:(solver))).
-    + refine (IH_ds_d5Sy ltac:(try clear IH_ds_d5Sy; solver) m' ltac:(try clear IH_ds_d5Sy; solver)).
+  - destruct ds_d5Ti as [| m'].
+    + refine (S (exist (λ (VV : MyNat_u), MyNat_wf VV ∧ True) ds_d5Tj ltac:(solver))).
+    + refine (IH_ds_d5Tj ltac:(try clear IH_ds_d5Tj; solver) m' ltac:(try clear IH_ds_d5Tj; solver)).
 Defined.
 
 Inductive minus_rel: MyNat_u → MyNat_u → MyNat_u → Prop :=
-  | minus_O_x: ∀ ds_d5Sx, minus_rel O_u ds_d5Sx O_u
-  | minus_S_O: ∀ ds_d5Sy, minus_rel (S_u ds_d5Sy) O_u (S_u ds_d5Sy)
-  | minus_S_S: ∀ ds_d5Sy m' (minus_res : MyNat_u),
-               minus_rel ds_d5Sy m' minus_res → minus_rel (S_u ds_d5Sy) (S_u m') minus_res.
+  | minus_O_x: ∀ ds_d5Ti, minus_rel O_u ds_d5Ti O_u
+  | minus_S_O: ∀ ds_d5Tj, minus_rel (S_u ds_d5Tj) O_u (S_u ds_d5Tj)
+  | minus_S_S: ∀ ds_d5Tj m' (minus_res : MyNat_u),
+               minus_rel ds_d5Tj m' minus_res → minus_rel (S_u ds_d5Tj) (S_u m') minus_res.
 
 #[global] Hint Constructors minus_rel: core_hint_db.
 
@@ -2954,13 +3003,13 @@ Inductive minus_rel: MyNat_u → MyNat_u → MyNat_u → Prop :=
 
 #[global] Instance minus_getF: getFunc minus_rel := { getF' := minus }.
 
-Theorem minus_rel_funct [ds_d5Sw ds_d5Sx : MyNat_u]:
-  ∀ (VV VV' : MyNat_u), minus_rel ds_d5Sw ds_d5Sx VV → (minus_rel ds_d5Sw ds_d5Sx VV' → VV = VV').
+Theorem minus_rel_funct [ds_d5Th ds_d5Ti : MyNat_u]:
+  ∀ (VV VV' : MyNat_u), minus_rel ds_d5Th ds_d5Ti VV → (minus_rel ds_d5Th ds_d5Ti VV' → VV = VV').
 Proof.
-  try revert ds_d5Sx_p; generalize dependent ds_d5Sx;
-  induction ds_d5Sw as [| ds_d5Sy IH_ds_d5Sy];
+  try revert ds_d5Ti_p; generalize dependent ds_d5Ti;
+  induction ds_d5Th as [| ds_d5Tj IH_ds_d5Tj];
   intros;
-  [ | destruct ds_d5Sx as [| m']];
+  [ | destruct ds_d5Ti as [| m']];
   rel_functionhood_body.
 Qed.
 
@@ -2969,25 +3018,25 @@ Qed.
 #[global] Instance minus_lookup_funct: dictionary functionhood minus := {
     lookup' := minus_rel_funct }.
 
-Theorem minus_O_x_lem ds_d5Sx minus_O_x_lem_res:
-  minus_rel O_u ds_d5Sx minus_O_x_lem_res ↔ minus_O_x_lem_res == O_u.
+Theorem minus_O_x_lem ds_d5Ti minus_O_x_lem_res:
+  minus_rel O_u ds_d5Ti minus_O_x_lem_res ↔ minus_O_x_lem_res == O_u.
 Proof.
   rel_back' _nil.
 Qed.
 
 #[global] Hint Rewrite minus_O_x_lem: f_rel_back.
 
-Theorem minus_S_O_lem ds_d5Sy minus_S_O_lem_res:
-  minus_rel (S_u ds_d5Sy) O_u minus_S_O_lem_res ↔ minus_S_O_lem_res == S_u ds_d5Sy.
+Theorem minus_S_O_lem ds_d5Tj minus_S_O_lem_res:
+  minus_rel (S_u ds_d5Tj) O_u minus_S_O_lem_res ↔ minus_S_O_lem_res == S_u ds_d5Tj.
 Proof.
   rel_back' _nil.
 Qed.
 
 #[global] Hint Rewrite minus_S_O_lem: f_rel_back.
 
-Theorem minus_S_S_lem ds_d5Sy m' minus_S_S_lem_res:
-  minus_rel (S_u ds_d5Sy) (S_u m') minus_S_S_lem_res
-  ↔ ∃ (minus_res : MyNat_u), minus_rel ds_d5Sy m' minus_res ∧ minus_S_S_lem_res == minus_res.
+Theorem minus_S_S_lem ds_d5Tj m' minus_S_S_lem_res:
+  minus_rel (S_u ds_d5Tj) (S_u m') minus_S_S_lem_res
+  ↔ ∃ (minus_res : MyNat_u), minus_rel ds_d5Tj m' minus_res ∧ minus_S_S_lem_res == minus_res.
 Proof.
   rel_back' _nil.
 Qed.
@@ -2995,26 +3044,26 @@ Qed.
 #[global] Hint Rewrite minus_S_S_lem: f_rel_back.
 
 Theorem minus_rel_ex
-  (ds_d5Sw : MyNat_u)
-  (ds_d5Sw_p : MyNat_wf ds_d5Sw ∧ True)
-  (ds_d5Sx : MyNat_u)
-  (ds_d5Sx_p : MyNat_wf ds_d5Sx ∧ True):
-  minus_rel ds_d5Sw ds_d5Sx ⌊ minus (exist _ ds_d5Sw ds_d5Sw_p) (exist _ ds_d5Sx ds_d5Sx_p) -⌋.
+  (ds_d5Th : MyNat_u)
+  (ds_d5Th_p : MyNat_wf ds_d5Th ∧ True)
+  (ds_d5Ti : MyNat_u)
+  (ds_d5Ti_p : MyNat_wf ds_d5Ti ∧ True):
+  minus_rel ds_d5Th ds_d5Ti ⌊ minus (exist _ ds_d5Th ds_d5Th_p) (exist _ ds_d5Ti ds_d5Ti_p) -⌋.
 Proof.
   Opaque minus.
   existence_lemma_pre minus;
-  try revert ds_d5Sx_p; generalize dependent ds_d5Sx;
-  induction ds_d5Sw as [| ds_d5Sy IH_ds_d5Sy];
+  try revert ds_d5Ti_p; generalize dependent ds_d5Ti;
+  induction ds_d5Th as [| ds_d5Tj IH_ds_d5Tj];
   intros;
   [fix_notations |
-   destruct ds_d5Sx as [| m'];
+   destruct ds_d5Ti as [| m'];
    [fix_notations |
     fix_notations;
-    pose proof (IH_ds_d5Sy
-                ltac:(try clear IH_ds_d5Sy; solver)
+    pose proof (IH_ds_d5Tj
+                ltac:(try clear IH_ds_d5Tj; solver)
                 m'
-                ltac:(try clear IH_ds_d5Sy; solver)) as IH_87163363;
-    try clear IH_ds_d5Sy]];
+                ltac:(try clear IH_ds_d5Tj; solver)) as IH_68920425;
+    try clear IH_ds_d5Tj]];
   simpl in *.
   Transparent minus.
   all: (existence_lemma_quicksolve minus; f__f_rel_ex_body; f_rel_finish).
@@ -3025,13 +3074,13 @@ Qed.
 #[global] Opaque minus.
 
 Theorem minus__minus_rel_rw
-  (ds_d5Sw : MyNat_u)
-  (ds_d5Sw_p : MyNat_wf ds_d5Sw ∧ True)
-  (ds_d5Sx : MyNat_u)
-  (ds_d5Sx_p : MyNat_wf ds_d5Sx ∧ True)
+  (ds_d5Th : MyNat_u)
+  (ds_d5Th_p : MyNat_wf ds_d5Th ∧ True)
+  (ds_d5Ti : MyNat_u)
+  (ds_d5Ti_p : MyNat_wf ds_d5Ti ∧ True)
   (VV : MyNat_u):
-  ⌊ minus (exist _ ds_d5Sw ds_d5Sw_p) (exist _ ds_d5Sx ds_d5Sx_p) -⌋ = VV
-  ↔ minus_rel ds_d5Sw ds_d5Sx VV.
+  ⌊ minus (exist _ ds_d5Th ds_d5Th_p) (exist _ ds_d5Ti ds_d5Ti_p) -⌋ = VV
+  ↔ minus_rel ds_d5Th ds_d5Ti VV.
 Proof.
   f__f_rel_rw.
 Qed.
@@ -3042,35 +3091,35 @@ Qed.
 
 #[global] Instance minus_lookup_rw: dictionary rwLem minus := { lookup' := minus__minus_rel_rw }.
 
-Theorem minus__minus_rel (ds_d5Sw ds_d5Sx : MyNat) (VV : MyNat_u):
-  ⌊ minus ds_d5Sw ds_d5Sx -⌋ = VV ↔ minus_rel ⌊ ds_d5Sw ⌋ ⌊ ds_d5Sx ⌋ VV.
+Theorem minus__minus_rel (ds_d5Th ds_d5Ti : MyNat) (VV : MyNat_u):
+  ⌊ minus ds_d5Th ds_d5Ti -⌋ = VV ↔ minus_rel ⌊ ds_d5Th ⌋ ⌊ ds_d5Ti ⌋ VV.
 Proof.
   f__f_rel.
 Qed.
 
 #[global] Hint Rewrite minus__minus_rel: f_rel_funct_db.
 
-Theorem minus__minus_rel' (ds_d5Sw_u ds_d5Sx_u : MyNat_u) (ds_d5Sw ds_d5Sx : MyNat) (VV : MyNat_u):
-  ds_d5Sw_u = ⌊ ds_d5Sw ⌋
-  → (ds_d5Sx_u = ⌊ ds_d5Sx ⌋ → ⌊ minus ds_d5Sw ds_d5Sx -⌋ = VV ↔ minus_rel ds_d5Sw_u ds_d5Sx_u VV).
+Theorem minus__minus_rel' (ds_d5Th_u ds_d5Ti_u : MyNat_u) (ds_d5Th ds_d5Ti : MyNat) (VV : MyNat_u):
+  ds_d5Th_u = ⌊ ds_d5Th ⌋
+  → (ds_d5Ti_u = ⌊ ds_d5Ti ⌋ → ⌊ minus ds_d5Th ds_d5Ti -⌋ = VV ↔ minus_rel ds_d5Th_u ds_d5Ti_u VV).
 Proof.
-  intros -> ->. refine (minus__minus_rel ds_d5Sw ds_d5Sx VV).
+  intros -> ->. refine (minus__minus_rel ds_d5Th ds_d5Ti VV).
 Qed.
 
 #[global] Hint Resolve minus__minus_rel': f_rel_funct_db.
 
 Theorem minus_rel_mk
-  (ds_d5Sw : MyNat_u)
-  (ds_d5Sw_p : MyNat_wf ds_d5Sw ∧ True)
-  (ds_d5Sx : MyNat_u)
-  (ds_d5Sx_p : MyNat_wf ds_d5Sx ∧ True):
-  {VV: _ | minus_rel ds_d5Sw ds_d5Sx VV}.
+  (ds_d5Th : MyNat_u)
+  (ds_d5Th_p : MyNat_wf ds_d5Th ∧ True)
+  (ds_d5Ti : MyNat_u)
+  (ds_d5Ti_p : MyNat_wf ds_d5Ti ∧ True):
+  {VV: _ | minus_rel ds_d5Th ds_d5Ti VV}.
 Proof.
   intros;
   refine (subsumptionCast
           _
-          (λ VV, minus_rel ds_d5Sw ds_d5Sx VV)
-          (minus (exist _ ds_d5Sw ds_d5Sw_p) (exist _ ds_d5Sx ds_d5Sx_p))
+          (λ VV, minus_rel ds_d5Th ds_d5Ti VV)
+          (minus (exist _ ds_d5Th ds_d5Th_p) (exist _ ds_d5Ti ds_d5Ti_p))
           _);
   rewrite <- minus__minus_rel';
   quicksolve.
@@ -3080,14 +3129,14 @@ Qed.
 
 #[global] Instance minus_pack:
   @Pack
-  (MyNat ::RT λ (ds_d5Sw : MyNat), MyNat ::RT λ (ds_d5Sx : MyNat), nilRT)
+  (MyNat ::RT λ (ds_d5Th : MyNat), MyNat ::RT λ (ds_d5Ti : MyNat), nilRT)
   (MyNat_u ::UT (MyNat_u ::UT nilUT))
   ltac:(mkProjectsArgListTG (MyNat
- ::RT λ (ds_d5Sw : MyNat), MyNat ::RT λ (ds_d5Sx : MyNat), nilRT) ((MyNat_u ::UT (MyNat_u ::UT nilUT))))
+ ::RT λ (ds_d5Th : MyNat), MyNat ::RT λ (ds_d5Ti : MyNat), nilRT) ((MyNat_u ::UT (MyNat_u ::UT nilUT))))
   MyNat_u
-  (λ (x_57956602 : ArgList (MyNat ::RT λ (ds_d5Sw : MyNat), MyNat ::RT λ (ds_d5Sx : MyNat), nilRT))
-     (v_x_57956602 : MyNat_u),
-   ltac:(flattenP (λ (ds_d5Sw ds_d5Sx : MyNat) (VV : MyNat_u), MyNat_wf VV ∧ True) x_57956602 v_x_57956602)).
+  (λ (x_65985781 : ArgList (MyNat ::RT λ (ds_d5Th : MyNat), MyNat ::RT λ (ds_d5Ti : MyNat), nilRT))
+     (v_x_65985781 : MyNat_u),
+   ltac:(flattenP (λ (ds_d5Th ds_d5Ti : MyNat) (VV : MyNat_u), MyNat_wf VV ∧ True) x_65985781 v_x_65985781)).
 Proof.
   buildPackG minus minus_rel minus__minus_rel minus_rel_funct.
 Defined.
@@ -3097,15 +3146,15 @@ Proof.
   buildUPackG minus_rel minus_rel_funct.
 Defined.
 
-Definition minus_n_n_spec (ds_d5Ri : MyNat): Type :=
-  {{∃ (minus_res : MyNat_u), minus_rel ⌊ ds_d5Ri -⌋ ⌊ ds_d5Ri -⌋ minus_res ∧ minus_res == O_u}}.
+Definition minus_n_n_spec (ds_d5S3 : MyNat): Type :=
+  {{∃ (minus_res : MyNat_u), minus_rel ⌊ ds_d5S3 -⌋ ⌊ ds_d5S3 -⌋ minus_res ∧ minus_res == O_u}}.
 
 #[global] Hint Unfold minus_n_n_spec: lia_unfold.
 
-Theorem minus_n_n (ds_d5Ri : MyNat): minus_n_n_spec ds_d5Ri.
+Theorem minus_n_n (ds_d5S3 : MyNat): minus_n_n_spec ds_d5S3.
 Proof.
-  destruct ds_d5Ri as [ds_d5Ri ds_d5Ri_p].
-  induction ds_d5Ri as [| n' IH_n'].
+  destruct ds_d5S3 as [ds_d5S3 ds_d5S3_p].
+  induction ds_d5S3 as [| n' IH_n'].
   - refine (subsumptionCast
             Unit
             (λ (VV : Unit), ∃ (minus_res : MyNat_u), minus_rel O_u O_u minus_res ∧ minus_res == O_u)
@@ -3118,17 +3167,17 @@ Proof.
             ltac:(solver)).
 Qed.
 
-Definition minustwo_spec (ds_d5SX : MyNat): Type :=
+Definition minustwo_spec (ds_d5TI : MyNat): Type :=
   MyNat.
 
 #[global] Hint Unfold minustwo_spec: lia_unfold.
 
-Definition minustwo (ds_d5SX : MyNat): minustwo_spec ds_d5SX.
+Definition minustwo (ds_d5TI : MyNat): minustwo_spec ds_d5TI.
 Proof.
-  destruct ds_d5SX as [ds_d5SX ds_d5SX_p].
-  destruct ds_d5SX as [| ds_d5SY].
+  destruct ds_d5TI as [ds_d5TI ds_d5TI_p].
+  destruct ds_d5TI as [| ds_d5TJ].
   - refine O.
-  - destruct ds_d5SY as [| n'].
+  - destruct ds_d5TJ as [| n'].
     + refine O.
     + refine (exist (λ (VV : MyNat_u), MyNat_wf VV ∧ True) n' ltac:(solver)).
 Defined.
@@ -3143,16 +3192,16 @@ Proof.
   refine (S O).
 Defined.
 
-Definition plus_spec (ds_d5SL m : MyNat): Type :=
+Definition plus_spec (ds_d5Tw m : MyNat): Type :=
   MyNat.
 
 #[global] Hint Unfold plus_spec: lia_unfold.
 
-Definition plus (ds_d5SL m : MyNat): plus_spec ds_d5SL m.
+Definition plus (ds_d5Tw m : MyNat): plus_spec ds_d5Tw m.
 Proof.
-  destruct ds_d5SL as [ds_d5SL ds_d5SL_p].
+  destruct ds_d5Tw as [ds_d5Tw ds_d5Tw_p].
   destruct m as [m m_p].
-  try revert m_p; generalize dependent m; induction ds_d5SL as [| n' IH_n']; intros.
+  try revert m_p; generalize dependent m; induction ds_d5Tw as [| n' IH_n']; intros.
   - refine (exist (λ (m : MyNat_u), MyNat_wf m ∧ True) m ltac:(solver)).
   - refine (S (IH_n' ltac:(try clear IH_n'; solver) m ltac:(try clear IH_n'; solver))).
 Defined.
@@ -3168,10 +3217,10 @@ Inductive plus_rel: MyNat_u → MyNat_u → MyNat_u → Prop :=
 
 #[global] Instance plus_getF: getFunc plus_rel := { getF' := plus }.
 
-Theorem plus_rel_funct [ds_d5SL m : MyNat_u]:
-  ∀ (VV VV' : MyNat_u), plus_rel ds_d5SL m VV → (plus_rel ds_d5SL m VV' → VV = VV').
+Theorem plus_rel_funct [ds_d5Tw m : MyNat_u]:
+  ∀ (VV VV' : MyNat_u), plus_rel ds_d5Tw m VV → (plus_rel ds_d5Tw m VV' → VV = VV').
 Proof.
-  try revert m_p; generalize dependent m; induction ds_d5SL as [| n' IH_n']; intros;
+  try revert m_p; generalize dependent m; induction ds_d5Tw as [| n' IH_n']; intros;
   rel_functionhood_body.
 Qed.
 
@@ -3197,12 +3246,12 @@ Qed.
 #[global] Hint Rewrite plus_S_x_lem: f_rel_back.
 
 Theorem plus_rel_ex
-  (ds_d5SL : MyNat_u) (ds_d5SL_p : MyNat_wf ds_d5SL ∧ True) (m : MyNat_u) (m_p : MyNat_wf m ∧ True):
-  plus_rel ds_d5SL m ⌊ plus (exist _ ds_d5SL ds_d5SL_p) (exist _ m m_p) -⌋.
+  (ds_d5Tw : MyNat_u) (ds_d5Tw_p : MyNat_wf ds_d5Tw ∧ True) (m : MyNat_u) (m_p : MyNat_wf m ∧ True):
+  plus_rel ds_d5Tw m ⌊ plus (exist _ ds_d5Tw ds_d5Tw_p) (exist _ m m_p) -⌋.
 Proof.
   Opaque plus.
   existence_lemma_pre plus;
-  try revert m_p; generalize dependent m; induction ds_d5SL as [| n' IH_n']; intros;
+  try revert m_p; generalize dependent m; induction ds_d5Tw as [| n' IH_n']; intros;
   [fix_notations |
    fix_notations;
    pose proof (IH_n' ltac:(try clear IH_n'; solver) m ltac:(try clear IH_n'; solver)) as IH_47989236;
@@ -3217,12 +3266,12 @@ Qed.
 #[global] Opaque plus.
 
 Theorem plus__plus_rel_rw
-  (ds_d5SL : MyNat_u)
-  (ds_d5SL_p : MyNat_wf ds_d5SL ∧ True)
+  (ds_d5Tw : MyNat_u)
+  (ds_d5Tw_p : MyNat_wf ds_d5Tw ∧ True)
   (m : MyNat_u)
   (m_p : MyNat_wf m ∧ True)
   (VV : MyNat_u):
-  ⌊ plus (exist _ ds_d5SL ds_d5SL_p) (exist _ m m_p) -⌋ = VV ↔ plus_rel ds_d5SL m VV.
+  ⌊ plus (exist _ ds_d5Tw ds_d5Tw_p) (exist _ m m_p) -⌋ = VV ↔ plus_rel ds_d5Tw m VV.
 Proof.
   f__f_rel_rw.
 Qed.
@@ -3233,31 +3282,31 @@ Qed.
 
 #[global] Instance plus_lookup_rw: dictionary rwLem plus := { lookup' := plus__plus_rel_rw }.
 
-Theorem plus__plus_rel (ds_d5SL m : MyNat) (VV : MyNat_u):
-  ⌊ plus ds_d5SL m -⌋ = VV ↔ plus_rel ⌊ ds_d5SL ⌋ ⌊ m ⌋ VV.
+Theorem plus__plus_rel (ds_d5Tw m : MyNat) (VV : MyNat_u):
+  ⌊ plus ds_d5Tw m -⌋ = VV ↔ plus_rel ⌊ ds_d5Tw ⌋ ⌊ m ⌋ VV.
 Proof.
   f__f_rel.
 Qed.
 
 #[global] Hint Rewrite plus__plus_rel: f_rel_funct_db.
 
-Theorem plus__plus_rel' (ds_d5SL_u m_u : MyNat_u) (ds_d5SL m : MyNat) (VV : MyNat_u):
-  ds_d5SL_u = ⌊ ds_d5SL ⌋ → (m_u = ⌊ m ⌋ → ⌊ plus ds_d5SL m -⌋ = VV ↔ plus_rel ds_d5SL_u m_u VV).
+Theorem plus__plus_rel' (ds_d5Tw_u m_u : MyNat_u) (ds_d5Tw m : MyNat) (VV : MyNat_u):
+  ds_d5Tw_u = ⌊ ds_d5Tw ⌋ → (m_u = ⌊ m ⌋ → ⌊ plus ds_d5Tw m -⌋ = VV ↔ plus_rel ds_d5Tw_u m_u VV).
 Proof.
-  intros -> ->. refine (plus__plus_rel ds_d5SL m VV).
+  intros -> ->. refine (plus__plus_rel ds_d5Tw m VV).
 Qed.
 
 #[global] Hint Resolve plus__plus_rel': f_rel_funct_db.
 
 Theorem plus_rel_mk
-  (ds_d5SL : MyNat_u) (ds_d5SL_p : MyNat_wf ds_d5SL ∧ True) (m : MyNat_u) (m_p : MyNat_wf m ∧ True):
-  {VV: _ | plus_rel ds_d5SL m VV}.
+  (ds_d5Tw : MyNat_u) (ds_d5Tw_p : MyNat_wf ds_d5Tw ∧ True) (m : MyNat_u) (m_p : MyNat_wf m ∧ True):
+  {VV: _ | plus_rel ds_d5Tw m VV}.
 Proof.
   intros;
   refine (subsumptionCast
           _
-          (λ VV, plus_rel ds_d5SL m VV)
-          (plus (exist _ ds_d5SL ds_d5SL_p) (exist _ m m_p))
+          (λ VV, plus_rel ds_d5Tw m VV)
+          (plus (exist _ ds_d5Tw ds_d5Tw_p) (exist _ m m_p))
           _);
   rewrite <- plus__plus_rel';
   quicksolve.
@@ -3267,13 +3316,13 @@ Qed.
 
 #[global] Instance plus_pack:
   @Pack
-  (MyNat ::RT λ (ds_d5SL : MyNat), MyNat ::RT λ (m : MyNat), nilRT)
+  (MyNat ::RT λ (ds_d5Tw : MyNat), MyNat ::RT λ (m : MyNat), nilRT)
   (MyNat_u ::UT (MyNat_u ::UT nilUT))
-  ltac:(mkProjectsArgListTG (MyNat ::RT λ (ds_d5SL : MyNat), MyNat ::RT λ (m : MyNat), nilRT) ((MyNat_u ::UT (MyNat_u ::UT nilUT))))
+  ltac:(mkProjectsArgListTG (MyNat ::RT λ (ds_d5Tw : MyNat), MyNat ::RT λ (m : MyNat), nilRT) ((MyNat_u ::UT (MyNat_u ::UT nilUT))))
   MyNat_u
-  (λ (x_28417923 : ArgList (MyNat ::RT λ (ds_d5SL : MyNat), MyNat ::RT λ (m : MyNat), nilRT))
-     (v_x_28417923 : MyNat_u),
-   ltac:(flattenP (λ (ds_d5SL m : MyNat) (VV : MyNat_u), MyNat_wf VV ∧ True) x_28417923 v_x_28417923)).
+  (λ (x_33049879 : ArgList (MyNat ::RT λ (ds_d5Tw : MyNat), MyNat ::RT λ (m : MyNat), nilRT))
+     (v_x_33049879 : MyNat_u),
+   ltac:(flattenP (λ (ds_d5Tw m : MyNat) (VV : MyNat_u), MyNat_wf VV ∧ True) x_33049879 v_x_33049879)).
 Proof.
   buildPackG plus plus_rel plus__plus_rel plus_rel_funct.
 Defined.
@@ -3283,15 +3332,15 @@ Proof.
   buildUPackG plus_rel plus_rel_funct.
 Defined.
 
-Definition add_0_r_spec (ds_d5Rj : MyNat): Type :=
-  {{∃ (plus_res : MyNat_u), plus_rel ⌊ ds_d5Rj -⌋ O_u plus_res ∧ plus_res == ⌊ ds_d5Rj -⌋}}.
+Definition add_0_r_spec (ds_d5S4 : MyNat): Type :=
+  {{∃ (plus_res : MyNat_u), plus_rel ⌊ ds_d5S4 -⌋ O_u plus_res ∧ plus_res == ⌊ ds_d5S4 -⌋}}.
 
 #[global] Hint Unfold add_0_r_spec: lia_unfold.
 
-Theorem add_0_r (ds_d5Rj : MyNat): add_0_r_spec ds_d5Rj.
+Theorem add_0_r (ds_d5S4 : MyNat): add_0_r_spec ds_d5S4.
 Proof.
-  destruct ds_d5Rj as [ds_d5Rj ds_d5Rj_p].
-  induction ds_d5Rj as [| n' IH_n'].
+  destruct ds_d5S4 as [ds_d5S4 ds_d5S4_p].
+  induction ds_d5S4 as [| n' IH_n'].
   - refine (subsumptionCast
             Unit
             (λ (VV : Unit), ∃ (plus_res : MyNat_u), plus_rel O_u O_u plus_res ∧ plus_res == O_u)
@@ -3304,110 +3353,110 @@ Proof.
             ltac:(solver)).
 Qed.
 
-Definition add_assoc_spec (ds_d5Sk ds_d5Sl ds_d5Sm : MyNat): Type :=
+Definition add_assoc_spec (ds_d5T5 ds_d5T6 ds_d5T7 : MyNat): Type :=
   {{∃ (plus_res : MyNat_u),
-    plus_rel ⌊ ds_d5Sl -⌋ ⌊ ds_d5Sm -⌋ plus_res
+    plus_rel ⌊ ds_d5T6 -⌋ ⌊ ds_d5T7 -⌋ plus_res
     ∧ ∃ (plus_res_2 : MyNat_u),
-      plus_rel ⌊ ds_d5Sk -⌋ plus_res plus_res_2
+      plus_rel ⌊ ds_d5T5 -⌋ plus_res plus_res_2
       ∧ ∃ (plus_res_3 : MyNat_u),
-        plus_rel ⌊ ds_d5Sk -⌋ ⌊ ds_d5Sl -⌋ plus_res_3
+        plus_rel ⌊ ds_d5T5 -⌋ ⌊ ds_d5T6 -⌋ plus_res_3
         ∧ ∃ (plus_res_4 : MyNat_u),
-          plus_rel plus_res_3 ⌊ ds_d5Sm -⌋ plus_res_4 ∧ plus_res_2 == plus_res_4}}.
+          plus_rel plus_res_3 ⌊ ds_d5T7 -⌋ plus_res_4 ∧ plus_res_2 == plus_res_4}}.
 
 #[global] Hint Unfold add_assoc_spec: lia_unfold.
 
-Theorem add_assoc (ds_d5Sk ds_d5Sl ds_d5Sm : MyNat): add_assoc_spec ds_d5Sk ds_d5Sl ds_d5Sm.
+Theorem add_assoc (ds_d5T5 ds_d5T6 ds_d5T7 : MyNat): add_assoc_spec ds_d5T5 ds_d5T6 ds_d5T7.
 Proof.
-  destruct ds_d5Sk as [ds_d5Sk ds_d5Sk_p].
-  destruct ds_d5Sl as [ds_d5Sl ds_d5Sl_p].
-  destruct ds_d5Sm as [ds_d5Sm ds_d5Sm_p].
-  try revert ds_d5Sm_p; generalize dependent ds_d5Sm;
-  try revert ds_d5Sl_p; generalize dependent ds_d5Sl;
-  induction ds_d5Sk as [| n' IH_n'];
+  destruct ds_d5T5 as [ds_d5T5 ds_d5T5_p].
+  destruct ds_d5T6 as [ds_d5T6 ds_d5T6_p].
+  destruct ds_d5T7 as [ds_d5T7 ds_d5T7_p].
+  try revert ds_d5T7_p; generalize dependent ds_d5T7;
+  try revert ds_d5T6_p; generalize dependent ds_d5T6;
+  induction ds_d5T5 as [| n' IH_n'];
   intros.
   - refine (subsumptionCast
             Unit
             (λ (VV : Unit),
              ∃ (plus_res : MyNat_u),
-             plus_rel ds_d5Sl ds_d5Sm plus_res
+             plus_rel ds_d5T6 ds_d5T7 plus_res
              ∧ ∃ (plus_res_2 : MyNat_u),
                plus_rel O_u plus_res plus_res_2
                ∧ ∃ (plus_res_3 : MyNat_u),
-                 plus_rel O_u ds_d5Sl plus_res_3
-                 ∧ ∃ (plus_res_4 : MyNat_u), plus_rel plus_res_3 ds_d5Sm plus_res_4 ∧ plus_res_2 == plus_res_4)
+                 plus_rel O_u ds_d5T6 plus_res_3
+                 ∧ ∃ (plus_res_4 : MyNat_u), plus_rel plus_res_3 ds_d5T7 plus_res_4 ∧ plus_res_2 == plus_res_4)
             (# unit)
             ltac:(solver)).
   - refine (subsumptionCast
             Unit
             (λ (VV : Unit),
              ∃ (plus_res : MyNat_u),
-             plus_rel ds_d5Sl ds_d5Sm plus_res
+             plus_rel ds_d5T6 ds_d5T7 plus_res
              ∧ ∃ (plus_res_2 : MyNat_u),
                plus_rel (S_u n') plus_res plus_res_2
                ∧ ∃ (plus_res_3 : MyNat_u),
-                 plus_rel (S_u n') ds_d5Sl plus_res_3
-                 ∧ ∃ (plus_res_4 : MyNat_u), plus_rel plus_res_3 ds_d5Sm plus_res_4 ∧ plus_res_2 == plus_res_4)
+                 plus_rel (S_u n') ds_d5T6 plus_res_3
+                 ∧ ∃ (plus_res_4 : MyNat_u), plus_rel plus_res_3 ds_d5T7 plus_res_4 ∧ plus_res_2 == plus_res_4)
             (IH_n'
              ltac:(try clear IH_n'; solver)
-             ds_d5Sl
+             ds_d5T6
              ltac:(try clear IH_n'; solver)
-             ds_d5Sm
+             ds_d5T7
              ltac:(try clear IH_n'; solver))
             ltac:(solver)).
 Qed.
 
-Definition add_succ_r_spec (ds_d5Sn ds_d5So : MyNat): Type :=
+Definition add_succ_r_spec (ds_d5T8 ds_d5T9 : MyNat): Type :=
   {{∃ (plus_res : MyNat_u),
-    plus_rel ⌊ ds_d5Sn -⌋ (S_u ⌊ ds_d5So -⌋) plus_res
+    plus_rel ⌊ ds_d5T8 -⌋ (S_u ⌊ ds_d5T9 -⌋) plus_res
     ∧ ∃ (plus_res_2 : MyNat_u),
-      plus_rel ⌊ ds_d5Sn -⌋ ⌊ ds_d5So -⌋ plus_res_2 ∧ plus_res == S_u plus_res_2}}.
+      plus_rel ⌊ ds_d5T8 -⌋ ⌊ ds_d5T9 -⌋ plus_res_2 ∧ plus_res == S_u plus_res_2}}.
 
 #[global] Hint Unfold add_succ_r_spec: lia_unfold.
 
-Theorem add_succ_r (ds_d5Sn ds_d5So : MyNat): add_succ_r_spec ds_d5Sn ds_d5So.
+Theorem add_succ_r (ds_d5T8 ds_d5T9 : MyNat): add_succ_r_spec ds_d5T8 ds_d5T9.
 Proof.
-  destruct ds_d5Sn as [ds_d5Sn ds_d5Sn_p].
-  destruct ds_d5So as [ds_d5So ds_d5So_p].
-  try revert ds_d5So_p; generalize dependent ds_d5So; induction ds_d5Sn as [| n' IH_n']; intros.
+  destruct ds_d5T8 as [ds_d5T8 ds_d5T8_p].
+  destruct ds_d5T9 as [ds_d5T9 ds_d5T9_p].
+  try revert ds_d5T9_p; generalize dependent ds_d5T9; induction ds_d5T8 as [| n' IH_n']; intros.
   - refine (subsumptionCast
             Unit
             (λ (VV : Unit),
              ∃ (plus_res : MyNat_u),
-             plus_rel O_u (S_u ds_d5So) plus_res
-             ∧ ∃ (plus_res_2 : MyNat_u), plus_rel O_u ds_d5So plus_res_2 ∧ plus_res == S_u plus_res_2)
+             plus_rel O_u (S_u ds_d5T9) plus_res
+             ∧ ∃ (plus_res_2 : MyNat_u), plus_rel O_u ds_d5T9 plus_res_2 ∧ plus_res == S_u plus_res_2)
             (# unit)
             ltac:(solver)).
   - refine (subsumptionCast
             Unit
             (λ (VV : Unit),
              ∃ (plus_res : MyNat_u),
-             plus_rel (S_u n') (S_u ds_d5So) plus_res
-             ∧ ∃ (plus_res_2 : MyNat_u), plus_rel (S_u n') ds_d5So plus_res_2 ∧ plus_res == S_u plus_res_2)
-            (IH_n' ltac:(try clear IH_n'; solver) ds_d5So ltac:(try clear IH_n'; solver))
+             plus_rel (S_u n') (S_u ds_d5T9) plus_res
+             ∧ ∃ (plus_res_2 : MyNat_u), plus_rel (S_u n') ds_d5T9 plus_res_2 ∧ plus_res == S_u plus_res_2)
+            (IH_n' ltac:(try clear IH_n'; solver) ds_d5T9 ltac:(try clear IH_n'; solver))
             ltac:(solver)).
 Qed.
 
-Definition mult_spec (ds_d5SN ds_d5SO : MyNat): Type :=
+Definition mult_spec (ds_d5Ty ds_d5Tz : MyNat): Type :=
   MyNat.
 
 #[global] Hint Unfold mult_spec: lia_unfold.
 
-Definition mult (ds_d5SN ds_d5SO : MyNat): mult_spec ds_d5SN ds_d5SO.
+Definition mult (ds_d5Ty ds_d5Tz : MyNat): mult_spec ds_d5Ty ds_d5Tz.
 Proof.
-  destruct ds_d5SN as [ds_d5SN ds_d5SN_p].
-  destruct ds_d5SO as [ds_d5SO ds_d5SO_p].
-  try revert ds_d5SO_p; generalize dependent ds_d5SO; induction ds_d5SN as [| n' IH_n']; intros.
+  destruct ds_d5Ty as [ds_d5Ty ds_d5Ty_p].
+  destruct ds_d5Tz as [ds_d5Tz ds_d5Tz_p].
+  try revert ds_d5Tz_p; generalize dependent ds_d5Tz; induction ds_d5Ty as [| n' IH_n']; intros.
   - refine O.
   - refine (plus
-            (exist (λ (ds_d5SO : MyNat_u), MyNat_wf ds_d5SO ∧ True) ds_d5SO ltac:(solver))
-            (IH_n' ltac:(try clear IH_n'; solver) ds_d5SO ltac:(try clear IH_n'; solver))).
+            (exist (λ (ds_d5Tz : MyNat_u), MyNat_wf ds_d5Tz ∧ True) ds_d5Tz ltac:(solver))
+            (IH_n' ltac:(try clear IH_n'; solver) ds_d5Tz ltac:(try clear IH_n'; solver))).
 Defined.
 
 Inductive mult_rel: MyNat_u → MyNat_u → MyNat_u → Prop :=
-  | mult_O_x: ∀ ds_d5SO, mult_rel O_u ds_d5SO O_u
-  | mult_S_x: ∀ n' ds_d5SO (mult_res : MyNat_u),
-              mult_rel n' ds_d5SO mult_res
-              → ∀ (plus_res : MyNat_u), plus_rel ds_d5SO mult_res plus_res → mult_rel (S_u n') ds_d5SO plus_res.
+  | mult_O_x: ∀ ds_d5Tz, mult_rel O_u ds_d5Tz O_u
+  | mult_S_x: ∀ n' ds_d5Tz (mult_res : MyNat_u),
+              mult_rel n' ds_d5Tz mult_res
+              → ∀ (plus_res : MyNat_u), plus_rel ds_d5Tz mult_res plus_res → mult_rel (S_u n') ds_d5Tz plus_res.
 
 #[global] Hint Constructors mult_rel: core_hint_db.
 
@@ -3415,10 +3464,10 @@ Inductive mult_rel: MyNat_u → MyNat_u → MyNat_u → Prop :=
 
 #[global] Instance mult_getF: getFunc mult_rel := { getF' := mult }.
 
-Theorem mult_rel_funct [ds_d5SN ds_d5SO : MyNat_u]:
-  ∀ (VV VV' : MyNat_u), mult_rel ds_d5SN ds_d5SO VV → (mult_rel ds_d5SN ds_d5SO VV' → VV = VV').
+Theorem mult_rel_funct [ds_d5Ty ds_d5Tz : MyNat_u]:
+  ∀ (VV VV' : MyNat_u), mult_rel ds_d5Ty ds_d5Tz VV → (mult_rel ds_d5Ty ds_d5Tz VV' → VV = VV').
 Proof.
-  try revert ds_d5SO_p; generalize dependent ds_d5SO; induction ds_d5SN as [| n' IH_n']; intros;
+  try revert ds_d5Tz_p; generalize dependent ds_d5Tz; induction ds_d5Ty as [| n' IH_n']; intros;
   rel_functionhood_body.
 Qed.
 
@@ -3427,19 +3476,19 @@ Qed.
 #[global] Instance mult_lookup_funct: dictionary functionhood mult := {
     lookup' := mult_rel_funct }.
 
-Theorem mult_O_x_lem ds_d5SO mult_O_x_lem_res:
-  mult_rel O_u ds_d5SO mult_O_x_lem_res ↔ mult_O_x_lem_res == O_u.
+Theorem mult_O_x_lem ds_d5Tz mult_O_x_lem_res:
+  mult_rel O_u ds_d5Tz mult_O_x_lem_res ↔ mult_O_x_lem_res == O_u.
 Proof.
   rel_back' _nil.
 Qed.
 
 #[global] Hint Rewrite mult_O_x_lem: f_rel_back.
 
-Theorem mult_S_x_lem ds_d5SO n' mult_S_x_lem_res:
-  mult_rel (S_u n') ds_d5SO mult_S_x_lem_res
+Theorem mult_S_x_lem ds_d5Tz n' mult_S_x_lem_res:
+  mult_rel (S_u n') ds_d5Tz mult_S_x_lem_res
   ↔ ∃ (mult_res : MyNat_u),
-    mult_rel n' ds_d5SO mult_res
-    ∧ ∃ (plus_res : MyNat_u), plus_rel ds_d5SO mult_res plus_res ∧ mult_S_x_lem_res == plus_res.
+    mult_rel n' ds_d5Tz mult_res
+    ∧ ∃ (plus_res : MyNat_u), plus_rel ds_d5Tz mult_res plus_res ∧ mult_S_x_lem_res == plus_res.
 Proof.
   rel_back' _nil.
 Qed.
@@ -3447,21 +3496,21 @@ Qed.
 #[global] Hint Rewrite mult_S_x_lem: f_rel_back.
 
 Theorem mult_rel_ex
-  (ds_d5SN : MyNat_u)
-  (ds_d5SN_p : MyNat_wf ds_d5SN ∧ True)
-  (ds_d5SO : MyNat_u)
-  (ds_d5SO_p : MyNat_wf ds_d5SO ∧ True):
-  mult_rel ds_d5SN ds_d5SO ⌊ mult (exist _ ds_d5SN ds_d5SN_p) (exist _ ds_d5SO ds_d5SO_p) -⌋.
+  (ds_d5Ty : MyNat_u)
+  (ds_d5Ty_p : MyNat_wf ds_d5Ty ∧ True)
+  (ds_d5Tz : MyNat_u)
+  (ds_d5Tz_p : MyNat_wf ds_d5Tz ∧ True):
+  mult_rel ds_d5Ty ds_d5Tz ⌊ mult (exist _ ds_d5Ty ds_d5Ty_p) (exist _ ds_d5Tz ds_d5Tz_p) -⌋.
 Proof.
   Opaque mult.
   existence_lemma_pre mult;
-  try revert ds_d5SO_p; generalize dependent ds_d5SO; induction ds_d5SN as [| n' IH_n']; intros;
+  try revert ds_d5Tz_p; generalize dependent ds_d5Tz; induction ds_d5Ty as [| n' IH_n']; intros;
   [fix_notations |
    fix_notations;
    pose proof (IH_n'
                ltac:(try clear IH_n'; solver)
-               ds_d5SO
-               ltac:(try clear IH_n'; solver)) as IH_92617003;
+               ds_d5Tz
+               ltac:(try clear IH_n'; solver)) as IH_91299355;
    try clear IH_n'];
   simpl in *.
   Transparent mult.
@@ -3473,13 +3522,13 @@ Qed.
 #[global] Opaque mult.
 
 Theorem mult__mult_rel_rw
-  (ds_d5SN : MyNat_u)
-  (ds_d5SN_p : MyNat_wf ds_d5SN ∧ True)
-  (ds_d5SO : MyNat_u)
-  (ds_d5SO_p : MyNat_wf ds_d5SO ∧ True)
+  (ds_d5Ty : MyNat_u)
+  (ds_d5Ty_p : MyNat_wf ds_d5Ty ∧ True)
+  (ds_d5Tz : MyNat_u)
+  (ds_d5Tz_p : MyNat_wf ds_d5Tz ∧ True)
   (VV : MyNat_u):
-  ⌊ mult (exist _ ds_d5SN ds_d5SN_p) (exist _ ds_d5SO ds_d5SO_p) -⌋ = VV
-  ↔ mult_rel ds_d5SN ds_d5SO VV.
+  ⌊ mult (exist _ ds_d5Ty ds_d5Ty_p) (exist _ ds_d5Tz ds_d5Tz_p) -⌋ = VV
+  ↔ mult_rel ds_d5Ty ds_d5Tz VV.
 Proof.
   f__f_rel_rw.
 Qed.
@@ -3490,35 +3539,35 @@ Qed.
 
 #[global] Instance mult_lookup_rw: dictionary rwLem mult := { lookup' := mult__mult_rel_rw }.
 
-Theorem mult__mult_rel (ds_d5SN ds_d5SO : MyNat) (VV : MyNat_u):
-  ⌊ mult ds_d5SN ds_d5SO -⌋ = VV ↔ mult_rel ⌊ ds_d5SN ⌋ ⌊ ds_d5SO ⌋ VV.
+Theorem mult__mult_rel (ds_d5Ty ds_d5Tz : MyNat) (VV : MyNat_u):
+  ⌊ mult ds_d5Ty ds_d5Tz -⌋ = VV ↔ mult_rel ⌊ ds_d5Ty ⌋ ⌊ ds_d5Tz ⌋ VV.
 Proof.
   f__f_rel.
 Qed.
 
 #[global] Hint Rewrite mult__mult_rel: f_rel_funct_db.
 
-Theorem mult__mult_rel' (ds_d5SN_u ds_d5SO_u : MyNat_u) (ds_d5SN ds_d5SO : MyNat) (VV : MyNat_u):
-  ds_d5SN_u = ⌊ ds_d5SN ⌋
-  → (ds_d5SO_u = ⌊ ds_d5SO ⌋ → ⌊ mult ds_d5SN ds_d5SO -⌋ = VV ↔ mult_rel ds_d5SN_u ds_d5SO_u VV).
+Theorem mult__mult_rel' (ds_d5Ty_u ds_d5Tz_u : MyNat_u) (ds_d5Ty ds_d5Tz : MyNat) (VV : MyNat_u):
+  ds_d5Ty_u = ⌊ ds_d5Ty ⌋
+  → (ds_d5Tz_u = ⌊ ds_d5Tz ⌋ → ⌊ mult ds_d5Ty ds_d5Tz -⌋ = VV ↔ mult_rel ds_d5Ty_u ds_d5Tz_u VV).
 Proof.
-  intros -> ->. refine (mult__mult_rel ds_d5SN ds_d5SO VV).
+  intros -> ->. refine (mult__mult_rel ds_d5Ty ds_d5Tz VV).
 Qed.
 
 #[global] Hint Resolve mult__mult_rel': f_rel_funct_db.
 
 Theorem mult_rel_mk
-  (ds_d5SN : MyNat_u)
-  (ds_d5SN_p : MyNat_wf ds_d5SN ∧ True)
-  (ds_d5SO : MyNat_u)
-  (ds_d5SO_p : MyNat_wf ds_d5SO ∧ True):
-  {VV: _ | mult_rel ds_d5SN ds_d5SO VV}.
+  (ds_d5Ty : MyNat_u)
+  (ds_d5Ty_p : MyNat_wf ds_d5Ty ∧ True)
+  (ds_d5Tz : MyNat_u)
+  (ds_d5Tz_p : MyNat_wf ds_d5Tz ∧ True):
+  {VV: _ | mult_rel ds_d5Ty ds_d5Tz VV}.
 Proof.
   intros;
   refine (subsumptionCast
           _
-          (λ VV, mult_rel ds_d5SN ds_d5SO VV)
-          (mult (exist _ ds_d5SN ds_d5SN_p) (exist _ ds_d5SO ds_d5SO_p))
+          (λ VV, mult_rel ds_d5Ty ds_d5Tz VV)
+          (mult (exist _ ds_d5Ty ds_d5Ty_p) (exist _ ds_d5Tz ds_d5Tz_p))
           _);
   rewrite <- mult__mult_rel';
   quicksolve.
@@ -3528,14 +3577,14 @@ Qed.
 
 #[global] Instance mult_pack:
   @Pack
-  (MyNat ::RT λ (ds_d5SN : MyNat), MyNat ::RT λ (ds_d5SO : MyNat), nilRT)
+  (MyNat ::RT λ (ds_d5Ty : MyNat), MyNat ::RT λ (ds_d5Tz : MyNat), nilRT)
   (MyNat_u ::UT (MyNat_u ::UT nilUT))
   ltac:(mkProjectsArgListTG (MyNat
- ::RT λ (ds_d5SN : MyNat), MyNat ::RT λ (ds_d5SO : MyNat), nilRT) ((MyNat_u ::UT (MyNat_u ::UT nilUT))))
+ ::RT λ (ds_d5Ty : MyNat), MyNat ::RT λ (ds_d5Tz : MyNat), nilRT) ((MyNat_u ::UT (MyNat_u ::UT nilUT))))
   MyNat_u
-  (λ (x_49566504 : ArgList (MyNat ::RT λ (ds_d5SN : MyNat), MyNat ::RT λ (ds_d5SO : MyNat), nilRT))
-     (v_x_49566504 : MyNat_u),
-   ltac:(flattenP (λ (ds_d5SN ds_d5SO : MyNat) (VV : MyNat_u), MyNat_wf VV ∧ True) x_49566504 v_x_49566504)).
+  (λ (x_24892408 : ArgList (MyNat ::RT λ (ds_d5Ty : MyNat), MyNat ::RT λ (ds_d5Tz : MyNat), nilRT))
+     (v_x_24892408 : MyNat_u),
+   ltac:(flattenP (λ (ds_d5Ty ds_d5Tz : MyNat) (VV : MyNat_u), MyNat_wf VV ∧ True) x_24892408 v_x_24892408)).
 Proof.
   buildPackG mult mult_rel mult__mult_rel mult_rel_funct.
 Defined.
@@ -3545,15 +3594,15 @@ Proof.
   buildUPackG mult_rel mult_rel_funct.
 Defined.
 
-Definition factorial_spec (ds_d5SS : MyNat): Type :=
+Definition factorial_spec (ds_d5TD : MyNat): Type :=
   MyNat.
 
 #[global] Hint Unfold factorial_spec: lia_unfold.
 
-Definition factorial (ds_d5SS : MyNat): factorial_spec ds_d5SS.
+Definition factorial (ds_d5TD : MyNat): factorial_spec ds_d5TD.
 Proof.
-  destruct ds_d5SS as [ds_d5SS ds_d5SS_p].
-  induction ds_d5SS as [| n' IH_n'].
+  destruct ds_d5TD as [ds_d5TD ds_d5TD_p].
+  induction ds_d5TD as [| n' IH_n'].
   - refine (S O).
   - refine (mult
             (S (exist (λ (VV : MyNat_u), MyNat_wf VV ∧ True) n' ltac:(solver)))
@@ -3573,10 +3622,10 @@ Inductive factorial_rel: MyNat_u → MyNat_u → Prop :=
 
 #[global] Instance factorial_getF: getFunc factorial_rel := { getF' := factorial }.
 
-Theorem factorial_rel_funct [ds_d5SS : MyNat_u]:
-  ∀ (VV VV' : MyNat_u), factorial_rel ds_d5SS VV → (factorial_rel ds_d5SS VV' → VV = VV').
+Theorem factorial_rel_funct [ds_d5TD : MyNat_u]:
+  ∀ (VV VV' : MyNat_u), factorial_rel ds_d5TD VV → (factorial_rel ds_d5TD VV' → VV = VV').
 Proof.
-  induction ds_d5SS as [| n' IH_n']; rel_functionhood_body.
+  induction ds_d5TD as [| n' IH_n']; rel_functionhood_body.
 Qed.
 
 #[global] Hint Resolve factorial_rel_funct: f_rel_funct_db.
@@ -3604,12 +3653,12 @@ Qed.
 
 #[global] Hint Rewrite factorial_S_lem: f_rel_back.
 
-Theorem factorial_rel_ex (ds_d5SS : MyNat_u) (ds_d5SS_p : MyNat_wf ds_d5SS ∧ True):
-  factorial_rel ds_d5SS ⌊ factorial (exist _ ds_d5SS ds_d5SS_p) -⌋.
+Theorem factorial_rel_ex (ds_d5TD : MyNat_u) (ds_d5TD_p : MyNat_wf ds_d5TD ∧ True):
+  factorial_rel ds_d5TD ⌊ factorial (exist _ ds_d5TD ds_d5TD_p) -⌋.
 Proof.
   Opaque factorial.
   existence_lemma_pre factorial;
-  induction ds_d5SS as [| n' IH_n'];
+  induction ds_d5TD as [| n' IH_n'];
   [fix_notations |
    fix_notations; pose proof (IH_n' ltac:(try clear IH_n'; solver)) as IH_36186333; try clear IH_n'];
   simpl in *.
@@ -3622,8 +3671,8 @@ Qed.
 #[global] Opaque factorial.
 
 Theorem factorial__factorial_rel_rw
-  (ds_d5SS : MyNat_u) (ds_d5SS_p : MyNat_wf ds_d5SS ∧ True) (VV : MyNat_u):
-  ⌊ factorial (exist _ ds_d5SS ds_d5SS_p) -⌋ = VV ↔ factorial_rel ds_d5SS VV.
+  (ds_d5TD : MyNat_u) (ds_d5TD_p : MyNat_wf ds_d5TD ∧ True) (VV : MyNat_u):
+  ⌊ factorial (exist _ ds_d5TD ds_d5TD_p) -⌋ = VV ↔ factorial_rel ds_d5TD VV.
 Proof.
   f__f_rel_rw.
 Qed.
@@ -3635,30 +3684,30 @@ Qed.
 #[global] Instance factorial_lookup_rw: dictionary rwLem factorial := {
     lookup' := factorial__factorial_rel_rw }.
 
-Theorem factorial__factorial_rel (ds_d5SS : MyNat) (VV : MyNat_u):
-  ⌊ factorial ds_d5SS -⌋ = VV ↔ factorial_rel ⌊ ds_d5SS ⌋ VV.
+Theorem factorial__factorial_rel (ds_d5TD : MyNat) (VV : MyNat_u):
+  ⌊ factorial ds_d5TD -⌋ = VV ↔ factorial_rel ⌊ ds_d5TD ⌋ VV.
 Proof.
   f__f_rel.
 Qed.
 
 #[global] Hint Rewrite factorial__factorial_rel: f_rel_funct_db.
 
-Theorem factorial__factorial_rel' (ds_d5SS_u : MyNat_u) (ds_d5SS : MyNat) (VV : MyNat_u):
-  ds_d5SS_u = ⌊ ds_d5SS ⌋ → ⌊ factorial ds_d5SS -⌋ = VV ↔ factorial_rel ds_d5SS_u VV.
+Theorem factorial__factorial_rel' (ds_d5TD_u : MyNat_u) (ds_d5TD : MyNat) (VV : MyNat_u):
+  ds_d5TD_u = ⌊ ds_d5TD ⌋ → ⌊ factorial ds_d5TD -⌋ = VV ↔ factorial_rel ds_d5TD_u VV.
 Proof.
-  intros ->. refine (factorial__factorial_rel ds_d5SS VV).
+  intros ->. refine (factorial__factorial_rel ds_d5TD VV).
 Qed.
 
 #[global] Hint Resolve factorial__factorial_rel': f_rel_funct_db.
 
-Theorem factorial_rel_mk (ds_d5SS : MyNat_u) (ds_d5SS_p : MyNat_wf ds_d5SS ∧ True):
-  {VV: _ | factorial_rel ds_d5SS VV}.
+Theorem factorial_rel_mk (ds_d5TD : MyNat_u) (ds_d5TD_p : MyNat_wf ds_d5TD ∧ True):
+  {VV: _ | factorial_rel ds_d5TD VV}.
 Proof.
   intros;
   refine (subsumptionCast
           _
-          (λ VV, factorial_rel ds_d5SS VV)
-          (factorial (exist _ ds_d5SS ds_d5SS_p))
+          (λ VV, factorial_rel ds_d5TD VV)
+          (factorial (exist _ ds_d5TD ds_d5TD_p))
           _);
   rewrite <- factorial__factorial_rel';
   quicksolve.
@@ -3668,12 +3717,12 @@ Qed.
 
 #[global] Instance factorial_pack:
   @Pack
-  (MyNat ::RT λ (ds_d5SS : MyNat), nilRT)
+  (MyNat ::RT λ (ds_d5TD : MyNat), nilRT)
   (MyNat_u ::UT nilUT)
-  ltac:(mkProjectsArgListTG (MyNat ::RT λ (ds_d5SS : MyNat), nilRT) ((MyNat_u ::UT nilUT)))
+  ltac:(mkProjectsArgListTG (MyNat ::RT λ (ds_d5TD : MyNat), nilRT) ((MyNat_u ::UT nilUT)))
   MyNat_u
-  (λ (x_45728972 : ArgList (MyNat ::RT λ (ds_d5SS : MyNat), nilRT)) (v_x_45728972 : MyNat_u),
-   ltac:(flattenP (λ (ds_d5SS : MyNat) (VV : MyNat_u), MyNat_wf VV ∧ True) x_45728972 v_x_45728972)).
+  (λ (x_50130673 : ArgList (MyNat ::RT λ (ds_d5TD : MyNat), nilRT)) (v_x_50130673 : MyNat_u),
+   ltac:(flattenP (λ (ds_d5TD : MyNat) (VV : MyNat_u), MyNat_wf VV ∧ True) x_50130673 v_x_50130673)).
 Proof.
   buildPackG factorial factorial_rel factorial__factorial_rel factorial_rel_funct.
 Defined.
@@ -3683,15 +3732,15 @@ Proof.
   buildUPackG factorial_rel factorial_rel_funct.
 Defined.
 
-Definition mul_0_r_spec (ds_d5Rh : MyNat): Type :=
-  {{∃ (mult_res : MyNat_u), mult_rel ⌊ ds_d5Rh -⌋ O_u mult_res ∧ mult_res == O_u}}.
+Definition mul_0_r_spec (ds_d5S2 : MyNat): Type :=
+  {{∃ (mult_res : MyNat_u), mult_rel ⌊ ds_d5S2 -⌋ O_u mult_res ∧ mult_res == O_u}}.
 
 #[global] Hint Unfold mul_0_r_spec: lia_unfold.
 
-Theorem mul_0_r (ds_d5Rh : MyNat): mul_0_r_spec ds_d5Rh.
+Theorem mul_0_r (ds_d5S2 : MyNat): mul_0_r_spec ds_d5S2.
 Proof.
-  destruct ds_d5Rh as [ds_d5Rh ds_d5Rh_p].
-  induction ds_d5Rh as [| n' IH_n'].
+  destruct ds_d5S2 as [ds_d5S2 ds_d5S2_p].
+  induction ds_d5S2 as [| n' IH_n'].
   - refine (subsumptionCast
             Unit
             (λ (VV : Unit), ∃ (mult_res : MyNat_u), mult_rel O_u O_u mult_res ∧ mult_res == O_u)
@@ -3719,15 +3768,15 @@ Proof.
           ltac:(solver)).
 Qed.
 
-Definition mult_n_O_spec (ds_d5Sp : MyNat): Type :=
-  {{∃ (mult_res : MyNat_u), mult_rel ⌊ ds_d5Sp -⌋ O_u mult_res ∧ O_u == mult_res}}.
+Definition mult_n_O_spec (ds_d5Ta : MyNat): Type :=
+  {{∃ (mult_res : MyNat_u), mult_rel ⌊ ds_d5Ta -⌋ O_u mult_res ∧ O_u == mult_res}}.
 
 #[global] Hint Unfold mult_n_O_spec: lia_unfold.
 
-Theorem mult_n_O (ds_d5Sp : MyNat): mult_n_O_spec ds_d5Sp.
+Theorem mult_n_O (ds_d5Ta : MyNat): mult_n_O_spec ds_d5Ta.
 Proof.
-  destruct ds_d5Sp as [ds_d5Sp ds_d5Sp_p].
-  induction ds_d5Sp as [| n' IH_n'].
+  destruct ds_d5Ta as [ds_d5Ta ds_d5Ta_p].
+  induction ds_d5Ta as [| n' IH_n'].
   - refine (subsumptionCast
             Unit
             (λ (VV : Unit), ∃ (mult_res : MyNat_u), mult_rel O_u O_u mult_res ∧ O_u == mult_res)
@@ -3768,69 +3817,69 @@ Proof.
           ltac:(solver)).
 Qed.
 
-Definition mult_n_Sm_spec (ds_d5SV ds_d5SW : MyNat): Type :=
+Definition mult_n_Sm_spec (ds_d5TG ds_d5TH : MyNat): Type :=
   {{∃ (mult_res : MyNat_u),
-    mult_rel ⌊ ds_d5SV -⌋ ⌊ ds_d5SW -⌋ mult_res
+    mult_rel ⌊ ds_d5TG -⌋ ⌊ ds_d5TH -⌋ mult_res
     ∧ ∃ (plus_res : MyNat_u),
-      plus_rel mult_res ⌊ ds_d5SV -⌋ plus_res
+      plus_rel mult_res ⌊ ds_d5TG -⌋ plus_res
       ∧ ∃ (mult_res_2 : MyNat_u),
-        mult_rel ⌊ ds_d5SV -⌋ (S_u ⌊ ds_d5SW -⌋) mult_res_2 ∧ plus_res == mult_res_2}}.
+        mult_rel ⌊ ds_d5TG -⌋ (S_u ⌊ ds_d5TH -⌋) mult_res_2 ∧ plus_res == mult_res_2}}.
 
 #[global] Hint Unfold mult_n_Sm_spec: lia_unfold.
 
-Theorem mult_n_Sm (ds_d5SV ds_d5SW : MyNat): mult_n_Sm_spec ds_d5SV ds_d5SW.
+Theorem mult_n_Sm (ds_d5TG ds_d5TH : MyNat): mult_n_Sm_spec ds_d5TG ds_d5TH.
 Proof.
-  destruct ds_d5SV as [ds_d5SV ds_d5SV_p].
-  destruct ds_d5SW as [ds_d5SW ds_d5SW_p].
-  try revert ds_d5SW_p; generalize dependent ds_d5SW; induction ds_d5SV as [| n' IH_n']; intros.
+  destruct ds_d5TG as [ds_d5TG ds_d5TG_p].
+  destruct ds_d5TH as [ds_d5TH ds_d5TH_p].
+  try revert ds_d5TH_p; generalize dependent ds_d5TH; induction ds_d5TG as [| n' IH_n']; intros.
   - refine (subsumptionCast
             Unit
             (λ (VV : Unit),
              ∃ (mult_res : MyNat_u),
-             mult_rel O_u ds_d5SW mult_res
+             mult_rel O_u ds_d5TH mult_res
              ∧ ∃ (plus_res : MyNat_u),
                plus_rel mult_res O_u plus_res
-               ∧ ∃ (mult_res_2 : MyNat_u), mult_rel O_u (S_u ds_d5SW) mult_res_2 ∧ plus_res == mult_res_2)
+               ∧ ∃ (mult_res_2 : MyNat_u), mult_rel O_u (S_u ds_d5TH) mult_res_2 ∧ plus_res == mult_res_2)
             (# unit)
             ltac:(solver)).
-  - try assert (ds_d5SW_inj_wit_60446462 : (λ (ds_d5SW : MyNat_u), MyNat_wf ds_d5SW ∧ True)
-                                           ds_d5SW) by (solver).
-    pose (exist (λ (ds_d5SW : MyNat_u),
-                 MyNat_wf ds_d5SW ∧ True) ds_d5SW ds_d5SW_inj_wit_60446462) as h_61136385_1.
+  - try assert (ds_d5TH_inj_wit_19375046 : (λ (ds_d5TH : MyNat_u), MyNat_wf ds_d5TH ∧ True)
+                                           ds_d5TH) by (solver).
+    pose (exist (λ (ds_d5TH : MyNat_u),
+                 MyNat_wf ds_d5TH ∧ True) ds_d5TH ds_d5TH_inj_wit_19375046) as h_76901889_1.
     try assert (VV_inj_wit_67733700 : (λ (VV : MyNat_u), MyNat_wf VV ∧ True) n') by (solver).
-    pose (exist (λ (VV : MyNat_u), MyNat_wf VV ∧ True) n' VV_inj_wit_67733700) as h_61136385_2_1.
-    try assert (ds_d5SW_inj_wit_60446462 : (λ (ds_d5SW : MyNat_u), MyNat_wf ds_d5SW ∧ True)
-                                           ds_d5SW) by (solver).
-    pose (exist (λ (ds_d5SW : MyNat_u),
-                 MyNat_wf ds_d5SW ∧ True) ds_d5SW ds_d5SW_inj_wit_60446462) as h_61136385_2_2.
-    pose (mult h_61136385_2_1 h_61136385_2_2) as h_61136385_2.
+    pose (exist (λ (VV : MyNat_u), MyNat_wf VV ∧ True) n' VV_inj_wit_67733700) as h_76901889_2_1.
+    try assert (ds_d5TH_inj_wit_19375046 : (λ (ds_d5TH : MyNat_u), MyNat_wf ds_d5TH ∧ True)
+                                           ds_d5TH) by (solver).
+    pose (exist (λ (ds_d5TH : MyNat_u),
+                 MyNat_wf ds_d5TH ∧ True) ds_d5TH ds_d5TH_inj_wit_19375046) as h_76901889_2_2.
+    pose (mult h_76901889_2_1 h_76901889_2_2) as h_76901889_2.
     try assert (VV_inj_wit_67733700 : (λ (VV : MyNat_u), MyNat_wf VV ∧ True) n') by (solver).
-    pose (exist (λ (VV : MyNat_u), MyNat_wf VV ∧ True) n' VV_inj_wit_67733700) as h_61136385_3.
-    pose (add_assoc h_61136385_1 h_61136385_2 h_61136385_3) as h_61136385.
-    try assert (ds_d5SW_inj_wit_60446462 : (λ (ds_d5SW : MyNat_u), MyNat_wf ds_d5SW ∧ True)
-                                           ds_d5SW) by (solver).
-    pose (exist (λ (ds_d5SW : MyNat_u),
-                 MyNat_wf ds_d5SW ∧ True) ds_d5SW ds_d5SW_inj_wit_60446462) as h_41322049_1_1.
+    pose (exist (λ (VV : MyNat_u), MyNat_wf VV ∧ True) n' VV_inj_wit_67733700) as h_76901889_3.
+    pose (add_assoc h_76901889_1 h_76901889_2 h_76901889_3) as h_76901889.
+    try assert (ds_d5TH_inj_wit_19375046 : (λ (ds_d5TH : MyNat_u), MyNat_wf ds_d5TH ∧ True)
+                                           ds_d5TH) by (solver).
+    pose (exist (λ (ds_d5TH : MyNat_u),
+                 MyNat_wf ds_d5TH ∧ True) ds_d5TH ds_d5TH_inj_wit_19375046) as h_17685865_1_1.
     try assert (VV_inj_wit_67733700 : (λ (VV : MyNat_u), MyNat_wf VV ∧ True) n') by (solver).
-    pose (exist (λ (VV : MyNat_u), MyNat_wf VV ∧ True) n' VV_inj_wit_67733700) as h_41322049_1_2_1.
-    try assert (ds_d5SW_inj_wit_60446462 : (λ (ds_d5SW : MyNat_u), MyNat_wf ds_d5SW ∧ True)
-                                           ds_d5SW) by (solver).
-    pose (exist (λ (ds_d5SW : MyNat_u),
-                 MyNat_wf ds_d5SW ∧ True) ds_d5SW ds_d5SW_inj_wit_60446462) as h_41322049_1_2_2.
-    pose (mult h_41322049_1_2_1 h_41322049_1_2_2) as h_41322049_1_2.
-    pose (plus h_41322049_1_1 h_41322049_1_2) as h_41322049_1.
+    pose (exist (λ (VV : MyNat_u), MyNat_wf VV ∧ True) n' VV_inj_wit_67733700) as h_17685865_1_2_1.
+    try assert (ds_d5TH_inj_wit_19375046 : (λ (ds_d5TH : MyNat_u), MyNat_wf ds_d5TH ∧ True)
+                                           ds_d5TH) by (solver).
+    pose (exist (λ (ds_d5TH : MyNat_u),
+                 MyNat_wf ds_d5TH ∧ True) ds_d5TH ds_d5TH_inj_wit_19375046) as h_17685865_1_2_2.
+    pose (mult h_17685865_1_2_1 h_17685865_1_2_2) as h_17685865_1_2.
+    pose (plus h_17685865_1_1 h_17685865_1_2) as h_17685865_1.
     try assert (VV_inj_wit_67733700 : (λ (VV : MyNat_u), MyNat_wf VV ∧ True) n') by (solver).
-    pose (exist (λ (VV : MyNat_u), MyNat_wf VV ∧ True) n' VV_inj_wit_67733700) as h_41322049_2.
-    pose (add_succ_r h_41322049_1 h_41322049_2) as h_41322049.
+    pose (exist (λ (VV : MyNat_u), MyNat_wf VV ∧ True) n' VV_inj_wit_67733700) as h_17685865_2.
+    pose (add_succ_r h_17685865_1 h_17685865_2) as h_17685865.
     refine (subsumptionCast
             Unit
             (λ (VV : Unit),
              ∃ (mult_res : MyNat_u),
-             mult_rel (S_u n') ds_d5SW mult_res
+             mult_rel (S_u n') ds_d5TH mult_res
              ∧ ∃ (plus_res : MyNat_u),
                plus_rel mult_res (S_u n') plus_res
-               ∧ ∃ (mult_res_2 : MyNat_u), mult_rel (S_u n') (S_u ds_d5SW) mult_res_2 ∧ plus_res == mult_res_2)
-            (IH_n' ltac:(try clear IH_n'; solver) ds_d5SW ltac:(try clear IH_n'; solver))
+               ∧ ∃ (mult_res_2 : MyNat_u), mult_rel (S_u n') (S_u ds_d5TH) mult_res_2 ∧ plus_res == mult_res_2)
+            (IH_n' ltac:(try clear IH_n'; solver) ds_d5TH ltac:(try clear IH_n'; solver))
             ltac:(solver)).
 Qed.
 
@@ -3867,15 +3916,15 @@ Proof.
           ltac:(solver)).
 Qed.
 
-Definition plus_1_neq_0_spec (ds_d5Si : MyNat): Type :=
-  {{∃ (plus_res : MyNat_u), plus_rel ⌊ ds_d5Si -⌋ ⌊ one -⌋ plus_res ∧ plus_res ≠ O_u}}.
+Definition plus_1_neq_0_spec (ds_d5T3 : MyNat): Type :=
+  {{∃ (plus_res : MyNat_u), plus_rel ⌊ ds_d5T3 -⌋ ⌊ one -⌋ plus_res ∧ plus_res ≠ O_u}}.
 
 #[global] Hint Unfold plus_1_neq_0_spec: lia_unfold.
 
-Theorem plus_1_neq_0 (ds_d5Si : MyNat): plus_1_neq_0_spec ds_d5Si.
+Theorem plus_1_neq_0 (ds_d5T3 : MyNat): plus_1_neq_0_spec ds_d5T3.
 Proof.
-  destruct ds_d5Si as [ds_d5Si ds_d5Si_p].
-  destruct ds_d5Si as [| ds_d5Sj].
+  destruct ds_d5T3 as [ds_d5T3 ds_d5T3_p].
+  destruct ds_d5T3 as [| ds_d5T4].
   - refine (subsumptionCast
             Unit
             (λ (VV : Unit), ∃ (plus_res : MyNat_u), plus_rel O_u ⌊ one -⌋ plus_res ∧ plus_res ≠ O_u)
@@ -3883,7 +3932,7 @@ Proof.
             ltac:(solver)).
   - refine (subsumptionCast
             Unit
-            (λ (VV : Unit), ∃ (plus_res : MyNat_u), plus_rel (S_u ds_d5Sj) ⌊ one -⌋ plus_res ∧ plus_res ≠ O_u)
+            (λ (VV : Unit), ∃ (plus_res : MyNat_u), plus_rel (S_u ds_d5T4) ⌊ one -⌋ plus_res ∧ plus_res ≠ O_u)
             (# unit)
             ltac:(solver)).
 Qed.
@@ -3950,19 +3999,19 @@ Proof.
           ltac:(solver)).
 Qed.
 
-Definition plus_n_Sm_spec (ds_d5Rg m : MyNat): Type :=
+Definition plus_n_Sm_spec (ds_d5S1 m : MyNat): Type :=
   {{∃ (plus_res : MyNat_u),
-    plus_rel ⌊ ds_d5Rg -⌋ ⌊ m -⌋ plus_res
+    plus_rel ⌊ ds_d5S1 -⌋ ⌊ m -⌋ plus_res
     ∧ ∃ (plus_res_2 : MyNat_u),
-      plus_rel ⌊ ds_d5Rg -⌋ (S_u ⌊ m -⌋) plus_res_2 ∧ S_u plus_res == plus_res_2}}.
+      plus_rel ⌊ ds_d5S1 -⌋ (S_u ⌊ m -⌋) plus_res_2 ∧ S_u plus_res == plus_res_2}}.
 
 #[global] Hint Unfold plus_n_Sm_spec: lia_unfold.
 
-Theorem plus_n_Sm (ds_d5Rg m : MyNat): plus_n_Sm_spec ds_d5Rg m.
+Theorem plus_n_Sm (ds_d5S1 m : MyNat): plus_n_Sm_spec ds_d5S1 m.
 Proof.
-  destruct ds_d5Rg as [ds_d5Rg ds_d5Rg_p].
+  destruct ds_d5S1 as [ds_d5S1 ds_d5S1_p].
   destruct m as [m m_p].
-  try revert m_p; generalize dependent m; induction ds_d5Rg as [| n' IH_n']; intros.
+  try revert m_p; generalize dependent m; induction ds_d5S1 as [| n' IH_n']; intros.
   - refine (subsumptionCast
             Unit
             (λ (VV : Unit),
@@ -3981,18 +4030,18 @@ Proof.
             ltac:(solver)).
 Qed.
 
-Definition add_comm_spec (ds_d5Rk m : MyNat): Type :=
+Definition add_comm_spec (ds_d5S5 m : MyNat): Type :=
   {{∃ (plus_res : MyNat_u),
-    plus_rel ⌊ ds_d5Rk -⌋ ⌊ m -⌋ plus_res
-    ∧ ∃ (plus_res_2 : MyNat_u), plus_rel ⌊ m -⌋ ⌊ ds_d5Rk -⌋ plus_res_2 ∧ plus_res == plus_res_2}}.
+    plus_rel ⌊ ds_d5S5 -⌋ ⌊ m -⌋ plus_res
+    ∧ ∃ (plus_res_2 : MyNat_u), plus_rel ⌊ m -⌋ ⌊ ds_d5S5 -⌋ plus_res_2 ∧ plus_res == plus_res_2}}.
 
 #[global] Hint Unfold add_comm_spec: lia_unfold.
 
-Theorem add_comm (ds_d5Rk m : MyNat): add_comm_spec ds_d5Rk m.
+Theorem add_comm (ds_d5S5 m : MyNat): add_comm_spec ds_d5S5 m.
 Proof.
-  destruct ds_d5Rk as [ds_d5Rk ds_d5Rk_p].
+  destruct ds_d5S5 as [ds_d5S5 ds_d5S5_p].
   destruct m as [m m_p].
-  try revert m_p; generalize dependent m; induction ds_d5Rk as [| n' IH_n']; intros.
+  try revert m_p; generalize dependent m; induction ds_d5S5 as [| n' IH_n']; intros.
   - refine (subsumptionCast
             Unit
             (λ (VV : Unit),
@@ -4021,15 +4070,15 @@ Proof.
             ltac:(solver)).
 Qed.
 
-Definition pred_spec (ds_d5SZ : MyNat): Type :=
+Definition pred_spec (ds_d5TK : MyNat): Type :=
   MyNat.
 
 #[global] Hint Unfold pred_spec: lia_unfold.
 
-Definition pred (ds_d5SZ : MyNat): pred_spec ds_d5SZ.
+Definition pred (ds_d5TK : MyNat): pred_spec ds_d5TK.
 Proof.
-  destruct ds_d5SZ as [ds_d5SZ ds_d5SZ_p].
-  destruct ds_d5SZ as [| n'].
+  destruct ds_d5TK as [ds_d5TK ds_d5TK_p].
+  destruct ds_d5TK as [| n'].
   - refine O.
   - refine (exist (λ (VV : MyNat_u), MyNat_wf VV ∧ True) n' ltac:(solver)).
 Defined.
@@ -4043,10 +4092,10 @@ Inductive pred_rel: MyNat_u → MyNat_u → Prop :=
 
 #[global] Instance pred_getF: getFunc pred_rel := { getF' := pred }.
 
-Theorem pred_rel_funct [ds_d5SZ : MyNat_u]:
-  ∀ (VV VV' : MyNat_u), pred_rel ds_d5SZ VV → (pred_rel ds_d5SZ VV' → VV = VV').
+Theorem pred_rel_funct [ds_d5TK : MyNat_u]:
+  ∀ (VV VV' : MyNat_u), pred_rel ds_d5TK VV → (pred_rel ds_d5TK VV' → VV = VV').
 Proof.
-  destruct ds_d5SZ as [| n']; rel_functionhood_body.
+  destruct ds_d5TK as [| n']; rel_functionhood_body.
 Qed.
 
 #[global] Hint Resolve pred_rel_funct: f_rel_funct_db.
@@ -4068,12 +4117,12 @@ Qed.
 
 #[global] Hint Rewrite pred_S_lem: f_rel_back.
 
-Theorem pred_rel_ex (ds_d5SZ : MyNat_u) (ds_d5SZ_p : MyNat_wf ds_d5SZ ∧ True):
-  pred_rel ds_d5SZ ⌊ pred (exist _ ds_d5SZ ds_d5SZ_p) -⌋.
+Theorem pred_rel_ex (ds_d5TK : MyNat_u) (ds_d5TK_p : MyNat_wf ds_d5TK ∧ True):
+  pred_rel ds_d5TK ⌊ pred (exist _ ds_d5TK ds_d5TK_p) -⌋.
 Proof.
   Opaque pred.
   existence_lemma_pre pred;
-  destruct ds_d5SZ as [| n'];
+  destruct ds_d5TK as [| n'];
   [fix_notations | fix_notations];
   simpl in *.
   Transparent pred.
@@ -4084,8 +4133,8 @@ Qed.
 
 #[global] Opaque pred.
 
-Theorem pred__pred_rel_rw (ds_d5SZ : MyNat_u) (ds_d5SZ_p : MyNat_wf ds_d5SZ ∧ True) (VV : MyNat_u):
-  ⌊ pred (exist _ ds_d5SZ ds_d5SZ_p) -⌋ = VV ↔ pred_rel ds_d5SZ VV.
+Theorem pred__pred_rel_rw (ds_d5TK : MyNat_u) (ds_d5TK_p : MyNat_wf ds_d5TK ∧ True) (VV : MyNat_u):
+  ⌊ pred (exist _ ds_d5TK ds_d5TK_p) -⌋ = VV ↔ pred_rel ds_d5TK VV.
 Proof.
   f__f_rel_rw.
 Qed.
@@ -4096,27 +4145,27 @@ Qed.
 
 #[global] Instance pred_lookup_rw: dictionary rwLem pred := { lookup' := pred__pred_rel_rw }.
 
-Theorem pred__pred_rel (ds_d5SZ : MyNat) (VV : MyNat_u):
-  ⌊ pred ds_d5SZ -⌋ = VV ↔ pred_rel ⌊ ds_d5SZ ⌋ VV.
+Theorem pred__pred_rel (ds_d5TK : MyNat) (VV : MyNat_u):
+  ⌊ pred ds_d5TK -⌋ = VV ↔ pred_rel ⌊ ds_d5TK ⌋ VV.
 Proof.
   f__f_rel.
 Qed.
 
 #[global] Hint Rewrite pred__pred_rel: f_rel_funct_db.
 
-Theorem pred__pred_rel' (ds_d5SZ_u : MyNat_u) (ds_d5SZ : MyNat) (VV : MyNat_u):
-  ds_d5SZ_u = ⌊ ds_d5SZ ⌋ → ⌊ pred ds_d5SZ -⌋ = VV ↔ pred_rel ds_d5SZ_u VV.
+Theorem pred__pred_rel' (ds_d5TK_u : MyNat_u) (ds_d5TK : MyNat) (VV : MyNat_u):
+  ds_d5TK_u = ⌊ ds_d5TK ⌋ → ⌊ pred ds_d5TK -⌋ = VV ↔ pred_rel ds_d5TK_u VV.
 Proof.
-  intros ->. refine (pred__pred_rel ds_d5SZ VV).
+  intros ->. refine (pred__pred_rel ds_d5TK VV).
 Qed.
 
 #[global] Hint Resolve pred__pred_rel': f_rel_funct_db.
 
-Theorem pred_rel_mk (ds_d5SZ : MyNat_u) (ds_d5SZ_p : MyNat_wf ds_d5SZ ∧ True):
-  {VV: _ | pred_rel ds_d5SZ VV}.
+Theorem pred_rel_mk (ds_d5TK : MyNat_u) (ds_d5TK_p : MyNat_wf ds_d5TK ∧ True):
+  {VV: _ | pred_rel ds_d5TK VV}.
 Proof.
   intros;
-  refine (subsumptionCast _ (λ VV, pred_rel ds_d5SZ VV) (pred (exist _ ds_d5SZ ds_d5SZ_p)) _);
+  refine (subsumptionCast _ (λ VV, pred_rel ds_d5TK VV) (pred (exist _ ds_d5TK ds_d5TK_p)) _);
   rewrite <- pred__pred_rel';
   quicksolve.
 Qed.
@@ -4125,12 +4174,12 @@ Qed.
 
 #[global] Instance pred_pack:
   @Pack
-  (MyNat ::RT λ (ds_d5SZ : MyNat), nilRT)
+  (MyNat ::RT λ (ds_d5TK : MyNat), nilRT)
   (MyNat_u ::UT nilUT)
-  ltac:(mkProjectsArgListTG (MyNat ::RT λ (ds_d5SZ : MyNat), nilRT) ((MyNat_u ::UT nilUT)))
+  ltac:(mkProjectsArgListTG (MyNat ::RT λ (ds_d5TK : MyNat), nilRT) ((MyNat_u ::UT nilUT)))
   MyNat_u
-  (λ (x_31234608 : ArgList (MyNat ::RT λ (ds_d5SZ : MyNat), nilRT)) (v_x_31234608 : MyNat_u),
-   ltac:(flattenP (λ (ds_d5SZ : MyNat) (VV : MyNat_u), MyNat_wf VV ∧ True) x_31234608 v_x_31234608)).
+  (λ (x_36055662 : ArgList (MyNat ::RT λ (ds_d5TK : MyNat), nilRT)) (v_x_36055662 : MyNat_u),
+   ltac:(flattenP (λ (ds_d5TK : MyNat) (VV : MyNat_u), MyNat_wf VV ∧ True) x_36055662 v_x_36055662)).
 Proof.
   buildPackG pred pred_rel pred__pred_rel pred_rel_funct.
 Defined.
@@ -4140,28 +4189,28 @@ Proof.
   buildUPackG pred_rel pred_rel_funct.
 Defined.
 
-Definition sf_exp_spec (ds_d5SP ds_d5SQ : MyNat): Type :=
+Definition sf_exp_spec (ds_d5TA ds_d5TB : MyNat): Type :=
   MyNat.
 
 #[global] Hint Unfold sf_exp_spec: lia_unfold.
 
-Definition sf_exp (ds_d5SP ds_d5SQ : MyNat): sf_exp_spec ds_d5SP ds_d5SQ.
+Definition sf_exp (ds_d5TA ds_d5TB : MyNat): sf_exp_spec ds_d5TA ds_d5TB.
 Proof.
-  destruct ds_d5SP as [ds_d5SP ds_d5SP_p].
-  destruct ds_d5SQ as [ds_d5SQ ds_d5SQ_p].
-  try revert ds_d5SP_p; generalize dependent ds_d5SP; induction ds_d5SQ as [| p IH_p]; intros.
+  destruct ds_d5TA as [ds_d5TA ds_d5TA_p].
+  destruct ds_d5TB as [ds_d5TB ds_d5TB_p].
+  try revert ds_d5TA_p; generalize dependent ds_d5TA; induction ds_d5TB as [| p IH_p]; intros.
   - refine (S O).
   - refine (mult
-            (exist (λ (ds_d5SP : MyNat_u), MyNat_wf ds_d5SP ∧ True) ds_d5SP ltac:(solver))
-            (IH_p ltac:(try clear IH_p; solver) ds_d5SP ltac:(try clear IH_p; solver))).
+            (exist (λ (ds_d5TA : MyNat_u), MyNat_wf ds_d5TA ∧ True) ds_d5TA ltac:(solver))
+            (IH_p ltac:(try clear IH_p; solver) ds_d5TA ltac:(try clear IH_p; solver))).
 Defined.
 
 Inductive sf_exp_rel: MyNat_u → MyNat_u → MyNat_u → Prop :=
-  | sf_exp_x_O: ∀ ds_d5SP, sf_exp_rel ds_d5SP O_u (S_u O_u)
-  | sf_exp_x_S: ∀ ds_d5SP p (sf_exp_res : MyNat_u),
-                sf_exp_rel ds_d5SP p sf_exp_res
+  | sf_exp_x_O: ∀ ds_d5TA, sf_exp_rel ds_d5TA O_u (S_u O_u)
+  | sf_exp_x_S: ∀ ds_d5TA p (sf_exp_res : MyNat_u),
+                sf_exp_rel ds_d5TA p sf_exp_res
                 → ∀ (mult_res : MyNat_u),
-                  mult_rel ds_d5SP sf_exp_res mult_res → sf_exp_rel ds_d5SP (S_u p) mult_res.
+                  mult_rel ds_d5TA sf_exp_res mult_res → sf_exp_rel ds_d5TA (S_u p) mult_res.
 
 #[global] Hint Constructors sf_exp_rel: core_hint_db.
 
@@ -4169,10 +4218,10 @@ Inductive sf_exp_rel: MyNat_u → MyNat_u → MyNat_u → Prop :=
 
 #[global] Instance sf_exp_getF: getFunc sf_exp_rel := { getF' := sf_exp }.
 
-Theorem sf_exp_rel_funct [ds_d5SP ds_d5SQ : MyNat_u]:
-  ∀ (VV VV' : MyNat_u), sf_exp_rel ds_d5SP ds_d5SQ VV → (sf_exp_rel ds_d5SP ds_d5SQ VV' → VV = VV').
+Theorem sf_exp_rel_funct [ds_d5TA ds_d5TB : MyNat_u]:
+  ∀ (VV VV' : MyNat_u), sf_exp_rel ds_d5TA ds_d5TB VV → (sf_exp_rel ds_d5TA ds_d5TB VV' → VV = VV').
 Proof.
-  try revert ds_d5SP_p; generalize dependent ds_d5SP; induction ds_d5SQ as [| p IH_p]; intros;
+  try revert ds_d5TA_p; generalize dependent ds_d5TA; induction ds_d5TB as [| p IH_p]; intros;
   rel_functionhood_body.
 Qed.
 
@@ -4181,19 +4230,19 @@ Qed.
 #[global] Instance sf_exp_lookup_funct: dictionary functionhood sf_exp := {
     lookup' := sf_exp_rel_funct }.
 
-Theorem sf_exp_x_O_lem ds_d5SP sf_exp_x_O_lem_res:
-  sf_exp_rel ds_d5SP O_u sf_exp_x_O_lem_res ↔ sf_exp_x_O_lem_res == S_u O_u.
+Theorem sf_exp_x_O_lem ds_d5TA sf_exp_x_O_lem_res:
+  sf_exp_rel ds_d5TA O_u sf_exp_x_O_lem_res ↔ sf_exp_x_O_lem_res == S_u O_u.
 Proof.
   rel_back' _nil.
 Qed.
 
 #[global] Hint Rewrite sf_exp_x_O_lem: f_rel_back.
 
-Theorem sf_exp_x_S_lem ds_d5SP p sf_exp_x_S_lem_res:
-  sf_exp_rel ds_d5SP (S_u p) sf_exp_x_S_lem_res
+Theorem sf_exp_x_S_lem ds_d5TA p sf_exp_x_S_lem_res:
+  sf_exp_rel ds_d5TA (S_u p) sf_exp_x_S_lem_res
   ↔ ∃ (sf_exp_res : MyNat_u),
-    sf_exp_rel ds_d5SP p sf_exp_res
-    ∧ ∃ (mult_res : MyNat_u), mult_rel ds_d5SP sf_exp_res mult_res ∧ sf_exp_x_S_lem_res == mult_res.
+    sf_exp_rel ds_d5TA p sf_exp_res
+    ∧ ∃ (mult_res : MyNat_u), mult_rel ds_d5TA sf_exp_res mult_res ∧ sf_exp_x_S_lem_res == mult_res.
 Proof.
   rel_back' _nil.
 Qed.
@@ -4201,21 +4250,21 @@ Qed.
 #[global] Hint Rewrite sf_exp_x_S_lem: f_rel_back.
 
 Theorem sf_exp_rel_ex
-  (ds_d5SP : MyNat_u)
-  (ds_d5SP_p : MyNat_wf ds_d5SP ∧ True)
-  (ds_d5SQ : MyNat_u)
-  (ds_d5SQ_p : MyNat_wf ds_d5SQ ∧ True):
-  sf_exp_rel ds_d5SP ds_d5SQ ⌊ sf_exp (exist _ ds_d5SP ds_d5SP_p) (exist _ ds_d5SQ ds_d5SQ_p) -⌋.
+  (ds_d5TA : MyNat_u)
+  (ds_d5TA_p : MyNat_wf ds_d5TA ∧ True)
+  (ds_d5TB : MyNat_u)
+  (ds_d5TB_p : MyNat_wf ds_d5TB ∧ True):
+  sf_exp_rel ds_d5TA ds_d5TB ⌊ sf_exp (exist _ ds_d5TA ds_d5TA_p) (exist _ ds_d5TB ds_d5TB_p) -⌋.
 Proof.
   Opaque sf_exp.
   existence_lemma_pre sf_exp;
-  try revert ds_d5SP_p; generalize dependent ds_d5SP; induction ds_d5SQ as [| p IH_p]; intros;
+  try revert ds_d5TA_p; generalize dependent ds_d5TA; induction ds_d5TB as [| p IH_p]; intros;
   [fix_notations |
    fix_notations;
    pose proof (IH_p
                ltac:(try clear IH_p; solver)
-               ds_d5SP
-               ltac:(try clear IH_p; solver)) as IH_70234888;
+               ds_d5TA
+               ltac:(try clear IH_p; solver)) as IH_70297771;
    try clear IH_p];
   simpl in *.
   Transparent sf_exp.
@@ -4227,13 +4276,13 @@ Qed.
 #[global] Opaque sf_exp.
 
 Theorem sf_exp__sf_exp_rel_rw
-  (ds_d5SP : MyNat_u)
-  (ds_d5SP_p : MyNat_wf ds_d5SP ∧ True)
-  (ds_d5SQ : MyNat_u)
-  (ds_d5SQ_p : MyNat_wf ds_d5SQ ∧ True)
+  (ds_d5TA : MyNat_u)
+  (ds_d5TA_p : MyNat_wf ds_d5TA ∧ True)
+  (ds_d5TB : MyNat_u)
+  (ds_d5TB_p : MyNat_wf ds_d5TB ∧ True)
   (VV : MyNat_u):
-  ⌊ sf_exp (exist _ ds_d5SP ds_d5SP_p) (exist _ ds_d5SQ ds_d5SQ_p) -⌋ = VV
-  ↔ sf_exp_rel ds_d5SP ds_d5SQ VV.
+  ⌊ sf_exp (exist _ ds_d5TA ds_d5TA_p) (exist _ ds_d5TB ds_d5TB_p) -⌋ = VV
+  ↔ sf_exp_rel ds_d5TA ds_d5TB VV.
 Proof.
   f__f_rel_rw.
 Qed.
@@ -4245,8 +4294,8 @@ Qed.
 #[global] Instance sf_exp_lookup_rw: dictionary rwLem sf_exp := {
     lookup' := sf_exp__sf_exp_rel_rw }.
 
-Theorem sf_exp__sf_exp_rel (ds_d5SP ds_d5SQ : MyNat) (VV : MyNat_u):
-  ⌊ sf_exp ds_d5SP ds_d5SQ -⌋ = VV ↔ sf_exp_rel ⌊ ds_d5SP ⌋ ⌊ ds_d5SQ ⌋ VV.
+Theorem sf_exp__sf_exp_rel (ds_d5TA ds_d5TB : MyNat) (VV : MyNat_u):
+  ⌊ sf_exp ds_d5TA ds_d5TB -⌋ = VV ↔ sf_exp_rel ⌊ ds_d5TA ⌋ ⌊ ds_d5TB ⌋ VV.
 Proof.
   f__f_rel.
 Qed.
@@ -4254,27 +4303,27 @@ Qed.
 #[global] Hint Rewrite sf_exp__sf_exp_rel: f_rel_funct_db.
 
 Theorem sf_exp__sf_exp_rel'
-  (ds_d5SP_u ds_d5SQ_u : MyNat_u) (ds_d5SP ds_d5SQ : MyNat) (VV : MyNat_u):
-  ds_d5SP_u = ⌊ ds_d5SP ⌋
-  → (ds_d5SQ_u = ⌊ ds_d5SQ ⌋ → ⌊ sf_exp ds_d5SP ds_d5SQ -⌋ = VV ↔ sf_exp_rel ds_d5SP_u ds_d5SQ_u VV).
+  (ds_d5TA_u ds_d5TB_u : MyNat_u) (ds_d5TA ds_d5TB : MyNat) (VV : MyNat_u):
+  ds_d5TA_u = ⌊ ds_d5TA ⌋
+  → (ds_d5TB_u = ⌊ ds_d5TB ⌋ → ⌊ sf_exp ds_d5TA ds_d5TB -⌋ = VV ↔ sf_exp_rel ds_d5TA_u ds_d5TB_u VV).
 Proof.
-  intros -> ->. refine (sf_exp__sf_exp_rel ds_d5SP ds_d5SQ VV).
+  intros -> ->. refine (sf_exp__sf_exp_rel ds_d5TA ds_d5TB VV).
 Qed.
 
 #[global] Hint Resolve sf_exp__sf_exp_rel': f_rel_funct_db.
 
 Theorem sf_exp_rel_mk
-  (ds_d5SP : MyNat_u)
-  (ds_d5SP_p : MyNat_wf ds_d5SP ∧ True)
-  (ds_d5SQ : MyNat_u)
-  (ds_d5SQ_p : MyNat_wf ds_d5SQ ∧ True):
-  {VV: _ | sf_exp_rel ds_d5SP ds_d5SQ VV}.
+  (ds_d5TA : MyNat_u)
+  (ds_d5TA_p : MyNat_wf ds_d5TA ∧ True)
+  (ds_d5TB : MyNat_u)
+  (ds_d5TB_p : MyNat_wf ds_d5TB ∧ True):
+  {VV: _ | sf_exp_rel ds_d5TA ds_d5TB VV}.
 Proof.
   intros;
   refine (subsumptionCast
           _
-          (λ VV, sf_exp_rel ds_d5SP ds_d5SQ VV)
-          (sf_exp (exist _ ds_d5SP ds_d5SP_p) (exist _ ds_d5SQ ds_d5SQ_p))
+          (λ VV, sf_exp_rel ds_d5TA ds_d5TB VV)
+          (sf_exp (exist _ ds_d5TA ds_d5TA_p) (exist _ ds_d5TB ds_d5TB_p))
           _);
   rewrite <- sf_exp__sf_exp_rel';
   quicksolve.
@@ -4284,14 +4333,14 @@ Qed.
 
 #[global] Instance sf_exp_pack:
   @Pack
-  (MyNat ::RT λ (ds_d5SP : MyNat), MyNat ::RT λ (ds_d5SQ : MyNat), nilRT)
+  (MyNat ::RT λ (ds_d5TA : MyNat), MyNat ::RT λ (ds_d5TB : MyNat), nilRT)
   (MyNat_u ::UT (MyNat_u ::UT nilUT))
   ltac:(mkProjectsArgListTG (MyNat
- ::RT λ (ds_d5SP : MyNat), MyNat ::RT λ (ds_d5SQ : MyNat), nilRT) ((MyNat_u ::UT (MyNat_u ::UT nilUT))))
+ ::RT λ (ds_d5TA : MyNat), MyNat ::RT λ (ds_d5TB : MyNat), nilRT) ((MyNat_u ::UT (MyNat_u ::UT nilUT))))
   MyNat_u
-  (λ (x_28517735 : ArgList (MyNat ::RT λ (ds_d5SP : MyNat), MyNat ::RT λ (ds_d5SQ : MyNat), nilRT))
-     (v_x_28517735 : MyNat_u),
-   ltac:(flattenP (λ (ds_d5SP ds_d5SQ : MyNat) (VV : MyNat_u), MyNat_wf VV ∧ True) x_28517735 v_x_28517735)).
+  (λ (x_45573830 : ArgList (MyNat ::RT λ (ds_d5TA : MyNat), MyNat ::RT λ (ds_d5TB : MyNat), nilRT))
+     (v_x_45573830 : MyNat_u),
+   ltac:(flattenP (λ (ds_d5TA ds_d5TB : MyNat) (VV : MyNat_u), MyNat_wf VV ∧ True) x_45573830 v_x_45573830)).
 Proof.
   buildPackG sf_exp sf_exp_rel sf_exp__sf_exp_rel sf_exp_rel_funct.
 Defined.
@@ -4301,15 +4350,15 @@ Proof.
   buildUPackG sf_exp_rel sf_exp_rel_funct.
 Defined.
 
-Definition sndSF_spec (ds_d5Re : Natprod): Type :=
+Definition sndSF_spec (ds_d5RZ : Natprod): Type :=
   MyNat.
 
 #[global] Hint Unfold sndSF_spec: lia_unfold.
 
-Definition sndSF (ds_d5Re : Natprod): sndSF_spec ds_d5Re.
+Definition sndSF (ds_d5RZ : Natprod): sndSF_spec ds_d5RZ.
 Proof.
-  destruct ds_d5Re as [ds_d5Re ds_d5Re_p].
-  destruct ds_d5Re as [n1 n2].
+  destruct ds_d5RZ as [ds_d5RZ ds_d5RZ_p].
+  destruct ds_d5RZ as [n1 n2].
   - refine (exist (λ (n2 : MyNat_u), MyNat_wf n2 ∧ True) n2 ltac:(solver)).
 Defined.
 
@@ -4322,10 +4371,10 @@ Inductive sndSF_rel: Natprod_u → MyNat_u → Prop :=
 
 #[global] Instance sndSF_getF: getFunc sndSF_rel := { getF' := sndSF }.
 
-Theorem sndSF_rel_funct [ds_d5Re : Natprod_u]:
-  ∀ (VV VV' : MyNat_u), sndSF_rel ds_d5Re VV → (sndSF_rel ds_d5Re VV' → VV = VV').
+Theorem sndSF_rel_funct [ds_d5RZ : Natprod_u]:
+  ∀ (VV VV' : MyNat_u), sndSF_rel ds_d5RZ VV → (sndSF_rel ds_d5RZ VV' → VV = VV').
 Proof.
-  destruct ds_d5Re as [n1 n2]; rel_functionhood_body.
+  destruct ds_d5RZ as [n1 n2]; rel_functionhood_body.
 Qed.
 
 #[global] Hint Resolve sndSF_rel_funct: f_rel_funct_db.
@@ -4341,12 +4390,12 @@ Qed.
 
 #[global] Hint Rewrite sndSF_Pair_lem: f_rel_back.
 
-Theorem sndSF_rel_ex (ds_d5Re : Natprod_u) (ds_d5Re_p : Natprod_wf ds_d5Re ∧ True):
-  sndSF_rel ds_d5Re ⌊ sndSF (exist _ ds_d5Re ds_d5Re_p) -⌋.
+Theorem sndSF_rel_ex (ds_d5RZ : Natprod_u) (ds_d5RZ_p : Natprod_wf ds_d5RZ ∧ True):
+  sndSF_rel ds_d5RZ ⌊ sndSF (exist _ ds_d5RZ ds_d5RZ_p) -⌋.
 Proof.
   Opaque sndSF.
   existence_lemma_pre sndSF;
-  destruct ds_d5Re as [n1 n2];
+  destruct ds_d5RZ as [n1 n2];
   [fix_notations];
   simpl in *.
   Transparent sndSF.
@@ -4358,8 +4407,8 @@ Qed.
 #[global] Opaque sndSF.
 
 Theorem sndSF__sndSF_rel_rw
-  (ds_d5Re : Natprod_u) (ds_d5Re_p : Natprod_wf ds_d5Re ∧ True) (VV : MyNat_u):
-  ⌊ sndSF (exist _ ds_d5Re ds_d5Re_p) -⌋ = VV ↔ sndSF_rel ds_d5Re VV.
+  (ds_d5RZ : Natprod_u) (ds_d5RZ_p : Natprod_wf ds_d5RZ ∧ True) (VV : MyNat_u):
+  ⌊ sndSF (exist _ ds_d5RZ ds_d5RZ_p) -⌋ = VV ↔ sndSF_rel ds_d5RZ VV.
 Proof.
   f__f_rel_rw.
 Qed.
@@ -4370,27 +4419,27 @@ Qed.
 
 #[global] Instance sndSF_lookup_rw: dictionary rwLem sndSF := { lookup' := sndSF__sndSF_rel_rw }.
 
-Theorem sndSF__sndSF_rel (ds_d5Re : Natprod) (VV : MyNat_u):
-  ⌊ sndSF ds_d5Re -⌋ = VV ↔ sndSF_rel ⌊ ds_d5Re ⌋ VV.
+Theorem sndSF__sndSF_rel (ds_d5RZ : Natprod) (VV : MyNat_u):
+  ⌊ sndSF ds_d5RZ -⌋ = VV ↔ sndSF_rel ⌊ ds_d5RZ ⌋ VV.
 Proof.
   f__f_rel.
 Qed.
 
 #[global] Hint Rewrite sndSF__sndSF_rel: f_rel_funct_db.
 
-Theorem sndSF__sndSF_rel' (ds_d5Re_u : Natprod_u) (ds_d5Re : Natprod) (VV : MyNat_u):
-  ds_d5Re_u = ⌊ ds_d5Re ⌋ → ⌊ sndSF ds_d5Re -⌋ = VV ↔ sndSF_rel ds_d5Re_u VV.
+Theorem sndSF__sndSF_rel' (ds_d5RZ_u : Natprod_u) (ds_d5RZ : Natprod) (VV : MyNat_u):
+  ds_d5RZ_u = ⌊ ds_d5RZ ⌋ → ⌊ sndSF ds_d5RZ -⌋ = VV ↔ sndSF_rel ds_d5RZ_u VV.
 Proof.
-  intros ->. refine (sndSF__sndSF_rel ds_d5Re VV).
+  intros ->. refine (sndSF__sndSF_rel ds_d5RZ VV).
 Qed.
 
 #[global] Hint Resolve sndSF__sndSF_rel': f_rel_funct_db.
 
-Theorem sndSF_rel_mk (ds_d5Re : Natprod_u) (ds_d5Re_p : Natprod_wf ds_d5Re ∧ True):
-  {VV: _ | sndSF_rel ds_d5Re VV}.
+Theorem sndSF_rel_mk (ds_d5RZ : Natprod_u) (ds_d5RZ_p : Natprod_wf ds_d5RZ ∧ True):
+  {VV: _ | sndSF_rel ds_d5RZ VV}.
 Proof.
   intros;
-  refine (subsumptionCast _ (λ VV, sndSF_rel ds_d5Re VV) (sndSF (exist _ ds_d5Re ds_d5Re_p)) _);
+  refine (subsumptionCast _ (λ VV, sndSF_rel ds_d5RZ VV) (sndSF (exist _ ds_d5RZ ds_d5RZ_p)) _);
   rewrite <- sndSF__sndSF_rel';
   quicksolve.
 Qed.
@@ -4399,12 +4448,12 @@ Qed.
 
 #[global] Instance sndSF_pack:
   @Pack
-  (Natprod ::RT λ (ds_d5Re : Natprod), nilRT)
+  (Natprod ::RT λ (ds_d5RZ : Natprod), nilRT)
   (Natprod_u ::UT nilUT)
-  ltac:(mkProjectsArgListTG (Natprod ::RT λ (ds_d5Re : Natprod), nilRT) ((Natprod_u ::UT nilUT)))
+  ltac:(mkProjectsArgListTG (Natprod ::RT λ (ds_d5RZ : Natprod), nilRT) ((Natprod_u ::UT nilUT)))
   MyNat_u
-  (λ (x_67238264 : ArgList (Natprod ::RT λ (ds_d5Re : Natprod), nilRT)) (v_x_67238264 : MyNat_u),
-   ltac:(flattenP (λ (ds_d5Re : Natprod) (VV : MyNat_u), MyNat_wf VV ∧ True) x_67238264 v_x_67238264)).
+  (λ (x_29619004 : ArgList (Natprod ::RT λ (ds_d5RZ : Natprod), nilRT)) (v_x_29619004 : MyNat_u),
+   ltac:(flattenP (λ (ds_d5RZ : Natprod) (VV : MyNat_u), MyNat_wf VV ∧ True) x_29619004 v_x_29619004)).
 Proof.
   buildPackG sndSF sndSF_rel sndSF__sndSF_rel sndSF_rel_funct.
 Defined.
@@ -4414,18 +4463,18 @@ Proof.
   buildUPackG sndSF_rel sndSF_rel_funct.
 Defined.
 
-Definition surjective_pairing_spec (ds_d5Ra : Natprod): Type :=
+Definition surjective_pairing_spec (ds_d5RV : Natprod): Type :=
   {{∃ (sndSF_res : MyNat_u),
-    sndSF_rel ⌊ ds_d5Ra -⌋ sndSF_res
+    sndSF_rel ⌊ ds_d5RV -⌋ sndSF_res
     ∧ ∃ (fstSF_res : MyNat_u),
-      fstSF_rel ⌊ ds_d5Ra -⌋ fstSF_res ∧ ⌊ ds_d5Ra -⌋ == Pair_u fstSF_res sndSF_res}}.
+      fstSF_rel ⌊ ds_d5RV -⌋ fstSF_res ∧ ⌊ ds_d5RV -⌋ == Pair_u fstSF_res sndSF_res}}.
 
 #[global] Hint Unfold surjective_pairing_spec: lia_unfold.
 
-Theorem surjective_pairing (ds_d5Ra : Natprod): surjective_pairing_spec ds_d5Ra.
+Theorem surjective_pairing (ds_d5RV : Natprod): surjective_pairing_spec ds_d5RV.
 Proof.
-  destruct ds_d5Ra as [ds_d5Ra ds_d5Ra_p].
-  destruct ds_d5Ra as [n m].
+  destruct ds_d5RV as [ds_d5RV ds_d5RV_p].
+  destruct ds_d5RV as [n m].
   - refine (subsumptionCast
             Unit
             (λ (VV : Unit),
@@ -4685,17 +4734,17 @@ Proof.
           ltac:(solver)).
 Qed.
 
-Definition zero_nbeq_plus_1_spec (ds_d5Sb : MyNat): Type :=
+Definition zero_nbeq_plus_1_spec (ds_d5SW : MyNat): Type :=
   {{∃ (plus_res : MyNat_u),
-    plus_rel ⌊ ds_d5Sb -⌋ ⌊ one -⌋ plus_res
+    plus_rel ⌊ ds_d5SW -⌋ ⌊ one -⌋ plus_res
     ∧ ∃ (eqb_res : SFBool_u), eqb_rel O_u plus_res eqb_res ∧ eqb_res == SFFalse_u}}.
 
 #[global] Hint Unfold zero_nbeq_plus_1_spec: lia_unfold.
 
-Theorem zero_nbeq_plus_1 (ds_d5Sb : MyNat): zero_nbeq_plus_1_spec ds_d5Sb.
+Theorem zero_nbeq_plus_1 (ds_d5SW : MyNat): zero_nbeq_plus_1_spec ds_d5SW.
 Proof.
-  destruct ds_d5Sb as [ds_d5Sb ds_d5Sb_p].
-  destruct ds_d5Sb as [| n'].
+  destruct ds_d5SW as [ds_d5SW ds_d5SW_p].
+  destruct ds_d5SW as [| n'].
   - refine (subsumptionCast
             Unit
             (λ (VV : Unit),
@@ -4890,15 +4939,15 @@ Definition F : Letter :=
 
 #[global] Hint Unfold F: ref_constr_db.
 
-Definition lower_letter_spec (ds_d5Rv : Letter): Type :=
+Definition lower_letter_spec (ds_d5Sg : Letter): Type :=
   Letter.
 
 #[global] Hint Unfold lower_letter_spec: lia_unfold.
 
-Definition lower_letter (ds_d5Rv : Letter): lower_letter_spec ds_d5Rv.
+Definition lower_letter (ds_d5Sg : Letter): lower_letter_spec ds_d5Sg.
 Proof.
-  destruct ds_d5Rv as [ds_d5Rv ds_d5Rv_p].
-  destruct ds_d5Rv as [| | | |].
+  destruct ds_d5Sg as [ds_d5Sg ds_d5Sg_p].
+  destruct ds_d5Sg as [| | | |].
   - refine B.
   - refine C.
   - refine D.
@@ -4920,10 +4969,10 @@ Inductive lower_letter_rel: Letter_u → Letter_u → Prop :=
 
 #[global] Instance lower_letter_getF: getFunc lower_letter_rel := { getF' := lower_letter }.
 
-Theorem lower_letter_rel_funct [ds_d5Rv : Letter_u]:
-  ∀ (VV VV' : Letter_u), lower_letter_rel ds_d5Rv VV → (lower_letter_rel ds_d5Rv VV' → VV = VV').
+Theorem lower_letter_rel_funct [ds_d5Sg : Letter_u]:
+  ∀ (VV VV' : Letter_u), lower_letter_rel ds_d5Sg VV → (lower_letter_rel ds_d5Sg VV' → VV = VV').
 Proof.
-  destruct ds_d5Rv as [| | | |]; rel_functionhood_body.
+  destruct ds_d5Sg as [| | | |]; rel_functionhood_body.
 Qed.
 
 #[global] Hint Resolve lower_letter_rel_funct: f_rel_funct_db.
@@ -4971,12 +5020,12 @@ Qed.
 
 #[global] Hint Rewrite lower_letter_F_lem: f_rel_back.
 
-Theorem lower_letter_rel_ex (ds_d5Rv : Letter_u) (ds_d5Rv_p : Letter_wf ds_d5Rv ∧ True):
-  lower_letter_rel ds_d5Rv ⌊ lower_letter (exist _ ds_d5Rv ds_d5Rv_p) -⌋.
+Theorem lower_letter_rel_ex (ds_d5Sg : Letter_u) (ds_d5Sg_p : Letter_wf ds_d5Sg ∧ True):
+  lower_letter_rel ds_d5Sg ⌊ lower_letter (exist _ ds_d5Sg ds_d5Sg_p) -⌋.
 Proof.
   Opaque lower_letter.
   existence_lemma_pre lower_letter;
-  destruct ds_d5Rv as [| | | |];
+  destruct ds_d5Sg as [| | | |];
   [fix_notations | fix_notations | fix_notations | fix_notations | fix_notations];
   simpl in *.
   Transparent lower_letter.
@@ -4988,8 +5037,8 @@ Qed.
 #[global] Opaque lower_letter.
 
 Theorem lower_letter__lower_letter_rel_rw
-  (ds_d5Rv : Letter_u) (ds_d5Rv_p : Letter_wf ds_d5Rv ∧ True) (VV : Letter_u):
-  ⌊ lower_letter (exist _ ds_d5Rv ds_d5Rv_p) -⌋ = VV ↔ lower_letter_rel ds_d5Rv VV.
+  (ds_d5Sg : Letter_u) (ds_d5Sg_p : Letter_wf ds_d5Sg ∧ True) (VV : Letter_u):
+  ⌊ lower_letter (exist _ ds_d5Sg ds_d5Sg_p) -⌋ = VV ↔ lower_letter_rel ds_d5Sg VV.
 Proof.
   f__f_rel_rw.
 Qed.
@@ -5001,30 +5050,30 @@ Qed.
 #[global] Instance lower_letter_lookup_rw: dictionary rwLem lower_letter := {
     lookup' := lower_letter__lower_letter_rel_rw }.
 
-Theorem lower_letter__lower_letter_rel (ds_d5Rv : Letter) (VV : Letter_u):
-  ⌊ lower_letter ds_d5Rv -⌋ = VV ↔ lower_letter_rel ⌊ ds_d5Rv ⌋ VV.
+Theorem lower_letter__lower_letter_rel (ds_d5Sg : Letter) (VV : Letter_u):
+  ⌊ lower_letter ds_d5Sg -⌋ = VV ↔ lower_letter_rel ⌊ ds_d5Sg ⌋ VV.
 Proof.
   f__f_rel.
 Qed.
 
 #[global] Hint Rewrite lower_letter__lower_letter_rel: f_rel_funct_db.
 
-Theorem lower_letter__lower_letter_rel' (ds_d5Rv_u : Letter_u) (ds_d5Rv : Letter) (VV : Letter_u):
-  ds_d5Rv_u = ⌊ ds_d5Rv ⌋ → ⌊ lower_letter ds_d5Rv -⌋ = VV ↔ lower_letter_rel ds_d5Rv_u VV.
+Theorem lower_letter__lower_letter_rel' (ds_d5Sg_u : Letter_u) (ds_d5Sg : Letter) (VV : Letter_u):
+  ds_d5Sg_u = ⌊ ds_d5Sg ⌋ → ⌊ lower_letter ds_d5Sg -⌋ = VV ↔ lower_letter_rel ds_d5Sg_u VV.
 Proof.
-  intros ->. refine (lower_letter__lower_letter_rel ds_d5Rv VV).
+  intros ->. refine (lower_letter__lower_letter_rel ds_d5Sg VV).
 Qed.
 
 #[global] Hint Resolve lower_letter__lower_letter_rel': f_rel_funct_db.
 
-Theorem lower_letter_rel_mk (ds_d5Rv : Letter_u) (ds_d5Rv_p : Letter_wf ds_d5Rv ∧ True):
-  {VV: _ | lower_letter_rel ds_d5Rv VV}.
+Theorem lower_letter_rel_mk (ds_d5Sg : Letter_u) (ds_d5Sg_p : Letter_wf ds_d5Sg ∧ True):
+  {VV: _ | lower_letter_rel ds_d5Sg VV}.
 Proof.
   intros;
   refine (subsumptionCast
           _
-          (λ VV, lower_letter_rel ds_d5Rv VV)
-          (lower_letter (exist _ ds_d5Rv ds_d5Rv_p))
+          (λ VV, lower_letter_rel ds_d5Sg VV)
+          (lower_letter (exist _ ds_d5Sg ds_d5Sg_p))
           _);
   rewrite <- lower_letter__lower_letter_rel';
   quicksolve.
@@ -5034,12 +5083,12 @@ Qed.
 
 #[global] Instance lower_letter_pack:
   @Pack
-  (Letter ::RT λ (ds_d5Rv : Letter), nilRT)
+  (Letter ::RT λ (ds_d5Sg : Letter), nilRT)
   (Letter_u ::UT nilUT)
-  ltac:(mkProjectsArgListTG (Letter ::RT λ (ds_d5Rv : Letter), nilRT) ((Letter_u ::UT nilUT)))
+  ltac:(mkProjectsArgListTG (Letter ::RT λ (ds_d5Sg : Letter), nilRT) ((Letter_u ::UT nilUT)))
   Letter_u
-  (λ (x_19890185 : ArgList (Letter ::RT λ (ds_d5Rv : Letter), nilRT)) (v_x_19890185 : Letter_u),
-   ltac:(flattenP (λ (ds_d5Rv : Letter) (VV : Letter_u), Letter_wf VV ∧ True) x_19890185 v_x_19890185)).
+  (λ (x_26174575 : ArgList (Letter ::RT λ (ds_d5Sg : Letter), nilRT)) (v_x_26174575 : Letter_u),
+   ltac:(flattenP (λ (ds_d5Sg : Letter) (VV : Letter_u), Letter_wf VV ∧ True) x_26174575 v_x_26174575)).
 Proof.
   buildPackG lower_letter lower_letter_rel lower_letter__lower_letter_rel lower_letter_rel_funct.
 Defined.
@@ -5135,15 +5184,15 @@ Defined.
 
 #[global] Hint Unfold Grade: ref_constr_db.
 
-Definition lower_grade_spec (ds_d5Rw : Grades): Type :=
+Definition lower_grade_spec (ds_d5Sh : Grades): Type :=
   Grades.
 
 #[global] Hint Unfold lower_grade_spec: lia_unfold.
 
-Definition lower_grade (ds_d5Rw : Grades): lower_grade_spec ds_d5Rw.
+Definition lower_grade (ds_d5Sh : Grades): lower_grade_spec ds_d5Sh.
 Proof.
-  destruct ds_d5Rw as [ds_d5Rw ds_d5Rw_p].
-  destruct ds_d5Rw as [l m].
+  destruct ds_d5Sh as [ds_d5Sh ds_d5Sh_p].
+  destruct ds_d5Sh as [l m].
   - destruct m as [| |].
     + destruct l as [| | | |].
       * refine (Grade (lower_letter A) Plus).
@@ -5179,10 +5228,10 @@ Inductive lower_grade_rel: Grades_u → Grades_u → Prop :=
 
 #[global] Instance lower_grade_getF: getFunc lower_grade_rel := { getF' := lower_grade }.
 
-Theorem lower_grade_rel_funct [ds_d5Rw : Grades_u]:
-  ∀ (VV VV' : Grades_u), lower_grade_rel ds_d5Rw VV → (lower_grade_rel ds_d5Rw VV' → VV = VV').
+Theorem lower_grade_rel_funct [ds_d5Sh : Grades_u]:
+  ∀ (VV VV' : Grades_u), lower_grade_rel ds_d5Sh VV → (lower_grade_rel ds_d5Sh VV' → VV = VV').
 Proof.
-  destruct ds_d5Rw as [l m];
+  destruct ds_d5Sh as [l m];
   [destruct m as [| |];
    [destruct l as [| | | |] |  |]];
   rel_functionhood_body.
@@ -5264,12 +5313,12 @@ Qed.
 
 #[global] Hint Rewrite lower_grade__Grade_x_Plus_lem: f_rel_back.
 
-Theorem lower_grade_rel_ex (ds_d5Rw : Grades_u) (ds_d5Rw_p : Grades_wf ds_d5Rw ∧ True):
-  lower_grade_rel ds_d5Rw ⌊ lower_grade (exist _ ds_d5Rw ds_d5Rw_p) -⌋.
+Theorem lower_grade_rel_ex (ds_d5Sh : Grades_u) (ds_d5Sh_p : Grades_wf ds_d5Sh ∧ True):
+  lower_grade_rel ds_d5Sh ⌊ lower_grade (exist _ ds_d5Sh ds_d5Sh_p) -⌋.
 Proof.
   Opaque lower_grade.
   existence_lemma_pre lower_grade;
-  destruct ds_d5Rw as [l m];
+  destruct ds_d5Sh as [l m];
   [destruct m as [| |];
    [destruct l as [| | | |];
     [fix_notations | fix_notations | fix_notations | fix_notations | fix_notations] |
@@ -5285,8 +5334,8 @@ Qed.
 #[global] Opaque lower_grade.
 
 Theorem lower_grade__lower_grade_rel_rw
-  (ds_d5Rw : Grades_u) (ds_d5Rw_p : Grades_wf ds_d5Rw ∧ True) (VV : Grades_u):
-  ⌊ lower_grade (exist _ ds_d5Rw ds_d5Rw_p) -⌋ = VV ↔ lower_grade_rel ds_d5Rw VV.
+  (ds_d5Sh : Grades_u) (ds_d5Sh_p : Grades_wf ds_d5Sh ∧ True) (VV : Grades_u):
+  ⌊ lower_grade (exist _ ds_d5Sh ds_d5Sh_p) -⌋ = VV ↔ lower_grade_rel ds_d5Sh VV.
 Proof.
   f__f_rel_rw.
 Qed.
@@ -5298,30 +5347,30 @@ Qed.
 #[global] Instance lower_grade_lookup_rw: dictionary rwLem lower_grade := {
     lookup' := lower_grade__lower_grade_rel_rw }.
 
-Theorem lower_grade__lower_grade_rel (ds_d5Rw : Grades) (VV : Grades_u):
-  ⌊ lower_grade ds_d5Rw -⌋ = VV ↔ lower_grade_rel ⌊ ds_d5Rw ⌋ VV.
+Theorem lower_grade__lower_grade_rel (ds_d5Sh : Grades) (VV : Grades_u):
+  ⌊ lower_grade ds_d5Sh -⌋ = VV ↔ lower_grade_rel ⌊ ds_d5Sh ⌋ VV.
 Proof.
   f__f_rel.
 Qed.
 
 #[global] Hint Rewrite lower_grade__lower_grade_rel: f_rel_funct_db.
 
-Theorem lower_grade__lower_grade_rel' (ds_d5Rw_u : Grades_u) (ds_d5Rw : Grades) (VV : Grades_u):
-  ds_d5Rw_u = ⌊ ds_d5Rw ⌋ → ⌊ lower_grade ds_d5Rw -⌋ = VV ↔ lower_grade_rel ds_d5Rw_u VV.
+Theorem lower_grade__lower_grade_rel' (ds_d5Sh_u : Grades_u) (ds_d5Sh : Grades) (VV : Grades_u):
+  ds_d5Sh_u = ⌊ ds_d5Sh ⌋ → ⌊ lower_grade ds_d5Sh -⌋ = VV ↔ lower_grade_rel ds_d5Sh_u VV.
 Proof.
-  intros ->. refine (lower_grade__lower_grade_rel ds_d5Rw VV).
+  intros ->. refine (lower_grade__lower_grade_rel ds_d5Sh VV).
 Qed.
 
 #[global] Hint Resolve lower_grade__lower_grade_rel': f_rel_funct_db.
 
-Theorem lower_grade_rel_mk (ds_d5Rw : Grades_u) (ds_d5Rw_p : Grades_wf ds_d5Rw ∧ True):
-  {VV: _ | lower_grade_rel ds_d5Rw VV}.
+Theorem lower_grade_rel_mk (ds_d5Sh : Grades_u) (ds_d5Sh_p : Grades_wf ds_d5Sh ∧ True):
+  {VV: _ | lower_grade_rel ds_d5Sh VV}.
 Proof.
   intros;
   refine (subsumptionCast
           _
-          (λ VV, lower_grade_rel ds_d5Rw VV)
-          (lower_grade (exist _ ds_d5Rw ds_d5Rw_p))
+          (λ VV, lower_grade_rel ds_d5Sh VV)
+          (lower_grade (exist _ ds_d5Sh ds_d5Sh_p))
           _);
   rewrite <- lower_grade__lower_grade_rel';
   quicksolve.
@@ -5331,12 +5380,12 @@ Qed.
 
 #[global] Instance lower_grade_pack:
   @Pack
-  (Grades ::RT λ (ds_d5Rw : Grades), nilRT)
+  (Grades ::RT λ (ds_d5Sh : Grades), nilRT)
   (Grades_u ::UT nilUT)
-  ltac:(mkProjectsArgListTG (Grades ::RT λ (ds_d5Rw : Grades), nilRT) ((Grades_u ::UT nilUT)))
+  ltac:(mkProjectsArgListTG (Grades ::RT λ (ds_d5Sh : Grades), nilRT) ((Grades_u ::UT nilUT)))
   Grades_u
-  (λ (x_83185053 : ArgList (Grades ::RT λ (ds_d5Rw : Grades), nilRT)) (v_x_83185053 : Grades_u),
-   ltac:(flattenP (λ (ds_d5Rw : Grades) (VV : Grades_u), Grades_wf VV ∧ True) x_83185053 v_x_83185053)).
+  (λ (x_82546053 : ArgList (Grades ::RT λ (ds_d5Sh : Grades), nilRT)) (v_x_82546053 : Grades_u),
+   ltac:(flattenP (λ (ds_d5Sh : Grades) (VV : Grades_u), Grades_wf VV ∧ True) x_82546053 v_x_82546053)).
 Proof.
   buildPackG lower_grade lower_grade_rel lower_grade__lower_grade_rel lower_grade_rel_funct.
 Defined.
@@ -5783,15 +5832,15 @@ Definition Wednesday : Day :=
 
 #[global] Hint Unfold Wednesday: ref_constr_db.
 
-Definition next_weekday_spec (ds_d5Tw : Day): Type :=
+Definition next_weekday_spec (ds_d5Uh : Day): Type :=
   Day.
 
 #[global] Hint Unfold next_weekday_spec: lia_unfold.
 
-Definition next_weekday (ds_d5Tw : Day): next_weekday_spec ds_d5Tw.
+Definition next_weekday (ds_d5Uh : Day): next_weekday_spec ds_d5Uh.
 Proof.
-  destruct ds_d5Tw as [ds_d5Tw ds_d5Tw_p].
-  destruct ds_d5Tw as [| | | | | |].
+  destruct ds_d5Uh as [ds_d5Uh ds_d5Uh_p].
+  destruct ds_d5Uh as [| | | | | |].
   - refine Monday.
   - refine Tuesday.
   - refine Monday.
@@ -5817,10 +5866,10 @@ Inductive next_weekday_rel: Day_u → Day_u → Prop :=
 
 #[global] Instance next_weekday_getF: getFunc next_weekday_rel := { getF' := next_weekday }.
 
-Theorem next_weekday_rel_funct [ds_d5Tw : Day_u]:
-  ∀ (VV VV' : Day_u), next_weekday_rel ds_d5Tw VV → (next_weekday_rel ds_d5Tw VV' → VV = VV').
+Theorem next_weekday_rel_funct [ds_d5Uh : Day_u]:
+  ∀ (VV VV' : Day_u), next_weekday_rel ds_d5Uh VV → (next_weekday_rel ds_d5Uh VV' → VV = VV').
 Proof.
-  destruct ds_d5Tw as [| | | | | |]; rel_functionhood_body.
+  destruct ds_d5Uh as [| | | | | |]; rel_functionhood_body.
 Qed.
 
 #[global] Hint Resolve next_weekday_rel_funct: f_rel_funct_db.
@@ -5888,12 +5937,12 @@ Qed.
 
 #[global] Hint Rewrite next_weekday_Wednesday_lem: f_rel_back.
 
-Theorem next_weekday_rel_ex (ds_d5Tw : Day_u) (ds_d5Tw_p : Day_wf ds_d5Tw ∧ True):
-  next_weekday_rel ds_d5Tw ⌊ next_weekday (exist _ ds_d5Tw ds_d5Tw_p) -⌋.
+Theorem next_weekday_rel_ex (ds_d5Uh : Day_u) (ds_d5Uh_p : Day_wf ds_d5Uh ∧ True):
+  next_weekday_rel ds_d5Uh ⌊ next_weekday (exist _ ds_d5Uh ds_d5Uh_p) -⌋.
 Proof.
   Opaque next_weekday.
   existence_lemma_pre next_weekday;
-  destruct ds_d5Tw as [| | | | | |];
+  destruct ds_d5Uh as [| | | | | |];
   [fix_notations |
    fix_notations |
    fix_notations |
@@ -5911,8 +5960,8 @@ Qed.
 #[global] Opaque next_weekday.
 
 Theorem next_weekday__next_weekday_rel_rw
-  (ds_d5Tw : Day_u) (ds_d5Tw_p : Day_wf ds_d5Tw ∧ True) (VV : Day_u):
-  ⌊ next_weekday (exist _ ds_d5Tw ds_d5Tw_p) -⌋ = VV ↔ next_weekday_rel ds_d5Tw VV.
+  (ds_d5Uh : Day_u) (ds_d5Uh_p : Day_wf ds_d5Uh ∧ True) (VV : Day_u):
+  ⌊ next_weekday (exist _ ds_d5Uh ds_d5Uh_p) -⌋ = VV ↔ next_weekday_rel ds_d5Uh VV.
 Proof.
   f__f_rel_rw.
 Qed.
@@ -5924,30 +5973,30 @@ Qed.
 #[global] Instance next_weekday_lookup_rw: dictionary rwLem next_weekday := {
     lookup' := next_weekday__next_weekday_rel_rw }.
 
-Theorem next_weekday__next_weekday_rel (ds_d5Tw : Day) (VV : Day_u):
-  ⌊ next_weekday ds_d5Tw -⌋ = VV ↔ next_weekday_rel ⌊ ds_d5Tw ⌋ VV.
+Theorem next_weekday__next_weekday_rel (ds_d5Uh : Day) (VV : Day_u):
+  ⌊ next_weekday ds_d5Uh -⌋ = VV ↔ next_weekday_rel ⌊ ds_d5Uh ⌋ VV.
 Proof.
   f__f_rel.
 Qed.
 
 #[global] Hint Rewrite next_weekday__next_weekday_rel: f_rel_funct_db.
 
-Theorem next_weekday__next_weekday_rel' (ds_d5Tw_u : Day_u) (ds_d5Tw : Day) (VV : Day_u):
-  ds_d5Tw_u = ⌊ ds_d5Tw ⌋ → ⌊ next_weekday ds_d5Tw -⌋ = VV ↔ next_weekday_rel ds_d5Tw_u VV.
+Theorem next_weekday__next_weekday_rel' (ds_d5Uh_u : Day_u) (ds_d5Uh : Day) (VV : Day_u):
+  ds_d5Uh_u = ⌊ ds_d5Uh ⌋ → ⌊ next_weekday ds_d5Uh -⌋ = VV ↔ next_weekday_rel ds_d5Uh_u VV.
 Proof.
-  intros ->. refine (next_weekday__next_weekday_rel ds_d5Tw VV).
+  intros ->. refine (next_weekday__next_weekday_rel ds_d5Uh VV).
 Qed.
 
 #[global] Hint Resolve next_weekday__next_weekday_rel': f_rel_funct_db.
 
-Theorem next_weekday_rel_mk (ds_d5Tw : Day_u) (ds_d5Tw_p : Day_wf ds_d5Tw ∧ True):
-  {VV: _ | next_weekday_rel ds_d5Tw VV}.
+Theorem next_weekday_rel_mk (ds_d5Uh : Day_u) (ds_d5Uh_p : Day_wf ds_d5Uh ∧ True):
+  {VV: _ | next_weekday_rel ds_d5Uh VV}.
 Proof.
   intros;
   refine (subsumptionCast
           _
-          (λ VV, next_weekday_rel ds_d5Tw VV)
-          (next_weekday (exist _ ds_d5Tw ds_d5Tw_p))
+          (λ VV, next_weekday_rel ds_d5Uh VV)
+          (next_weekday (exist _ ds_d5Uh ds_d5Uh_p))
           _);
   rewrite <- next_weekday__next_weekday_rel';
   quicksolve.
@@ -5957,12 +6006,12 @@ Qed.
 
 #[global] Instance next_weekday_pack:
   @Pack
-  (Day ::RT λ (ds_d5Tw : Day), nilRT)
+  (Day ::RT λ (ds_d5Uh : Day), nilRT)
   (Day_u ::UT nilUT)
-  ltac:(mkProjectsArgListTG (Day ::RT λ (ds_d5Tw : Day), nilRT) ((Day_u ::UT nilUT)))
+  ltac:(mkProjectsArgListTG (Day ::RT λ (ds_d5Uh : Day), nilRT) ((Day_u ::UT nilUT)))
   Day_u
-  (λ (x_27400349 : ArgList (Day ::RT λ (ds_d5Tw : Day), nilRT)) (v_x_27400349 : Day_u),
-   ltac:(flattenP (λ (ds_d5Tw : Day) (VV : Day_u), Day_wf VV ∧ True) x_27400349 v_x_27400349)).
+  (λ (x_21463735 : ArgList (Day ::RT λ (ds_d5Uh : Day), nilRT)) (v_x_21463735 : Day_u),
+   ltac:(flattenP (λ (ds_d5Uh : Day) (VV : Day_u), Day_wf VV ∧ True) x_21463735 v_x_21463735)).
 Proof.
   buildPackG next_weekday next_weekday_rel next_weekday__next_weekday_rel next_weekday_rel_funct.
 Defined.
@@ -6071,41 +6120,41 @@ Definition Lt : Comparison :=
 
 #[global] Hint Unfold Lt: ref_constr_db.
 
-Definition letter_comparison_spec (ds_d5RU ds_d5RV : Letter): Type :=
+Definition letter_comparison_spec (ds_d5SF ds_d5SG : Letter): Type :=
   Comparison.
 
 #[global] Hint Unfold letter_comparison_spec: lia_unfold.
 
-Definition letter_comparison (ds_d5RU ds_d5RV : Letter): letter_comparison_spec ds_d5RU ds_d5RV.
+Definition letter_comparison (ds_d5SF ds_d5SG : Letter): letter_comparison_spec ds_d5SF ds_d5SG.
 Proof.
-  destruct ds_d5RU as [ds_d5RU ds_d5RU_p].
-  destruct ds_d5RV as [ds_d5RV ds_d5RV_p].
-  destruct ds_d5RU as [| | | |].
-  - destruct ds_d5RV as [| | | |].
+  destruct ds_d5SF as [ds_d5SF ds_d5SF_p].
+  destruct ds_d5SG as [ds_d5SG ds_d5SG_p].
+  destruct ds_d5SF as [| | | |].
+  - destruct ds_d5SG as [| | | |].
     + refine Eq.
     + refine Gt.
     + refine Gt.
     + refine Gt.
     + refine Gt.
-  - destruct ds_d5RV as [| | | |].
+  - destruct ds_d5SG as [| | | |].
     + refine Lt.
     + refine Eq.
     + refine Gt.
     + refine Gt.
     + refine Gt.
-  - destruct ds_d5RV as [| | | |].
+  - destruct ds_d5SG as [| | | |].
     + refine Lt.
     + refine Lt.
     + refine Eq.
     + refine Gt.
     + refine Gt.
-  - destruct ds_d5RV as [| | | |].
+  - destruct ds_d5SG as [| | | |].
     + refine Lt.
     + refine Lt.
     + refine Lt.
     + refine Eq.
     + refine Gt.
-  - destruct ds_d5RV as [| | | |].
+  - destruct ds_d5SG as [| | | |].
     + refine Lt.
     + refine Lt.
     + refine Lt.
@@ -6148,16 +6197,16 @@ Inductive letter_comparison_rel: Letter_u → Letter_u → Comparison_u → Prop
 #[global] Instance letter_comparison_getF: getFunc letter_comparison_rel := {
     getF' := letter_comparison }.
 
-Theorem letter_comparison_rel_funct [ds_d5RU ds_d5RV : Letter_u]:
+Theorem letter_comparison_rel_funct [ds_d5SF ds_d5SG : Letter_u]:
   ∀ (VV VV' : Comparison_u),
-  letter_comparison_rel ds_d5RU ds_d5RV VV → (letter_comparison_rel ds_d5RU ds_d5RV VV' → VV = VV').
+  letter_comparison_rel ds_d5SF ds_d5SG VV → (letter_comparison_rel ds_d5SF ds_d5SG VV' → VV = VV').
 Proof.
-  destruct ds_d5RU as [| | | |];
-  [destruct ds_d5RV as [| | | |] |
-   destruct ds_d5RV as [| | | |] |
-   destruct ds_d5RV as [| | | |] |
-   destruct ds_d5RV as [| | | |] |
-   destruct ds_d5RV as [| | | |]];
+  destruct ds_d5SF as [| | | |];
+  [destruct ds_d5SG as [| | | |] |
+   destruct ds_d5SG as [| | | |] |
+   destruct ds_d5SG as [| | | |] |
+   destruct ds_d5SG as [| | | |] |
+   destruct ds_d5SG as [| | | |]];
   rel_functionhood_body.
 Qed.
 
@@ -6367,27 +6416,27 @@ Qed.
 #[global] Hint Rewrite letter_comparison_F_F_lem: f_rel_back.
 
 Theorem letter_comparison_rel_ex
-  (ds_d5RU : Letter_u)
-  (ds_d5RU_p : Letter_wf ds_d5RU ∧ True)
-  (ds_d5RV : Letter_u)
-  (ds_d5RV_p : Letter_wf ds_d5RV ∧ True):
+  (ds_d5SF : Letter_u)
+  (ds_d5SF_p : Letter_wf ds_d5SF ∧ True)
+  (ds_d5SG : Letter_u)
+  (ds_d5SG_p : Letter_wf ds_d5SG ∧ True):
   letter_comparison_rel
-  ds_d5RU
-  ds_d5RV
-  ⌊ letter_comparison (exist _ ds_d5RU ds_d5RU_p) (exist _ ds_d5RV ds_d5RV_p) -⌋.
+  ds_d5SF
+  ds_d5SG
+  ⌊ letter_comparison (exist _ ds_d5SF ds_d5SF_p) (exist _ ds_d5SG ds_d5SG_p) -⌋.
 Proof.
   Opaque letter_comparison.
   existence_lemma_pre letter_comparison;
-  destruct ds_d5RU as [| | | |];
-  [destruct ds_d5RV as [| | | |];
+  destruct ds_d5SF as [| | | |];
+  [destruct ds_d5SG as [| | | |];
    [fix_notations | fix_notations | fix_notations | fix_notations | fix_notations] |
-   destruct ds_d5RV as [| | | |];
+   destruct ds_d5SG as [| | | |];
    [fix_notations | fix_notations | fix_notations | fix_notations | fix_notations] |
-   destruct ds_d5RV as [| | | |];
+   destruct ds_d5SG as [| | | |];
    [fix_notations | fix_notations | fix_notations | fix_notations | fix_notations] |
-   destruct ds_d5RV as [| | | |];
+   destruct ds_d5SG as [| | | |];
    [fix_notations | fix_notations | fix_notations | fix_notations | fix_notations] |
-   destruct ds_d5RV as [| | | |];
+   destruct ds_d5SG as [| | | |];
    [fix_notations | fix_notations | fix_notations | fix_notations | fix_notations]];
   simpl in *.
   Transparent letter_comparison.
@@ -6399,13 +6448,13 @@ Qed.
 #[global] Opaque letter_comparison.
 
 Theorem letter_comparison__letter_comparison_rel_rw
-  (ds_d5RU : Letter_u)
-  (ds_d5RU_p : Letter_wf ds_d5RU ∧ True)
-  (ds_d5RV : Letter_u)
-  (ds_d5RV_p : Letter_wf ds_d5RV ∧ True)
+  (ds_d5SF : Letter_u)
+  (ds_d5SF_p : Letter_wf ds_d5SF ∧ True)
+  (ds_d5SG : Letter_u)
+  (ds_d5SG_p : Letter_wf ds_d5SG ∧ True)
   (VV : Comparison_u):
-  ⌊ letter_comparison (exist _ ds_d5RU ds_d5RU_p) (exist _ ds_d5RV ds_d5RV_p) -⌋ = VV
-  ↔ letter_comparison_rel ds_d5RU ds_d5RV VV.
+  ⌊ letter_comparison (exist _ ds_d5SF ds_d5SF_p) (exist _ ds_d5SG ds_d5SG_p) -⌋ = VV
+  ↔ letter_comparison_rel ds_d5SF ds_d5SG VV.
 Proof.
   f__f_rel_rw.
 Qed.
@@ -6417,8 +6466,8 @@ Qed.
 #[global] Instance letter_comparison_lookup_rw: dictionary rwLem letter_comparison := {
     lookup' := letter_comparison__letter_comparison_rel_rw }.
 
-Theorem letter_comparison__letter_comparison_rel (ds_d5RU ds_d5RV : Letter) (VV : Comparison_u):
-  ⌊ letter_comparison ds_d5RU ds_d5RV -⌋ = VV ↔ letter_comparison_rel ⌊ ds_d5RU ⌋ ⌊ ds_d5RV ⌋ VV.
+Theorem letter_comparison__letter_comparison_rel (ds_d5SF ds_d5SG : Letter) (VV : Comparison_u):
+  ⌊ letter_comparison ds_d5SF ds_d5SG -⌋ = VV ↔ letter_comparison_rel ⌊ ds_d5SF ⌋ ⌊ ds_d5SG ⌋ VV.
 Proof.
   f__f_rel.
 Qed.
@@ -6426,28 +6475,28 @@ Qed.
 #[global] Hint Rewrite letter_comparison__letter_comparison_rel: f_rel_funct_db.
 
 Theorem letter_comparison__letter_comparison_rel'
-  (ds_d5RU_u ds_d5RV_u : Letter_u) (ds_d5RU ds_d5RV : Letter) (VV : Comparison_u):
-  ds_d5RU_u = ⌊ ds_d5RU ⌋
-  → (ds_d5RV_u = ⌊ ds_d5RV ⌋
-     → ⌊ letter_comparison ds_d5RU ds_d5RV -⌋ = VV ↔ letter_comparison_rel ds_d5RU_u ds_d5RV_u VV).
+  (ds_d5SF_u ds_d5SG_u : Letter_u) (ds_d5SF ds_d5SG : Letter) (VV : Comparison_u):
+  ds_d5SF_u = ⌊ ds_d5SF ⌋
+  → (ds_d5SG_u = ⌊ ds_d5SG ⌋
+     → ⌊ letter_comparison ds_d5SF ds_d5SG -⌋ = VV ↔ letter_comparison_rel ds_d5SF_u ds_d5SG_u VV).
 Proof.
-  intros -> ->. refine (letter_comparison__letter_comparison_rel ds_d5RU ds_d5RV VV).
+  intros -> ->. refine (letter_comparison__letter_comparison_rel ds_d5SF ds_d5SG VV).
 Qed.
 
 #[global] Hint Resolve letter_comparison__letter_comparison_rel': f_rel_funct_db.
 
 Theorem letter_comparison_rel_mk
-  (ds_d5RU : Letter_u)
-  (ds_d5RU_p : Letter_wf ds_d5RU ∧ True)
-  (ds_d5RV : Letter_u)
-  (ds_d5RV_p : Letter_wf ds_d5RV ∧ True):
-  {VV: _ | letter_comparison_rel ds_d5RU ds_d5RV VV}.
+  (ds_d5SF : Letter_u)
+  (ds_d5SF_p : Letter_wf ds_d5SF ∧ True)
+  (ds_d5SG : Letter_u)
+  (ds_d5SG_p : Letter_wf ds_d5SG ∧ True):
+  {VV: _ | letter_comparison_rel ds_d5SF ds_d5SG VV}.
 Proof.
   intros;
   refine (subsumptionCast
           _
-          (λ VV, letter_comparison_rel ds_d5RU ds_d5RV VV)
-          (letter_comparison (exist _ ds_d5RU ds_d5RU_p) (exist _ ds_d5RV ds_d5RV_p))
+          (λ VV, letter_comparison_rel ds_d5SF ds_d5SG VV)
+          (letter_comparison (exist _ ds_d5SF ds_d5SF_p) (exist _ ds_d5SG ds_d5SG_p))
           _);
   rewrite <- letter_comparison__letter_comparison_rel';
   quicksolve.
@@ -6457,16 +6506,16 @@ Qed.
 
 #[global] Instance letter_comparison_pack:
   @Pack
-  (Letter ::RT λ (ds_d5RU : Letter), Letter ::RT λ (ds_d5RV : Letter), nilRT)
+  (Letter ::RT λ (ds_d5SF : Letter), Letter ::RT λ (ds_d5SG : Letter), nilRT)
   (Letter_u ::UT (Letter_u ::UT nilUT))
   ltac:(mkProjectsArgListTG (Letter
- ::RT λ (ds_d5RU : Letter), Letter ::RT λ (ds_d5RV : Letter), nilRT) ((Letter_u ::UT (Letter_u ::UT nilUT))))
+ ::RT λ (ds_d5SF : Letter), Letter ::RT λ (ds_d5SG : Letter), nilRT) ((Letter_u ::UT (Letter_u ::UT nilUT))))
   Comparison_u
-  (λ (x_68686692 : ArgList (Letter
-                            ::RT λ (ds_d5RU : Letter), Letter ::RT λ (ds_d5RV : Letter), nilRT))
-     (v_x_68686692 : Comparison_u),
-   ltac:(flattenP (λ (ds_d5RU ds_d5RV : Letter) (VV : Comparison_u),
- Comparison_wf VV ∧ True) x_68686692 v_x_68686692)).
+  (λ (x_91087192 : ArgList (Letter
+                            ::RT λ (ds_d5SF : Letter), Letter ::RT λ (ds_d5SG : Letter), nilRT))
+     (v_x_91087192 : Comparison_u),
+   ltac:(flattenP (λ (ds_d5SF ds_d5SG : Letter) (VV : Comparison_u),
+ Comparison_wf VV ∧ True) x_91087192 v_x_91087192)).
 Proof.
   buildPackG letter_comparison letter_comparison_rel letter_comparison__letter_comparison_rel letter_comparison_rel_funct.
 Defined.
@@ -6477,17 +6526,17 @@ Proof.
   buildUPackG letter_comparison_rel letter_comparison_rel_funct.
 Defined.
 
-Definition letter_comparison_eq_spec (ds_d5RT : Letter): Type :=
+Definition letter_comparison_eq_spec (ds_d5SE : Letter): Type :=
   {{∃ (letter_comparison_res : Comparison_u),
-    letter_comparison_rel ⌊ ds_d5RT -⌋ ⌊ ds_d5RT -⌋ letter_comparison_res
+    letter_comparison_rel ⌊ ds_d5SE -⌋ ⌊ ds_d5SE -⌋ letter_comparison_res
     ∧ letter_comparison_res == Eq_u}}.
 
 #[global] Hint Unfold letter_comparison_eq_spec: lia_unfold.
 
-Theorem letter_comparison_eq (ds_d5RT : Letter): letter_comparison_eq_spec ds_d5RT.
+Theorem letter_comparison_eq (ds_d5SE : Letter): letter_comparison_eq_spec ds_d5SE.
 Proof.
-  destruct ds_d5RT as [ds_d5RT ds_d5RT_p].
-  destruct ds_d5RT as [| | | |].
+  destruct ds_d5SE as [ds_d5SE ds_d5SE_p].
+  destruct ds_d5SE as [| | | |].
   - refine (subsumptionCast
             Unit
             (λ (VV : Unit),
@@ -6597,26 +6646,26 @@ Proof.
             ltac:(solver)).
 Qed.
 
-Definition modifier_comparison_spec (ds_d5RL ds_d5RM : Modifier): Type :=
+Definition modifier_comparison_spec (ds_d5Sw ds_d5Sx : Modifier): Type :=
   Comparison.
 
 #[global] Hint Unfold modifier_comparison_spec: lia_unfold.
 
-Definition modifier_comparison (ds_d5RL ds_d5RM : Modifier):
-  modifier_comparison_spec ds_d5RL ds_d5RM.
+Definition modifier_comparison (ds_d5Sw ds_d5Sx : Modifier):
+  modifier_comparison_spec ds_d5Sw ds_d5Sx.
 Proof.
-  destruct ds_d5RL as [ds_d5RL ds_d5RL_p].
-  destruct ds_d5RM as [ds_d5RM ds_d5RM_p].
-  destruct ds_d5RL as [| |].
-  - destruct ds_d5RM as [| |].
+  destruct ds_d5Sw as [ds_d5Sw ds_d5Sw_p].
+  destruct ds_d5Sx as [ds_d5Sx ds_d5Sx_p].
+  destruct ds_d5Sw as [| |].
+  - destruct ds_d5Sx as [| |].
     + refine Eq.
     + refine Lt.
     + refine Lt.
-  - destruct ds_d5RM as [| |].
+  - destruct ds_d5Sx as [| |].
     + refine Gt.
     + refine Eq.
     + refine Lt.
-  - destruct ds_d5RM as [| |].
+  - destruct ds_d5Sx as [| |].
     + refine Gt.
     + refine Gt.
     + refine Eq.
@@ -6641,13 +6690,13 @@ Inductive modifier_comparison_rel: Modifier_u → Modifier_u → Comparison_u �
 #[global] Instance modifier_comparison_getF: getFunc modifier_comparison_rel := {
     getF' := modifier_comparison }.
 
-Theorem modifier_comparison_rel_funct [ds_d5RL ds_d5RM : Modifier_u]:
+Theorem modifier_comparison_rel_funct [ds_d5Sw ds_d5Sx : Modifier_u]:
   ∀ (VV VV' : Comparison_u),
-  modifier_comparison_rel ds_d5RL ds_d5RM VV
-  → (modifier_comparison_rel ds_d5RL ds_d5RM VV' → VV = VV').
+  modifier_comparison_rel ds_d5Sw ds_d5Sx VV
+  → (modifier_comparison_rel ds_d5Sw ds_d5Sx VV' → VV = VV').
 Proof.
-  destruct ds_d5RL as [| |];
-  [destruct ds_d5RM as [| |] | destruct ds_d5RM as [| |] | destruct ds_d5RM as [| |]];
+  destruct ds_d5Sw as [| |];
+  [destruct ds_d5Sx as [| |] | destruct ds_d5Sx as [| |] | destruct ds_d5Sx as [| |]];
   rel_functionhood_body.
 Qed.
 
@@ -6738,23 +6787,23 @@ Qed.
 #[global] Hint Rewrite modifier_comparison_Plus_Plus_lem: f_rel_back.
 
 Theorem modifier_comparison_rel_ex
-  (ds_d5RL : Modifier_u)
-  (ds_d5RL_p : Modifier_wf ds_d5RL ∧ True)
-  (ds_d5RM : Modifier_u)
-  (ds_d5RM_p : Modifier_wf ds_d5RM ∧ True):
+  (ds_d5Sw : Modifier_u)
+  (ds_d5Sw_p : Modifier_wf ds_d5Sw ∧ True)
+  (ds_d5Sx : Modifier_u)
+  (ds_d5Sx_p : Modifier_wf ds_d5Sx ∧ True):
   modifier_comparison_rel
-  ds_d5RL
-  ds_d5RM
-  ⌊ modifier_comparison (exist _ ds_d5RL ds_d5RL_p) (exist _ ds_d5RM ds_d5RM_p) -⌋.
+  ds_d5Sw
+  ds_d5Sx
+  ⌊ modifier_comparison (exist _ ds_d5Sw ds_d5Sw_p) (exist _ ds_d5Sx ds_d5Sx_p) -⌋.
 Proof.
   Opaque modifier_comparison.
   existence_lemma_pre modifier_comparison;
-  destruct ds_d5RL as [| |];
-  [destruct ds_d5RM as [| |];
+  destruct ds_d5Sw as [| |];
+  [destruct ds_d5Sx as [| |];
    [fix_notations | fix_notations | fix_notations] |
-   destruct ds_d5RM as [| |];
+   destruct ds_d5Sx as [| |];
    [fix_notations | fix_notations | fix_notations] |
-   destruct ds_d5RM as [| |];
+   destruct ds_d5Sx as [| |];
    [fix_notations | fix_notations | fix_notations]];
   simpl in *.
   Transparent modifier_comparison.
@@ -6766,13 +6815,13 @@ Qed.
 #[global] Opaque modifier_comparison.
 
 Theorem modifier_comparison__modifier_comparison_rel_rw
-  (ds_d5RL : Modifier_u)
-  (ds_d5RL_p : Modifier_wf ds_d5RL ∧ True)
-  (ds_d5RM : Modifier_u)
-  (ds_d5RM_p : Modifier_wf ds_d5RM ∧ True)
+  (ds_d5Sw : Modifier_u)
+  (ds_d5Sw_p : Modifier_wf ds_d5Sw ∧ True)
+  (ds_d5Sx : Modifier_u)
+  (ds_d5Sx_p : Modifier_wf ds_d5Sx ∧ True)
   (VV : Comparison_u):
-  ⌊ modifier_comparison (exist _ ds_d5RL ds_d5RL_p) (exist _ ds_d5RM ds_d5RM_p) -⌋ = VV
-  ↔ modifier_comparison_rel ds_d5RL ds_d5RM VV.
+  ⌊ modifier_comparison (exist _ ds_d5Sw ds_d5Sw_p) (exist _ ds_d5Sx ds_d5Sx_p) -⌋ = VV
+  ↔ modifier_comparison_rel ds_d5Sw ds_d5Sx VV.
 Proof.
   f__f_rel_rw.
 Qed.
@@ -6785,8 +6834,8 @@ Qed.
     lookup' := modifier_comparison__modifier_comparison_rel_rw }.
 
 Theorem modifier_comparison__modifier_comparison_rel
-  (ds_d5RL ds_d5RM : Modifier) (VV : Comparison_u):
-  ⌊ modifier_comparison ds_d5RL ds_d5RM -⌋ = VV ↔ modifier_comparison_rel ⌊ ds_d5RL ⌋ ⌊ ds_d5RM ⌋ VV.
+  (ds_d5Sw ds_d5Sx : Modifier) (VV : Comparison_u):
+  ⌊ modifier_comparison ds_d5Sw ds_d5Sx -⌋ = VV ↔ modifier_comparison_rel ⌊ ds_d5Sw ⌋ ⌊ ds_d5Sx ⌋ VV.
 Proof.
   f__f_rel.
 Qed.
@@ -6794,28 +6843,28 @@ Qed.
 #[global] Hint Rewrite modifier_comparison__modifier_comparison_rel: f_rel_funct_db.
 
 Theorem modifier_comparison__modifier_comparison_rel'
-  (ds_d5RL_u ds_d5RM_u : Modifier_u) (ds_d5RL ds_d5RM : Modifier) (VV : Comparison_u):
-  ds_d5RL_u = ⌊ ds_d5RL ⌋
-  → (ds_d5RM_u = ⌊ ds_d5RM ⌋
-     → ⌊ modifier_comparison ds_d5RL ds_d5RM -⌋ = VV ↔ modifier_comparison_rel ds_d5RL_u ds_d5RM_u VV).
+  (ds_d5Sw_u ds_d5Sx_u : Modifier_u) (ds_d5Sw ds_d5Sx : Modifier) (VV : Comparison_u):
+  ds_d5Sw_u = ⌊ ds_d5Sw ⌋
+  → (ds_d5Sx_u = ⌊ ds_d5Sx ⌋
+     → ⌊ modifier_comparison ds_d5Sw ds_d5Sx -⌋ = VV ↔ modifier_comparison_rel ds_d5Sw_u ds_d5Sx_u VV).
 Proof.
-  intros -> ->. refine (modifier_comparison__modifier_comparison_rel ds_d5RL ds_d5RM VV).
+  intros -> ->. refine (modifier_comparison__modifier_comparison_rel ds_d5Sw ds_d5Sx VV).
 Qed.
 
 #[global] Hint Resolve modifier_comparison__modifier_comparison_rel': f_rel_funct_db.
 
 Theorem modifier_comparison_rel_mk
-  (ds_d5RL : Modifier_u)
-  (ds_d5RL_p : Modifier_wf ds_d5RL ∧ True)
-  (ds_d5RM : Modifier_u)
-  (ds_d5RM_p : Modifier_wf ds_d5RM ∧ True):
-  {VV: _ | modifier_comparison_rel ds_d5RL ds_d5RM VV}.
+  (ds_d5Sw : Modifier_u)
+  (ds_d5Sw_p : Modifier_wf ds_d5Sw ∧ True)
+  (ds_d5Sx : Modifier_u)
+  (ds_d5Sx_p : Modifier_wf ds_d5Sx ∧ True):
+  {VV: _ | modifier_comparison_rel ds_d5Sw ds_d5Sx VV}.
 Proof.
   intros;
   refine (subsumptionCast
           _
-          (λ VV, modifier_comparison_rel ds_d5RL ds_d5RM VV)
-          (modifier_comparison (exist _ ds_d5RL ds_d5RL_p) (exist _ ds_d5RM ds_d5RM_p))
+          (λ VV, modifier_comparison_rel ds_d5Sw ds_d5Sx VV)
+          (modifier_comparison (exist _ ds_d5Sw ds_d5Sw_p) (exist _ ds_d5Sx ds_d5Sx_p))
           _);
   rewrite <- modifier_comparison__modifier_comparison_rel';
   quicksolve.
@@ -6825,17 +6874,17 @@ Qed.
 
 #[global] Instance modifier_comparison_pack:
   @Pack
-  (Modifier ::RT λ (ds_d5RL : Modifier), Modifier ::RT λ (ds_d5RM : Modifier), nilRT)
+  (Modifier ::RT λ (ds_d5Sw : Modifier), Modifier ::RT λ (ds_d5Sx : Modifier), nilRT)
   (Modifier_u ::UT (Modifier_u ::UT nilUT))
   ltac:(mkProjectsArgListTG (Modifier
- ::RT λ (ds_d5RL : Modifier),
-      Modifier ::RT λ (ds_d5RM : Modifier), nilRT) ((Modifier_u ::UT (Modifier_u ::UT nilUT))))
+ ::RT λ (ds_d5Sw : Modifier),
+      Modifier ::RT λ (ds_d5Sx : Modifier), nilRT) ((Modifier_u ::UT (Modifier_u ::UT nilUT))))
   Comparison_u
-  (λ (x_86702359 : ArgList (Modifier
-                            ::RT λ (ds_d5RL : Modifier), Modifier ::RT λ (ds_d5RM : Modifier), nilRT))
-     (v_x_86702359 : Comparison_u),
-   ltac:(flattenP (λ (ds_d5RL ds_d5RM : Modifier) (VV : Comparison_u),
- Comparison_wf VV ∧ True) x_86702359 v_x_86702359)).
+  (λ (x_24508278 : ArgList (Modifier
+                            ::RT λ (ds_d5Sw : Modifier), Modifier ::RT λ (ds_d5Sx : Modifier), nilRT))
+     (v_x_24508278 : Comparison_u),
+   ltac:(flattenP (λ (ds_d5Sw ds_d5Sx : Modifier) (VV : Comparison_u),
+ Comparison_wf VV ∧ True) x_24508278 v_x_24508278)).
 Proof.
   buildPackG modifier_comparison modifier_comparison_rel modifier_comparison__modifier_comparison_rel modifier_comparison_rel_funct.
 Defined.
@@ -6929,32 +6978,32 @@ Defined.
 
 #[global] Hint Unfold White: ref_constr_db.
 
-Definition isred_spec (ds_d5T9 : Color): Type :=
+Definition isred_spec (ds_d5TU : Color): Type :=
   SFBool.
 
 #[global] Hint Unfold isred_spec: lia_unfold.
 
-Definition isred (ds_d5T9 : Color): isred_spec ds_d5T9.
+Definition isred (ds_d5TU : Color): isred_spec ds_d5TU.
 Proof.
-  destruct ds_d5T9 as [ds_d5T9 ds_d5T9_p].
-  destruct ds_d5T9 as [| ds_d5Ta|].
+  destruct ds_d5TU as [ds_d5TU ds_d5TU_p].
+  destruct ds_d5TU as [| ds_d5TV|].
   - refine SFFalse.
-  - destruct ds_d5Ta as [| |].
+  - destruct ds_d5TV as [| |].
     + refine SFFalse.
     + refine SFFalse.
     + refine SFTrue.
   - refine SFFalse.
 Defined.
 
-Definition monochrome_spec (ds_d5Tf : Color): Type :=
+Definition monochrome_spec (ds_d5U0 : Color): Type :=
   SFBool.
 
 #[global] Hint Unfold monochrome_spec: lia_unfold.
 
-Definition monochrome (ds_d5Tf : Color): monochrome_spec ds_d5Tf.
+Definition monochrome (ds_d5U0 : Color): monochrome_spec ds_d5U0.
 Proof.
-  destruct ds_d5Tf as [ds_d5Tf ds_d5Tf_p].
-  destruct ds_d5Tf as [| p|].
+  destruct ds_d5U0 as [ds_d5U0 ds_d5U0_p].
+  destruct ds_d5U0 as [| p|].
   - refine SFTrue.
   - refine SFFalse.
   - refine SFTrue.
@@ -6972,10 +7021,10 @@ Inductive monochrome_rel: Color_u → SFBool_u → Prop :=
 
 #[global] Instance monochrome_getF: getFunc monochrome_rel := { getF' := monochrome }.
 
-Theorem monochrome_rel_funct [ds_d5Tf : Color_u]:
-  ∀ (VV VV' : SFBool_u), monochrome_rel ds_d5Tf VV → (monochrome_rel ds_d5Tf VV' → VV = VV').
+Theorem monochrome_rel_funct [ds_d5U0 : Color_u]:
+  ∀ (VV VV' : SFBool_u), monochrome_rel ds_d5U0 VV → (monochrome_rel ds_d5U0 VV' → VV = VV').
 Proof.
-  destruct ds_d5Tf as [| p|]; rel_functionhood_body.
+  destruct ds_d5U0 as [| p|]; rel_functionhood_body.
 Qed.
 
 #[global] Hint Resolve monochrome_rel_funct: f_rel_funct_db.
@@ -7007,12 +7056,12 @@ Qed.
 
 #[global] Hint Rewrite monochrome_White_lem: f_rel_back.
 
-Theorem monochrome_rel_ex (ds_d5Tf : Color_u) (ds_d5Tf_p : Color_wf ds_d5Tf ∧ True):
-  monochrome_rel ds_d5Tf ⌊ monochrome (exist _ ds_d5Tf ds_d5Tf_p) -⌋.
+Theorem monochrome_rel_ex (ds_d5U0 : Color_u) (ds_d5U0_p : Color_wf ds_d5U0 ∧ True):
+  monochrome_rel ds_d5U0 ⌊ monochrome (exist _ ds_d5U0 ds_d5U0_p) -⌋.
 Proof.
   Opaque monochrome.
   existence_lemma_pre monochrome;
-  destruct ds_d5Tf as [| p|];
+  destruct ds_d5U0 as [| p|];
   [fix_notations | fix_notations | fix_notations];
   simpl in *.
   Transparent monochrome.
@@ -7024,8 +7073,8 @@ Qed.
 #[global] Opaque monochrome.
 
 Theorem monochrome__monochrome_rel_rw
-  (ds_d5Tf : Color_u) (ds_d5Tf_p : Color_wf ds_d5Tf ∧ True) (VV : SFBool_u):
-  ⌊ monochrome (exist _ ds_d5Tf ds_d5Tf_p) -⌋ = VV ↔ monochrome_rel ds_d5Tf VV.
+  (ds_d5U0 : Color_u) (ds_d5U0_p : Color_wf ds_d5U0 ∧ True) (VV : SFBool_u):
+  ⌊ monochrome (exist _ ds_d5U0 ds_d5U0_p) -⌋ = VV ↔ monochrome_rel ds_d5U0 VV.
 Proof.
   f__f_rel_rw.
 Qed.
@@ -7037,30 +7086,30 @@ Qed.
 #[global] Instance monochrome_lookup_rw: dictionary rwLem monochrome := {
     lookup' := monochrome__monochrome_rel_rw }.
 
-Theorem monochrome__monochrome_rel (ds_d5Tf : Color) (VV : SFBool_u):
-  ⌊ monochrome ds_d5Tf -⌋ = VV ↔ monochrome_rel ⌊ ds_d5Tf ⌋ VV.
+Theorem monochrome__monochrome_rel (ds_d5U0 : Color) (VV : SFBool_u):
+  ⌊ monochrome ds_d5U0 -⌋ = VV ↔ monochrome_rel ⌊ ds_d5U0 ⌋ VV.
 Proof.
   f__f_rel.
 Qed.
 
 #[global] Hint Rewrite monochrome__monochrome_rel: f_rel_funct_db.
 
-Theorem monochrome__monochrome_rel' (ds_d5Tf_u : Color_u) (ds_d5Tf : Color) (VV : SFBool_u):
-  ds_d5Tf_u = ⌊ ds_d5Tf ⌋ → ⌊ monochrome ds_d5Tf -⌋ = VV ↔ monochrome_rel ds_d5Tf_u VV.
+Theorem monochrome__monochrome_rel' (ds_d5U0_u : Color_u) (ds_d5U0 : Color) (VV : SFBool_u):
+  ds_d5U0_u = ⌊ ds_d5U0 ⌋ → ⌊ monochrome ds_d5U0 -⌋ = VV ↔ monochrome_rel ds_d5U0_u VV.
 Proof.
-  intros ->. refine (monochrome__monochrome_rel ds_d5Tf VV).
+  intros ->. refine (monochrome__monochrome_rel ds_d5U0 VV).
 Qed.
 
 #[global] Hint Resolve monochrome__monochrome_rel': f_rel_funct_db.
 
-Theorem monochrome_rel_mk (ds_d5Tf : Color_u) (ds_d5Tf_p : Color_wf ds_d5Tf ∧ True):
-  {VV: _ | monochrome_rel ds_d5Tf VV}.
+Theorem monochrome_rel_mk (ds_d5U0 : Color_u) (ds_d5U0_p : Color_wf ds_d5U0 ∧ True):
+  {VV: _ | monochrome_rel ds_d5U0 VV}.
 Proof.
   intros;
   refine (subsumptionCast
           _
-          (λ VV, monochrome_rel ds_d5Tf VV)
-          (monochrome (exist _ ds_d5Tf ds_d5Tf_p))
+          (λ VV, monochrome_rel ds_d5U0 VV)
+          (monochrome (exist _ ds_d5U0 ds_d5U0_p))
           _);
   rewrite <- monochrome__monochrome_rel';
   quicksolve.
@@ -7070,12 +7119,12 @@ Qed.
 
 #[global] Instance monochrome_pack:
   @Pack
-  (Color ::RT λ (ds_d5Tf : Color), nilRT)
+  (Color ::RT λ (ds_d5U0 : Color), nilRT)
   (Color_u ::UT nilUT)
-  ltac:(mkProjectsArgListTG (Color ::RT λ (ds_d5Tf : Color), nilRT) ((Color_u ::UT nilUT)))
+  ltac:(mkProjectsArgListTG (Color ::RT λ (ds_d5U0 : Color), nilRT) ((Color_u ::UT nilUT)))
   SFBool_u
-  (λ (x_78541034 : ArgList (Color ::RT λ (ds_d5Tf : Color), nilRT)) (v_x_78541034 : SFBool_u),
-   ltac:(flattenP (λ (ds_d5Tf : Color) (VV : SFBool_u), SFBool_wf VV ∧ True) x_78541034 v_x_78541034)).
+  (λ (x_78360544 : ArgList (Color ::RT λ (ds_d5U0 : Color), nilRT)) (v_x_78360544 : SFBool_u),
+   ltac:(flattenP (λ (ds_d5U0 : Color) (VV : SFBool_u), SFBool_wf VV ∧ True) x_78360544 v_x_78360544)).
 Proof.
   buildPackG monochrome monochrome_rel monochrome__monochrome_rel monochrome_rel_funct.
 Defined.
